<?xml version="1.0"?>
<rdf:RDF xmlns="http://postdata.linhd.uned.es/ontology/postdata-core#"
     xml:base="http://postdata.linhd.uned.es/ontology/postdata-core"
     xmlns:dc="http://purl.org/dc/elements/1.1/"
     xmlns:ns="https://creativecommons.org/ns#"
     xmlns:edm="http://www.europeana.eu/schemas/edm/"
     xmlns:ns1="http://creativecommons.org/ns#"
     xmlns:ns2="http://www.w3.org/2003/06/sw-vocab-status/ns#"
     xmlns:owl="http://www.w3.org/2002/07/owl#"
     xmlns:rdf="http://www.w3.org/1999/02/22-rdf-syntax-ns#"
     xmlns:wot="http://xmlns.com/wot/0.1/"
     xmlns:xml="http://www.w3.org/XML/1998/namespace"
     xmlns:xsd="http://www.w3.org/2001/XMLSchema#"
     xmlns:adms="http://www.w3.org/ns/adms#"
     xmlns:foaf="http://xmlns.com/foaf/0.1/"
     xmlns:meta="http://swpatho.ag-nbi.de/context/meta.owl#"
     xmlns:opla="http://ontologydesignpatterns.org/opla/"
     xmlns:prov="http://www.w3.org/ns/prov#"
     xmlns:rdfs="http://www.w3.org/2000/01/rdf-schema#"
     xmlns:skos="http://www.w3.org/2004/02/skos/core#"
     xmlns:vann="http://purl.org/vocab/vann/"
     xmlns:voaf="http://purl.org/vocommons/voaf#"
     xmlns:regap="http://metadataregistry.org/uri/profile/regap/"
     xmlns:terms="http://purl.org/dc/terms/"
     xmlns:radion="http://www.w3.org/ns/radion#"
     xmlns:schema="http://schema.org/"
     xmlns:cpannotationschema="http://www.ontologydesignpatterns.org/schemas/cpannotationschema.owl#">
    <owl:Ontology rdf:about="http://postdata.linhd.uned.es/ontology/postdata-core">
        <ns1:license rdf:resource="https://creativecommons.org/licenses/by/4.0/"/>
        <opla:reusesPatternAsTemplate>http://purl.org/ontology/olo/core</opla:reusesPatternAsTemplate>
        <opla:reusesPatternAsTemplate>http://www.ontologydesignpatterns.org/cp/owl/agentrole.owl</opla:reusesPatternAsTemplate>
        <opla:reusesPatternAsTemplate>http://www.ontologydesignpatterns.org/cp/owl/objectrole.owl</opla:reusesPatternAsTemplate>
        <opla:reusesPatternAsTemplate>http://www.ontologydesignpatterns.org/cp/owl/partof.owl</opla:reusesPatternAsTemplate>
        <dc:contributor>Aitor Díaz Medina (LINHD_POSTDATA-UNED) 
https://www.linkedin.com/in/aitordiazmedina/</dc:contributor>
        <dc:contributor>Alvaro Pérez (LINHD_POSTDATA-UNED) 
https://www.linkedin.com/in/álvaro-pérez-pozo-ab241154/</dc:contributor>
        <dc:contributor>Bruno Sartini (Bolonia University)
https://orcid.org/0000-0002-9152-4402</dc:contributor>
        <dc:contributor>Helena Bermúdez Sabel
https://orcid.org/0000-0001-7782-206X</dc:contributor>
        <dc:contributor>Javier de la Rosa (LINHD_POSTDATA-UNED)
https://www.linkedin.com/in/versae/</dc:contributor>
        <dc:contributor>Laura Hernández Lorenzo (LINHD_POSTDATA-UNED) 
https://orcid.org/0000-0003-3489-2193</dc:contributor>
        <dc:contributor xml:lang="scc.uned.es">Mirella De Sisto (LINHD_POSTDATA-UNED) 
mdesisto</dc:contributor>
        <dc:contributor>Mª Luisa Díez Platas
https://orcid.org/0000-0002-9416-3147</dc:contributor>
        <dc:contributor>Omar Khalil Gómez (LINHD_POSTDATA-UNED) 
http://www.linkedin.com/in/omar-k-0959a8129</dc:contributor>
        <dc:contributor>Oscar Corcho (Universidad Politécnica de Madrid)
http://orcid.org/0000-0002-9260-0753</dc:contributor>
        <dc:contributor xml:lang="gmail.com">Salvador Ros Muñoz (UNED)
srosmu</dc:contributor>
        <dc:creator xml:lang="en">POSTDATA Project “This project has received funding from the European Research Council (ERC) under the European Union’s Horizon 2020 research and innovation programme (grant agreement Nº [679528])”</dc:creator>
        <dc:date>2020-02-22</dc:date>
        <dc:description xml:lang="en">This ontology is the core of the POSTDATA network of ontologies. As such, it contains the most relevant classes and properties that allow representing poetic works and their characteristics. Besides, it contains common classes and properties that are used in many other ontologies in the network, such as those related to the representation of persons, organisations, events, places and roles that persons and organisations play in poetic works.</dc:description>
        <dc:title xml:lang="en">POSTDATA core ontology</dc:title>
        <terms:publisher xml:lang="en">POSTDATA Project “This project has received funding from the European Research Council (ERC) under the European Union’s Horizon 2020 research and innovation programme (grant agreement Nº [679528])”
        Principal Investigator. Elena González Blanco -- &lt;https://orcid.org/0000-0002-0448-1812&gt;
        Technical Director. Salvador Ros Muñoz -- &lt;https://orcid.org/0000-0001-6330-4958&gt;</terms:publisher>
        <vann:preferredNamespacePrefix>pdcore</vann:preferredNamespacePrefix>
        <owl:versionInfo>V1.3</owl:versionInfo>
    </owl:Ontology>
    


    <!-- 
    ///////////////////////////////////////////////////////////////////////////////////////
    //
    // Annotation properties
    //
    ///////////////////////////////////////////////////////////////////////////////////////
     -->

    


    <!-- http://creativecommons.org/ns#license -->

    <owl:AnnotationProperty rdf:about="http://creativecommons.org/ns#license"/>
    


    <!-- http://metadataregistry.org/uri/profile/regap/name -->

    <owl:AnnotationProperty rdf:about="http://metadataregistry.org/uri/profile/regap/name"/>
    


    <!-- http://metadataregistry.org/uri/profile/regap/status -->

    <owl:AnnotationProperty rdf:about="http://metadataregistry.org/uri/profile/regap/status"/>
    


    <!-- http://ontologydesignpatterns.org/opla/reusesPatternAsTemplate -->

    <owl:AnnotationProperty rdf:about="http://ontologydesignpatterns.org/opla/reusesPatternAsTemplate"/>
    


    <!-- http://postdata.linhd.uned.es/ontology/postdata-core#note -->

    <owl:AnnotationProperty rdf:about="http://postdata.linhd.uned.es/ontology/postdata-core#note">
        <rdfs:comment xml:lang="en">A textual description offering an explanation or textual annotation about an individual of interest.</rdfs:comment>
        <rdfs:label xml:lang="en">note</rdfs:label>
    </owl:AnnotationProperty>
    


    <!-- http://purl.org/dc/elements/1.1/contributor -->

    <owl:AnnotationProperty rdf:about="http://purl.org/dc/elements/1.1/contributor"/>
    


    <!-- http://purl.org/dc/elements/1.1/contributors -->

    <owl:AnnotationProperty rdf:about="http://purl.org/dc/elements/1.1/contributors"/>
    


    <!-- http://purl.org/dc/elements/1.1/creator -->

    <owl:AnnotationProperty rdf:about="http://purl.org/dc/elements/1.1/creator"/>
    


    <!-- http://purl.org/dc/elements/1.1/date -->

    <owl:AnnotationProperty rdf:about="http://purl.org/dc/elements/1.1/date"/>
    


    <!-- http://purl.org/dc/elements/1.1/description -->

    <owl:AnnotationProperty rdf:about="http://purl.org/dc/elements/1.1/description"/>
    


    <!-- http://purl.org/dc/elements/1.1/issued -->

    <owl:AnnotationProperty rdf:about="http://purl.org/dc/elements/1.1/issued"/>
    


    <!-- http://purl.org/dc/elements/1.1/modified -->

    <owl:AnnotationProperty rdf:about="http://purl.org/dc/elements/1.1/modified"/>
    


    <!-- http://purl.org/dc/elements/1.1/title -->

    <owl:AnnotationProperty rdf:about="http://purl.org/dc/elements/1.1/title"/>
    


    <!-- http://purl.org/dc/terms/abstract -->

    <owl:AnnotationProperty rdf:about="http://purl.org/dc/terms/abstract"/>
    


    <!-- http://purl.org/dc/terms/contributor -->

    <owl:AnnotationProperty rdf:about="http://purl.org/dc/terms/contributor"/>
    


    <!-- http://purl.org/dc/terms/date -->

    <owl:AnnotationProperty rdf:about="http://purl.org/dc/terms/date"/>
    


    <!-- http://purl.org/dc/terms/description -->

    <owl:AnnotationProperty rdf:about="http://purl.org/dc/terms/description"/>
    


    <!-- http://purl.org/dc/terms/issued -->

    <owl:AnnotationProperty rdf:about="http://purl.org/dc/terms/issued"/>
    


    <!-- http://purl.org/dc/terms/modified -->

    <owl:AnnotationProperty rdf:about="http://purl.org/dc/terms/modified"/>
    


    <!-- http://purl.org/dc/terms/provenance -->

    <owl:AnnotationProperty rdf:about="http://purl.org/dc/terms/provenance"/>
    


    <!-- http://purl.org/dc/terms/publisher -->

    <owl:AnnotationProperty rdf:about="http://purl.org/dc/terms/publisher"/>
    


    <!-- http://purl.org/dc/terms/temporal -->

    <owl:AnnotationProperty rdf:about="http://purl.org/dc/terms/temporal"/>
    


    <!-- http://purl.org/dc/terms/title -->

    <owl:AnnotationProperty rdf:about="http://purl.org/dc/terms/title"/>
    


    <!-- http://purl.org/vocab/vann/changes -->

    <owl:AnnotationProperty rdf:about="http://purl.org/vocab/vann/changes"/>
    


    <!-- http://purl.org/vocab/vann/example -->

    <owl:AnnotationProperty rdf:about="http://purl.org/vocab/vann/example"/>
    


    <!-- http://purl.org/vocab/vann/preferredNamespacePrefix -->

    <owl:AnnotationProperty rdf:about="http://purl.org/vocab/vann/preferredNamespacePrefix"/>
    


    <!-- http://purl.org/vocab/vann/preferredNamespaceUri -->

    <owl:AnnotationProperty rdf:about="http://purl.org/vocab/vann/preferredNamespaceUri"/>
    


    <!-- http://purl.org/vocommons/voaf#toDoList -->

    <owl:AnnotationProperty rdf:about="http://purl.org/vocommons/voaf#toDoList"/>
    


    <!-- http://schema.org/image -->

    <owl:AnnotationProperty rdf:about="http://schema.org/image"/>
    


    <!-- http://swpatho.ag-nbi.de/context/meta.owl#hasType -->

    <owl:AnnotationProperty rdf:about="http://swpatho.ag-nbi.de/context/meta.owl#hasType"/>
    


    <!-- http://www.europeana.eu/schemas/edm/userTag -->

    <owl:AnnotationProperty rdf:about="http://www.europeana.eu/schemas/edm/userTag">
        <rdfs:label xml:lang="en">User Tag</rdfs:label>
        <skos:definition xml:lang="en">This is a tag created by a user through the Europeana interface.</skos:definition>
        <rdfs:subPropertyOf rdf:resource="http://purl.org/dc/elements/1.1/description"/>
    </owl:AnnotationProperty>
    


    <!-- http://www.ontologydesignpatterns.org/schemas/cpannotationschema.owl#coversRequirements -->

    <owl:AnnotationProperty rdf:about="http://www.ontologydesignpatterns.org/schemas/cpannotationschema.owl#coversRequirements">
        <rdfs:comment>This annotation property is used for exemplifying possible requirements the content pattern provides a solution for. Requirements are expressed as natural language competency questions.</rdfs:comment>
    </owl:AnnotationProperty>
    


    <!-- http://www.ontologydesignpatterns.org/schemas/cpannotationschema.owl#extractedFrom -->

    <owl:AnnotationProperty rdf:about="http://www.ontologydesignpatterns.org/schemas/cpannotationschema.owl#extractedFrom">
        <rdfs:comment>This annotation property should be assigned with a URI, which points to the possible reference ontology which the annotated pattern was extracted from (i.e. the reference ontology that the ontology elements have been deeply or partially cloned by). The range is not explicit in the definition of the annotation property because it would turn the ontology to OWL Full. E.g. The participation pattern is extracted from the Dolce Ultra Lite ontology, hence the value for this annotation property is http://www.ontologydesignpatterns.org/ont/dul/DUL.owl</rdfs:comment>
    </owl:AnnotationProperty>
    


    <!-- http://www.ontologydesignpatterns.org/schemas/cpannotationschema.owl#hasComponent -->

    <owl:AnnotationProperty rdf:about="http://www.ontologydesignpatterns.org/schemas/cpannotationschema.owl#hasComponent">
        <rdfs:comment>This annotation property is useful for content ontology design patterns. Its value is a URI, which refers to another content ontology design pattern which is a component of the annotated one.</rdfs:comment>
    </owl:AnnotationProperty>
    


    <!-- http://www.ontologydesignpatterns.org/schemas/cpannotationschema.owl#hasConsequences -->

    <owl:AnnotationProperty rdf:about="http://www.ontologydesignpatterns.org/schemas/cpannotationschema.owl#hasConsequences">
        <rdfs:comment>This annotation property is used for briefly describing the benefits and/or possible trade-offs when using the CP.</rdfs:comment>
    </owl:AnnotationProperty>
    


    <!-- http://www.ontologydesignpatterns.org/schemas/cpannotationschema.owl#hasIntent -->

    <owl:AnnotationProperty rdf:about="http://www.ontologydesignpatterns.org/schemas/cpannotationschema.owl#hasIntent">
        <rdfs:comment>This annotation property is used in order to describe the intent of the content pattern.</rdfs:comment>
    </owl:AnnotationProperty>
    


    <!-- http://www.ontologydesignpatterns.org/schemas/cpannotationschema.owl#hasUnitTest -->

    <owl:AnnotationProperty rdf:about="http://www.ontologydesignpatterns.org/schemas/cpannotationschema.owl#hasUnitTest">
        <rdfs:comment>This property can be used to annotate a unit test (e.g. in the form of a SPARQL query) to be launched to evaluate an ontology against a requirement-based task.</rdfs:comment>
    </owl:AnnotationProperty>
    


    <!-- http://www.ontologydesignpatterns.org/schemas/cpannotationschema.owl#isCloneOf -->

    <owl:AnnotationProperty rdf:about="http://www.ontologydesignpatterns.org/schemas/cpannotationschema.owl#isCloneOf">
        <rdfs:comment>This annotation property is used for referring a cloned ontology entity to its cloning source.</rdfs:comment>
    </owl:AnnotationProperty>
    


    <!-- http://www.ontologydesignpatterns.org/schemas/cpannotationschema.owl#isSpecializationOf -->

    <owl:AnnotationProperty rdf:about="http://www.ontologydesignpatterns.org/schemas/cpannotationschema.owl#isSpecializationOf">
        <rdfs:comment>This annotation property is useful for content ontology design patterns and its elements. Its value is a URI, which refers either to a content ontology design pattern that is specialized by the annotated one, or to an ontology element that is specialized by the annotated one.</rdfs:comment>
    </owl:AnnotationProperty>
    


    <!-- http://www.ontologydesignpatterns.org/schemas/cpannotationschema.owl#reengineeredFrom -->

    <owl:AnnotationProperty rdf:about="http://www.ontologydesignpatterns.org/schemas/cpannotationschema.owl#reengineeredFrom">
        <rdfs:comment>This annotation property should be assigned with a URI, which points to the concept schema, page, or anything else from which the annotated pattern was reengineered.  If the source does not have any URI e.g., a printed book, this property value should provide information as precise as possible in order to identify the source. This property is alternative to the extractedFrom property because it is used when the pattern come from a concept schema which is not an owl ontology. For example content ontology design patterns, which are reengineered from data model patterns, rdf schemas, etc. should be annotatd with this property. E.g. The basicpersonalfoaf pattern is extracted from the rdf FOAF specification, hence the value for this annotation property is http://xmlns.com/foaf/spec/20071002.rdf</rdfs:comment>
    </owl:AnnotationProperty>
    


    <!-- http://www.ontologydesignpatterns.org/schemas/cpannotationschema.owl#relatedCPs -->

    <owl:AnnotationProperty rdf:about="http://www.ontologydesignpatterns.org/schemas/cpannotationschema.owl#relatedCPs">
        <rdfs:comment>This annotation property can be used to indicate other CPs (if any) that specialize, generalize, inlcude, or are components of the CP. Furthermore, this field may indicate other CPs that are typically used in conjunction with the described one. Important similarities and differences with other patterns can be also described here.</rdfs:comment>
    </owl:AnnotationProperty>
    


    <!-- http://www.ontologydesignpatterns.org/schemas/cpannotationschema.owl#scenarios -->

    <owl:AnnotationProperty rdf:about="http://www.ontologydesignpatterns.org/schemas/cpannotationschema.owl#scenarios">
        <rdfs:comment>This annotation property is used for describing examples of instantiation of the Content OP. For example, for the part-of Content OP (which represents part-whole relations) a possible scenario is the sentence: &quot;the brain is part of the human body&quot;. Scenarios are expressed as natural language sentences.</rdfs:comment>
    </owl:AnnotationProperty>
    


    <!-- http://www.w3.org/2002/07/owl#maxQualifiedCardinality -->

    <owl:AnnotationProperty rdf:about="http://www.w3.org/2002/07/owl#maxQualifiedCardinality"/>
    


    <!-- http://www.w3.org/2003/06/sw-vocab-status/ns#term_status -->

    <owl:AnnotationProperty rdf:about="http://www.w3.org/2003/06/sw-vocab-status/ns#term_status">
        <rdfs:comment>the status of a vocabulary term, expressed as a short symbolic string; known values include &apos;unstable&apos;,&apos;testing&apos;, &apos;stable&apos; and &apos;archaic&apos;</rdfs:comment>
        <rdfs:isDefinedBy rdf:resource="http://www.w3.org/2003/06/sw-vocab-status/ns#"/>
        <rdfs:label>term status</rdfs:label>
        <ns2:term_status>unstable</ns2:term_status>
    </owl:AnnotationProperty>
    


    <!-- http://www.w3.org/2004/02/skos/core#altLabel -->

    <owl:AnnotationProperty rdf:about="http://www.w3.org/2004/02/skos/core#altLabel">
        <rdfs:comment xml:lang="en">The range of skos:altLabel is the class of RDF plain literals.</rdfs:comment>
        <rdfs:comment xml:lang="en">skos:prefLabel, skos:altLabel and skos:hiddenLabel are pairwise disjoint properties.</rdfs:comment>
        <rdfs:isDefinedBy rdf:resource="http://www.w3.org/2004/02/skos/core"/>
        <rdfs:label xml:lang="en">alternative label</rdfs:label>
        <skos:definition xml:lang="en">An alternative lexical label for a resource.</skos:definition>
        <skos:example xml:lang="en">Acronyms, abbreviations, spelling variants, and irregular plural/singular forms may be included among the alternative labels for a concept. Mis-spelled terms are normally included as hidden labels (see skos:hiddenLabel).</skos:example>
        <rdfs:subPropertyOf rdf:resource="http://www.w3.org/2000/01/rdf-schema#label"/>
    </owl:AnnotationProperty>
    


    <!-- http://www.w3.org/2004/02/skos/core#changeNote -->

    <owl:AnnotationProperty rdf:about="http://www.w3.org/2004/02/skos/core#changeNote">
        <rdfs:isDefinedBy rdf:resource="http://www.w3.org/2004/02/skos/core"/>
        <rdfs:label xml:lang="en">change note</rdfs:label>
        <skos:definition xml:lang="en">A note about a modification to a concept.</skos:definition>
        <rdfs:subPropertyOf rdf:resource="http://www.w3.org/2004/02/skos/core#note"/>
    </owl:AnnotationProperty>
    


    <!-- http://www.w3.org/2004/02/skos/core#definition -->

    <owl:AnnotationProperty rdf:about="http://www.w3.org/2004/02/skos/core#definition">
        <rdfs:isDefinedBy rdf:resource="http://www.w3.org/2004/02/skos/core"/>
        <rdfs:label xml:lang="en">definition</rdfs:label>
        <skos:definition xml:lang="en">A statement or formal explanation of the meaning of a concept.</skos:definition>
        <rdfs:subPropertyOf rdf:resource="http://www.w3.org/2004/02/skos/core#note"/>
    </owl:AnnotationProperty>
    


    <!-- http://www.w3.org/2004/02/skos/core#editorialNote -->

    <owl:AnnotationProperty rdf:about="http://www.w3.org/2004/02/skos/core#editorialNote">
        <rdfs:isDefinedBy rdf:resource="http://www.w3.org/2004/02/skos/core"/>
        <rdfs:label xml:lang="en">editorial note</rdfs:label>
        <skos:definition xml:lang="en">A note for an editor, translator or maintainer of the vocabulary.</skos:definition>
        <rdfs:subPropertyOf rdf:resource="http://www.w3.org/2004/02/skos/core#note"/>
    </owl:AnnotationProperty>
    


    <!-- http://www.w3.org/2004/02/skos/core#example -->

    <owl:AnnotationProperty rdf:about="http://www.w3.org/2004/02/skos/core#example">
        <rdfs:isDefinedBy rdf:resource="http://www.w3.org/2004/02/skos/core"/>
        <rdfs:label xml:lang="en">example</rdfs:label>
        <skos:definition xml:lang="en">An example of the use of a concept.</skos:definition>
        <rdfs:subPropertyOf rdf:resource="http://www.w3.org/2004/02/skos/core#note"/>
    </owl:AnnotationProperty>
    


    <!-- http://www.w3.org/2004/02/skos/core#hasTopConcept -->

    <owl:AnnotationProperty rdf:about="http://www.w3.org/2004/02/skos/core#hasTopConcept"/>
    


    <!-- http://www.w3.org/2004/02/skos/core#hiddenLabel -->

    <owl:AnnotationProperty rdf:about="http://www.w3.org/2004/02/skos/core#hiddenLabel">
        <rdfs:comment xml:lang="en">The range of skos:hiddenLabel is the class of RDF plain literals.</rdfs:comment>
        <rdfs:comment xml:lang="en">skos:prefLabel, skos:altLabel and skos:hiddenLabel are pairwise disjoint properties.</rdfs:comment>
        <rdfs:isDefinedBy rdf:resource="http://www.w3.org/2004/02/skos/core"/>
        <rdfs:label xml:lang="en">hidden label</rdfs:label>
        <skos:definition xml:lang="en">A lexical label for a resource that should be hidden when generating visual displays of the resource, but should still be accessible to free text search operations.</skos:definition>
        <rdfs:subPropertyOf rdf:resource="http://www.w3.org/2000/01/rdf-schema#label"/>
    </owl:AnnotationProperty>
    


    <!-- http://www.w3.org/2004/02/skos/core#historyNote -->

    <owl:AnnotationProperty rdf:about="http://www.w3.org/2004/02/skos/core#historyNote">
        <rdfs:isDefinedBy rdf:resource="http://www.w3.org/2004/02/skos/core"/>
        <rdfs:label xml:lang="en">history note</rdfs:label>
        <skos:definition xml:lang="en">A note about the past state/use/meaning of a concept.</skos:definition>
        <rdfs:subPropertyOf rdf:resource="http://www.w3.org/2004/02/skos/core#note"/>
    </owl:AnnotationProperty>
    


    <!-- http://www.w3.org/2004/02/skos/core#notation -->

    <owl:AnnotationProperty rdf:about="http://www.w3.org/2004/02/skos/core#notation"/>
    


    <!-- http://www.w3.org/2004/02/skos/core#note -->

    <owl:AnnotationProperty rdf:about="http://www.w3.org/2004/02/skos/core#note">
        <rdfs:isDefinedBy rdf:resource="http://www.w3.org/2004/02/skos/core"/>
        <rdfs:label xml:lang="en">note</rdfs:label>
        <skos:definition xml:lang="en">A general note, for any purpose.</skos:definition>
        <skos:scopeNote xml:lang="en">This property may be used directly, or as a super-property for more specific note types.</skos:scopeNote>
    </owl:AnnotationProperty>
    


    <!-- http://www.w3.org/2004/02/skos/core#prefLabel -->

    <owl:AnnotationProperty rdf:about="http://www.w3.org/2004/02/skos/core#prefLabel">
        <rdfs:comment xml:lang="en">A resource has no more than one value of skos:prefLabel per language tag, and no more than one value of skos:prefLabel without language tag.</rdfs:comment>
        <rdfs:comment xml:lang="en">The range of skos:prefLabel is the class of RDF plain literals.</rdfs:comment>
        <rdfs:comment xml:lang="en">skos:prefLabel, skos:altLabel and skos:hiddenLabel are pairwise
      disjoint properties.</rdfs:comment>
        <rdfs:isDefinedBy rdf:resource="http://www.w3.org/2004/02/skos/core"/>
        <rdfs:label xml:lang="en">preferred label</rdfs:label>
        <skos:definition xml:lang="en">The preferred lexical label for a resource, in a given language.</skos:definition>
        <rdfs:subPropertyOf rdf:resource="http://www.w3.org/2000/01/rdf-schema#label"/>
    </owl:AnnotationProperty>
    


    <!-- http://www.w3.org/2004/02/skos/core#scopeNote -->

    <owl:AnnotationProperty rdf:about="http://www.w3.org/2004/02/skos/core#scopeNote">
        <rdfs:isDefinedBy rdf:resource="http://www.w3.org/2004/02/skos/core"/>
        <rdfs:label xml:lang="en">scope note</rdfs:label>
        <skos:definition xml:lang="en">A note that helps to clarify the meaning and/or the use of a concept.</skos:definition>
        <rdfs:subPropertyOf rdf:resource="http://www.w3.org/2004/02/skos/core#note"/>
    </owl:AnnotationProperty>
    


    <!-- http://www.w3.org/ns/adms#relatedDocumentation -->

    <owl:AnnotationProperty rdf:about="http://www.w3.org/ns/adms#relatedDocumentation"/>
    


    <!-- http://www.w3.org/ns/adms#relatedWebPage -->

    <owl:AnnotationProperty rdf:about="http://www.w3.org/ns/adms#relatedWebPage"/>
    


    <!-- http://www.w3.org/ns/prov#wasAttributedTo -->

    <owl:AnnotationProperty rdf:about="http://www.w3.org/ns/prov#wasAttributedTo"/>
    


    <!-- http://www.w3.org/ns/radion#versionNotes -->

    <owl:AnnotationProperty rdf:about="http://www.w3.org/ns/radion#versionNotes"/>
    


    <!-- http://xmlns.com/foaf/0.1/membershipClass -->

    <owl:AnnotationProperty rdf:about="http://xmlns.com/foaf/0.1/membershipClass">
        <rdfs:comment>Indicates the class of individuals that are a member of a Group</rdfs:comment>
        <rdfs:isDefinedBy rdf:resource="http://xmlns.com/foaf/0.1/"/>
        <rdfs:label>membershipClass</rdfs:label>
        <ns2:term_status>unstable</ns2:term_status>
    </owl:AnnotationProperty>
    


    <!-- http://xmlns.com/wot/0.1/assurance -->

    <owl:AnnotationProperty rdf:about="http://xmlns.com/wot/0.1/assurance"/>
    


    <!-- https://creativecommons.org/ns#license -->

    <owl:AnnotationProperty rdf:about="https://creativecommons.org/ns#license"/>
    


    <!-- 
    ///////////////////////////////////////////////////////////////////////////////////////
    //
    // Datatypes
    //
    ///////////////////////////////////////////////////////////////////////////////////////
     -->

    


    <!-- http://www.w3.org/2001/XMLSchema#date -->

    <rdfs:Datatype rdf:about="http://www.w3.org/2001/XMLSchema#date"/>
    


    <!-- 
    ///////////////////////////////////////////////////////////////////////////////////////
    //
    // Object Properties
    //
    ///////////////////////////////////////////////////////////////////////////////////////
     -->

    


    <!-- http://iflastandards.info/ns/fr/frbr/frbroo/R2 -->

    <owl:ObjectProperty rdf:about="http://iflastandards.info/ns/fr/frbr/frbroo/R2">
        <owl:inverseOf rdf:resource="http://iflastandards.info/ns/fr/frbr/frbroo/R2i"/>
        <rdfs:domain rdf:resource="http://iflastandards.info/ns/fr/frbr/frbroo/F1"/>
        <rdfs:range rdf:resource="http://iflastandards.info/ns/fr/frbr/frbroo/F1"/>
        <regap:name xml:lang="en">isDerivativeOf</regap:name>
        <rdfs:comment xml:lang="en">This property associates an instance of F1 Work which modifies the content of another instance of F1 Work with the latter. The property R2.1 has type of this property allows for specifying the kind of derivation, such as adaptation, summarisation etc.</rdfs:comment>
        <rdfs:isDefinedBy>http://iflastandards.info/ns/fr/frbr/frbroo/</rdfs:isDefinedBy>
        <rdfs:label xml:lang="en">is derivative of</rdfs:label>
        <skos:scopeNote xml:lang="en">The property R2.1 has type of this property allows for specifying the kind of derivation, such as adaptation, summarisation etc.</skos:scopeNote>
    </owl:ObjectProperty>
    


    <!-- http://iflastandards.info/ns/fr/frbr/frbroo/R2i -->

    <owl:ObjectProperty rdf:about="http://iflastandards.info/ns/fr/frbr/frbroo/R2i">
        <rdfs:domain rdf:resource="http://iflastandards.info/ns/fr/frbr/frbroo/F1"/>
        <rdfs:range rdf:resource="http://iflastandards.info/ns/fr/frbr/frbroo/F1"/>
        <regap:name xml:lang="en">hasDerivative</regap:name>
        <rdfs:comment xml:lang="en">Inverse of R2_is_derivative_of.</rdfs:comment>
        <rdfs:isDefinedBy>http://iflastandards.info/ns/fr/frbr/frbroo/</rdfs:isDefinedBy>
        <rdfs:label xml:lang="en">has derivative</rdfs:label>
    </owl:ObjectProperty>
    


    <!-- http://iflastandards.info/ns/fr/frbr/frbroo/R3 -->

    <owl:ObjectProperty rdf:about="http://iflastandards.info/ns/fr/frbr/frbroo/R3">
        <owl:inverseOf rdf:resource="http://iflastandards.info/ns/fr/frbr/frbroo/R3i"/>
        <rdfs:domain rdf:resource="http://iflastandards.info/ns/fr/frbr/frbroo/F1"/>
        <rdfs:range rdf:resource="http://iflastandards.info/ns/fr/frbr/frbroo/F22"/>
        <regap:name xml:lang="en">isRealisedInSelfContainedExpressionOfWork</regap:name>
        <rdfs:comment xml:lang="en">This property associates an instance of F22 Self-Contained Expression with an instance of F1 Work. This property expresses the association that exists between an expression (F22) and the work that this expression conveys. The semantics of the association will be different depending on what specific subtype of F1 Work the work is an instance of. If the work is an instance of F14 Individual Work, the F22 Self-Contained Expression completely conveys the individual work. If the work is an instance of F15 Complex work, the F22 Self-Contained Expression conveys an alternative member of the complex work. Our factual knowledge of how a given work is realised into an expression is often limited and this property makes it possible to express the association between instances of F22 Self-Contained Expression and the work it conveys without using the more developed paths.</rdfs:comment>
        <rdfs:isDefinedBy>http://iflastandards.info/ns/fr/frbr/frbroo/</rdfs:isDefinedBy>
        <rdfs:label xml:lang="en">is realised in Self-Contained Expression of Work</rdfs:label>
        <skos:definition xml:lang="en">This property associates an instance of F22 Self-Contained Expression with an instance of F1 Work.</skos:definition>
        <skos:scopeNote xml:lang="en">This property expresses the association that exists between an expression (F22) and the work that this expression conveys. The semantics of the association will be different depending on what specific subtype of F1 Work the work is an instance of. If the work is an instance of F14 Individual Work, the F22 Self-Contained Expression completely conveys the individual work. If the work is an instance of F15 Complex work, the F22 Self-Contained Expression conveys an alternative member of the complex work. Our factual knowledge of how a given work is realised into an expression is often limited and this property makes it possible to express the association between instances of F22 Self-Contained Expression and the work it conveys without using the more developed paths.</skos:scopeNote>
    </owl:ObjectProperty>
    


    <!-- http://iflastandards.info/ns/fr/frbr/frbroo/R3i -->

    <owl:ObjectProperty rdf:about="http://iflastandards.info/ns/fr/frbr/frbroo/R3i">
        <rdfs:domain rdf:resource="http://iflastandards.info/ns/fr/frbr/frbroo/F22"/>
        <rdfs:range rdf:resource="http://iflastandards.info/ns/fr/frbr/frbroo/F1"/>
        <regap:name xml:lang="en">realisesWorkBySelfContainedExpression</regap:name>
        <rdfs:comment xml:lang="en">Inverse of R3_is_realised_in.</rdfs:comment>
        <rdfs:isDefinedBy>http://iflastandards.info/ns/fr/frbr/frbroo/</rdfs:isDefinedBy>
        <rdfs:label xml:lang="en">realises Work by Self-Contained Expression</rdfs:label>
    </owl:ObjectProperty>
    


    <!-- http://postdata.linhd.uned.es/ontology/postdata-core#additionalFile -->

    <owl:ObjectProperty rdf:about="http://postdata.linhd.uned.es/ontology/postdata-core#additionalFile">
        <rdfs:subPropertyOf rdf:resource="http://www.europeana.eu/schemas/edm/isShownBy"/>
        <rdfs:domain rdf:resource="http://postdata.linhd.uned.es/ontology/postdata-core#Redaction"/>
        <rdfs:comment xml:lang="en">A file (XML, PFD, plain text) which contains the Redaction and, likely, other type of analytical information.

Taking as example the poem &quot;Amadís de Gaula a Don Quijote de la Mancha&quot;: Redaction could be an XML-TEI file (for example, the TEI annotated text of ADSO corpus (https://github.com/bncolorado/CorpusSonetosSigloDeOro/blob/master/Cervantes/Cervantes_1.xml)), whereas &quot;additionalFile&quot; could be another file containing a plain text version of the same poem.

This property is a subproperty of edm:isShownBy to keep an alignment with the Europeana Data Model.</rdfs:comment>
        <rdfs:isDefinedBy>http://postdata.linhd.uned.es/ontology/postdata-core/</rdfs:isDefinedBy>
        <rdfs:label xml:lang="en">additional File</rdfs:label>
    </owl:ObjectProperty>
    


    <!-- http://postdata.linhd.uned.es/ontology/postdata-core#audicenceEducationLevel -->

    <owl:ObjectProperty rdf:about="http://postdata.linhd.uned.es/ontology/postdata-core#audicenceEducationLevel">
        <rdfs:domain rdf:resource="http://postdata.linhd.uned.es/ontology/postdata-core#Redaction"/>
        <rdfs:range rdf:resource="http://www.w3.org/2004/02/skos/core#Concept"/>
        <rdfs:range>
            <owl:Restriction>
                <owl:onProperty rdf:resource="http://www.w3.org/2004/02/skos/core#inScheme"/>
                <owl:hasValue rdf:resource="http://postdata.linhd.uned.es/kos/education-level"/>
            </owl:Restriction>
        </rdfs:range>
        <rdfs:comment xml:lang="en">Level of education of the recipients of a Redaction.

Taking as example the play &quot;La segunda Celestina&quot; (Agustín de Salazar), &quot;audienceEducationLevel&quot; would be a learned audience.</rdfs:comment>
        <rdfs:label xml:lang="en">audience Education Level</rdfs:label>
    </owl:ObjectProperty>
    


    <!-- http://postdata.linhd.uned.es/ontology/postdata-core#authorEducationLevel -->

    <owl:ObjectProperty rdf:about="http://postdata.linhd.uned.es/ontology/postdata-core#authorEducationLevel">
        <rdfs:domain rdf:resource="http://postdata.linhd.uned.es/ontology/postdata-core#PoeticWork"/>
        <rdfs:range rdf:resource="http://www.w3.org/2004/02/skos/core#Concept"/>
        <rdfs:range>
            <owl:Restriction>
                <owl:onProperty rdf:resource="http://www.w3.org/2004/02/skos/core#inScheme"/>
                <owl:hasValue rdf:resource="http://postdata.linhd.uned.es/kos/education-level"/>
            </owl:Restriction>
        </rdfs:range>
        <rdfs:comment xml:lang="en">Level of education of the creator of a text/song. This property has as Domain PoeticWork and not Person since the education level of a person changes during time. That is, this is the education level of the author in the moment of writing the poem.</rdfs:comment>
        <rdfs:isDefinedBy>http://postdata.linhd.uned.es/ontology/postdata-core/</rdfs:isDefinedBy>
        <rdfs:label xml:lang="en">author Education Level</rdfs:label>
    </owl:ObjectProperty>
    


    <!-- http://postdata.linhd.uned.es/ontology/postdata-core#birthDate -->

    <owl:ObjectProperty rdf:about="http://postdata.linhd.uned.es/ontology/postdata-core#birthDate">
        <rdfs:subPropertyOf rdf:resource="http://www.w3.org/2002/07/owl#topObjectProperty"/>
        <rdfs:domain rdf:resource="http://postdata.linhd.uned.es/ontology/postdata-core#Person"/>
        <rdfs:range rdf:resource="http://postdata.linhd.uned.es/ontology/postdata-dates#DateEntity"/>
        <rdfs:comment xml:lang="en">Date of birth</rdfs:comment>
        <rdfs:isDefinedBy>http://postdata.linhd.uned.es/ontology/postdata-core/</rdfs:isDefinedBy>
        <rdfs:label xml:lang="en">birth Date</rdfs:label>
    </owl:ObjectProperty>
    


    <!-- http://postdata.linhd.uned.es/ontology/postdata-core#birthPlace -->

    <owl:ObjectProperty rdf:about="http://postdata.linhd.uned.es/ontology/postdata-core#birthPlace">
        <rdfs:subPropertyOf rdf:resource="http://postdata.linhd.uned.es/ontology/postdata-core#isFrom"/>
        <owl:inverseOf rdf:resource="http://postdata.linhd.uned.es/ontology/postdata-core#birthPlaceOf"/>
        <rdfs:domain rdf:resource="http://postdata.linhd.uned.es/ontology/postdata-core#Person"/>
        <rdfs:range rdf:resource="http://postdata.linhd.uned.es/ontology/postdata-core#Place"/>
        <rdfs:comment xml:lang="en">This property points to the Place which is the provenance of the current instance of Person</rdfs:comment>
        <rdfs:isDefinedBy>http://postdata.linhd.uned.es/ontology/postdata-core/</rdfs:isDefinedBy>
        <rdfs:label xml:lang="en">birth Place</rdfs:label>
    </owl:ObjectProperty>
    


    <!-- http://postdata.linhd.uned.es/ontology/postdata-core#birthPlaceCertainty -->

    <owl:ObjectProperty rdf:about="http://postdata.linhd.uned.es/ontology/postdata-core#birthPlaceCertainty">
        <rdfs:subPropertyOf rdf:resource="http://postdata.linhd.uned.es/ontology/postdata-core#certainty"/>
        <rdfs:domain rdf:resource="http://postdata.linhd.uned.es/ontology/postdata-core#Person"/>
        <rdfs:comment xml:lang="en">Certainty of the date of birth of a Person</rdfs:comment>
        <rdfs:isDefinedBy>http://postdata.linhd.uned.es/ontology/postdata-core/</rdfs:isDefinedBy>
        <rdfs:label xml:lang="en">birth Place Certainty</rdfs:label>
    </owl:ObjectProperty>
    


    <!-- http://postdata.linhd.uned.es/ontology/postdata-core#birthPlaceOf -->

    <owl:ObjectProperty rdf:about="http://postdata.linhd.uned.es/ontology/postdata-core#birthPlaceOf">
        <rdfs:domain rdf:resource="http://postdata.linhd.uned.es/ontology/postdata-core#Place"/>
        <rdfs:range rdf:resource="http://postdata.linhd.uned.es/ontology/postdata-core#Person"/>
        <rdfs:comment xml:lang="en">This property points to a Person who was born in the Place</rdfs:comment>
        <rdfs:isDefinedBy>http://postdata.linhd.uned.es/ontology/postdata-core/</rdfs:isDefinedBy>
        <rdfs:label xml:lang="en">birth Place Of</rdfs:label>
    </owl:ObjectProperty>
    


    <!-- http://postdata.linhd.uned.es/ontology/postdata-core#certainty -->

    <owl:ObjectProperty rdf:about="http://postdata.linhd.uned.es/ontology/postdata-core#certainty">
        <rdfs:range rdf:resource="http://www.w3.org/2004/02/skos/core#Concept"/>
        <rdfs:range>
            <owl:Restriction>
                <owl:onProperty rdf:resource="http://www.w3.org/2004/02/skos/core#inScheme"/>
                <owl:hasValue rdf:resource="http://postdata.linhd.uned.es/kos/certainty"/>
            </owl:Restriction>
        </rdfs:range>
        <rdfs:comment xml:lang="en">Level of confidence regarding the correspondent function</rdfs:comment>
        <rdfs:isDefinedBy>http://postdata.linhd.uned.es/ontology/postdata-core/</rdfs:isDefinedBy>
        <rdfs:label xml:lang="en">certainty</rdfs:label>
    </owl:ObjectProperty>
    


    <!-- http://postdata.linhd.uned.es/ontology/postdata-core#characterIn -->

    <owl:ObjectProperty rdf:about="http://postdata.linhd.uned.es/ontology/postdata-core#characterIn">
        <owl:inverseOf rdf:resource="http://postdata.linhd.uned.es/ontology/postdata-core#hasCharacter"/>
        <rdfs:domain rdf:resource="http://postdata.linhd.uned.es/ontology/postdata-core#Agent"/>
        <rdfs:range rdf:resource="http://postdata.linhd.uned.es/ontology/postdata-core#Redaction"/>
        <rdfs:comment xml:lang="en">This property points to the text in which the current instance of Person or Organisation is a character.</rdfs:comment>
        <rdfs:isDefinedBy>http://postdata.linhd.uned.es/ontology/postdata-core/</rdfs:isDefinedBy>
        <rdfs:label xml:lang="en">character In</rdfs:label>
    </owl:ObjectProperty>
    


    <!-- http://postdata.linhd.uned.es/ontology/postdata-core#date -->

    <owl:ObjectProperty rdf:about="http://postdata.linhd.uned.es/ontology/postdata-core#date">
        <rdfs:range rdf:resource="http://postdata.linhd.uned.es/ontology/postdata-dates#DateEntity"/>
        <rdfs:comment xml:lang="en">This property points to a date entity, which represents a particular point or period of time at which something happened or existed, or is expected to happen</rdfs:comment>
        <rdfs:isDefinedBy>http://postdata.linhd.uned.es/ontology/postdata-core/</rdfs:isDefinedBy>
        <rdfs:label xml:lang="en">date</rdfs:label>
    </owl:ObjectProperty>
    


    <!-- http://postdata.linhd.uned.es/ontology/postdata-core#deathDate -->

    <owl:ObjectProperty rdf:about="http://postdata.linhd.uned.es/ontology/postdata-core#deathDate">
        <rdfs:subPropertyOf rdf:resource="http://www.w3.org/2002/07/owl#topObjectProperty"/>
        <rdfs:domain rdf:resource="http://postdata.linhd.uned.es/ontology/postdata-core#Person"/>
        <rdfs:range rdf:resource="http://postdata.linhd.uned.es/ontology/postdata-dates#DateEntity"/>
        <rdfs:comment xml:lang="en">Date of death</rdfs:comment>
        <rdfs:isDefinedBy>http://postdata.linhd.uned.es/ontology/postdata-core/</rdfs:isDefinedBy>
        <rdfs:label xml:lang="en">death Date</rdfs:label>
    </owl:ObjectProperty>
    


    <!-- http://postdata.linhd.uned.es/ontology/postdata-core#deathPlace -->

    <owl:ObjectProperty rdf:about="http://postdata.linhd.uned.es/ontology/postdata-core#deathPlace">
        <owl:inverseOf rdf:resource="http://postdata.linhd.uned.es/ontology/postdata-core#deathPlaceOf"/>
        <rdfs:domain rdf:resource="http://postdata.linhd.uned.es/ontology/postdata-core#Person"/>
        <rdfs:range rdf:resource="http://postdata.linhd.uned.es/ontology/postdata-core#Place"/>
        <rdfs:comment xml:lang="en">This property points to the instance of Place where the Person died</rdfs:comment>
        <rdfs:isDefinedBy>http://postdata.linhd.uned.es/ontology/postdata-core/</rdfs:isDefinedBy>
        <rdfs:label xml:lang="en">death Place</rdfs:label>
    </owl:ObjectProperty>
    


    <!-- http://postdata.linhd.uned.es/ontology/postdata-core#deathPlaceOf -->

    <owl:ObjectProperty rdf:about="http://postdata.linhd.uned.es/ontology/postdata-core#deathPlaceOf">
        <rdfs:domain rdf:resource="http://postdata.linhd.uned.es/ontology/postdata-core#Place"/>
        <rdfs:range rdf:resource="http://postdata.linhd.uned.es/ontology/postdata-core#Person"/>
        <rdfs:comment xml:lang="en">This property points to a Person who died in the current instance of Place</rdfs:comment>
        <rdfs:isDefinedBy>http://postdata.linhd.uned.es/ontology/postdata-core/</rdfs:isDefinedBy>
        <rdfs:label xml:lang="en">death Place Of</rdfs:label>
    </owl:ObjectProperty>
    


    <!-- http://postdata.linhd.uned.es/ontology/postdata-core#dedicatedTo -->

    <owl:ObjectProperty rdf:about="http://postdata.linhd.uned.es/ontology/postdata-core#dedicatedTo">
        <owl:inverseOf rdf:resource="http://postdata.linhd.uned.es/ontology/postdata-core#hasDedication"/>
        <rdfs:domain rdf:resource="http://postdata.linhd.uned.es/ontology/postdata-core#Redaction"/>
        <rdfs:range rdf:resource="http://postdata.linhd.uned.es/ontology/postdata-core#Person"/>
        <rdfs:comment xml:lang="en">This property points to a Person to whom the current text was dedicated. This means that a Redaction includes a dedicated text to another person in an explicit way (frequently at the beginning of the text).</rdfs:comment>
        <rdfs:isDefinedBy>http://postdata.linhd.uned.es/ontology/postdata-core/</rdfs:isDefinedBy>
        <rdfs:label xml:lang="en">dedicated To</rdfs:label>
    </owl:ObjectProperty>
    


    <!-- http://postdata.linhd.uned.es/ontology/postdata-core#editedIn -->

    <owl:ObjectProperty rdf:about="http://postdata.linhd.uned.es/ontology/postdata-core#editedIn">
        <rdfs:domain rdf:resource="http://postdata.linhd.uned.es/ontology/postdata-core#Redaction"/>
        <rdfs:range rdf:resource="http://postdata.linhd.uned.es/ontology/postdata-transmission#Location"/>
        <rdfs:comment xml:lang="en">This property points to the specific Location in a bibliographic item that contains an edition of the current instance of Redaction.</rdfs:comment>
        <rdfs:isDefinedBy>http://postdata.linhd.uned.es/ontology/postdata-core/</rdfs:isDefinedBy>
        <rdfs:label xml:lang="en">edited In</rdfs:label>
    </owl:ObjectProperty>
    


    <!-- http://postdata.linhd.uned.es/ontology/postdata-core#firstPartOf -->

    <owl:ObjectProperty rdf:about="http://postdata.linhd.uned.es/ontology/postdata-core#firstPartOf">
        <rdfs:subPropertyOf rdf:resource="http://postdata.linhd.uned.es/ontology/postdata-core#isPartOf"/>
        <owl:inverseOf rdf:resource="http://postdata.linhd.uned.es/ontology/postdata-core#hasFirstPart"/>
        <rdfs:range rdf:resource="http://postdata.linhd.uned.es/ontology/postdata-core#Redaction"/>
        <rdfs:comment xml:lang="en">This property points to the container (an instance of Redaction) of which the item at hand is its first part</rdfs:comment>
        <rdfs:comment xml:lang="en">first Part of</rdfs:comment>
        <rdfs:isDefinedBy>http://postdata.linhd.uned.es/ontology/postdata-core/</rdfs:isDefinedBy>
    </owl:ObjectProperty>
    


    <!-- http://postdata.linhd.uned.es/ontology/postdata-core#floruit -->

    <owl:ObjectProperty rdf:about="http://postdata.linhd.uned.es/ontology/postdata-core#floruit">
        <rdfs:domain rdf:resource="http://postdata.linhd.uned.es/ontology/postdata-core#Person"/>
        <rdfs:range rdf:resource="http://postdata.linhd.uned.es/ontology/postdata-dates#DateEntity"/>
        <rdfs:comment xml:lang="en">The period of activity of a person, used when a range cannot be established (e.g. “3rd century”)</rdfs:comment>
        <rdfs:isDefinedBy>http://postdata.linhd.uned.es/ontology/postdata-core/</rdfs:isDefinedBy>
        <rdfs:label xml:lang="en">floruit</rdfs:label>
    </owl:ObjectProperty>
    


    <!-- http://postdata.linhd.uned.es/ontology/postdata-core#gender -->

    <owl:ObjectProperty rdf:about="http://postdata.linhd.uned.es/ontology/postdata-core#gender">
        <rdfs:domain rdf:resource="http://postdata.linhd.uned.es/ontology/postdata-core#Person"/>
        <rdfs:range rdf:resource="http://www.w3.org/2004/02/skos/core#Concept"/>
        <rdfs:range>
            <owl:Restriction>
                <owl:onProperty rdf:resource="http://www.w3.org/2004/02/skos/core#inScheme"/>
                <owl:hasValue rdf:resource="http://postdata.linhd.uned.es/kos/gender"/>
            </owl:Restriction>
        </rdfs:range>
        <rdfs:comment xml:lang="en">The gender of a Person</rdfs:comment>
        <rdfs:isDefinedBy>http://postdata.linhd.uned.es/ontology/postdata-core/</rdfs:isDefinedBy>
        <rdfs:label xml:lang="en">gender</rdfs:label>
    </owl:ObjectProperty>
    


    <!-- http://postdata.linhd.uned.es/ontology/postdata-core#genre -->

    <owl:ObjectProperty rdf:about="http://postdata.linhd.uned.es/ontology/postdata-core#genre">
        <rdfs:domain>
            <owl:Class>
                <owl:unionOf rdf:parseType="Collection">
                    <rdf:Description rdf:about="http://postdata.linhd.uned.es/ontology/postdata-core#PoeticWork"/>
                    <rdf:Description rdf:about="http://postdata.linhd.uned.es/ontology/postdata-core#Redaction"/>
                </owl:unionOf>
            </owl:Class>
        </rdfs:domain>
        <rdfs:range rdf:resource="http://www.w3.org/2004/02/skos/core#Concept"/>
        <rdfs:range>
            <owl:Restriction>
                <owl:onProperty rdf:resource="http://www.w3.org/2004/02/skos/core#inScheme"/>
                <owl:hasValue rdf:resource="http://postdata.linhd.uned.es/kos/genre"/>
            </owl:Restriction>
        </rdfs:range>
        <rdfs:comment xml:lang="en">Type of art, literature or music characterized by a specific form, content and style</rdfs:comment>
        <rdfs:isDefinedBy>http://postdata.linhd.uned.es/ontology/postdata-core/</rdfs:isDefinedBy>
        <rdfs:label xml:lang="en">genre</rdfs:label>
    </owl:ObjectProperty>
    


    <!-- http://postdata.linhd.uned.es/ontology/postdata-core#hasAgent -->

    <owl:ObjectProperty rdf:about="http://postdata.linhd.uned.es/ontology/postdata-core#hasAgent">
        <owl:inverseOf rdf:resource="http://postdata.linhd.uned.es/ontology/postdata-core#isAgentOf"/>
        <rdfs:domain rdf:resource="http://postdata.linhd.uned.es/ontology/postdata-core#AgentRole"/>
        <rdfs:range rdf:resource="http://postdata.linhd.uned.es/ontology/postdata-core#Agent"/>
        <rdfs:comment xml:lang="en">This property points to the Agent that participates in the Agent-Role aggregation.

This property emerges by reusing the Agent-Role Ontology Design Pattern:
- http://www.ontologydesignpatterns.org/cp/owl/agentrole.owl
- http://www.ontologydesignpatterns.org/cp/owl/objectrole.owl</rdfs:comment>
        <rdfs:isDefinedBy>http://postdata.linhd.uned.es/ontology/postdata-core/</rdfs:isDefinedBy>
        <rdfs:label xml:lang="en">has Agent</rdfs:label>
    </owl:ObjectProperty>
    


    <!-- http://postdata.linhd.uned.es/ontology/postdata-core#hasAgentRole -->

    <owl:ObjectProperty rdf:about="http://postdata.linhd.uned.es/ontology/postdata-core#hasAgentRole">
        <owl:inverseOf rdf:resource="http://postdata.linhd.uned.es/ontology/postdata-core#isAgentRoleOf"/>
        <rdfs:domain>
            <owl:Class>
                <owl:unionOf rdf:parseType="Collection">
                    <rdf:Description rdf:about="http://postdata.linhd.uned.es/ontology/postdata-core#Ensemble"/>
                    <rdf:Description rdf:about="http://postdata.linhd.uned.es/ontology/postdata-core#PoeticWork"/>
                    <rdf:Description rdf:about="http://postdata.linhd.uned.es/ontology/postdata-core#Redaction"/>
                </owl:unionOf>
            </owl:Class>
        </rdfs:domain>
        <rdfs:range rdf:resource="http://postdata.linhd.uned.es/ontology/postdata-core#AgentRole"/>
        <rdfs:comment xml:lang="en">This property points to an entity AgentRole that represents an Agent who plays a Role (such as an editor, critic or sponsor) associated to a given Poetic Work, a Redaction or an Ensemble</rdfs:comment>
        <rdfs:isDefinedBy>http://postdata.linhd.uned.es/ontology/postdata-core/</rdfs:isDefinedBy>
        <rdfs:label xml:lang="en">has Agent Role</rdfs:label>
    </owl:ObjectProperty>
    


    <!-- http://postdata.linhd.uned.es/ontology/postdata-core#hasCharacter -->

    <owl:ObjectProperty rdf:about="http://postdata.linhd.uned.es/ontology/postdata-core#hasCharacter">
        <rdfs:domain rdf:resource="http://postdata.linhd.uned.es/ontology/postdata-core#Redaction"/>
        <rdfs:range rdf:resource="http://postdata.linhd.uned.es/ontology/postdata-core#Agent"/>
        <rdfs:comment xml:lang="en">This property points to a character depicted in the text of a Redaction, if any. The character is an instance of Agent (Organisation or Person).</rdfs:comment>
        <rdfs:isDefinedBy>http://postdata.linhd.uned.es/ontology/postdata-core/</rdfs:isDefinedBy>
        <rdfs:label xml:lang="en">has Character</rdfs:label>
    </owl:ObjectProperty>
    


    <!-- http://postdata.linhd.uned.es/ontology/postdata-core#hasDedication -->

    <owl:ObjectProperty rdf:about="http://postdata.linhd.uned.es/ontology/postdata-core#hasDedication">
        <rdfs:domain rdf:resource="http://postdata.linhd.uned.es/ontology/postdata-core#Person"/>
        <rdfs:range rdf:resource="http://postdata.linhd.uned.es/ontology/postdata-core#Redaction"/>
        <rdfs:comment xml:lang="en">This property points to the text (an instance of Redaction) which was dedicated to the current Person.</rdfs:comment>
        <rdfs:isDefinedBy>http://postdata.linhd.uned.es/ontology/postdata-core/</rdfs:isDefinedBy>
        <rdfs:label xml:lang="en">has Dedication</rdfs:label>
    </owl:ObjectProperty>
    


    <!-- http://postdata.linhd.uned.es/ontology/postdata-core#hasFirstPart -->

    <owl:ObjectProperty rdf:about="http://postdata.linhd.uned.es/ontology/postdata-core#hasFirstPart">
        <rdfs:subPropertyOf rdf:resource="http://postdata.linhd.uned.es/ontology/postdata-core#hasPart"/>
        <rdfs:domain rdf:resource="http://postdata.linhd.uned.es/ontology/postdata-structuralElements#OrderedTextUnitList"/>
        <rdfs:comment xml:lang="en">This property points to the first text unit  which form the current element under analysis</rdfs:comment>
        <rdfs:isDefinedBy>http://postdata.linhd.uned.es/ontology/postdata-core/</rdfs:isDefinedBy>
        <rdfs:label xml:lang="en">has First Part</rdfs:label>
    </owl:ObjectProperty>
    


    <!-- http://postdata.linhd.uned.es/ontology/postdata-core#hasMember -->

    <owl:ObjectProperty rdf:about="http://postdata.linhd.uned.es/ontology/postdata-core#hasMember">
        <owl:inverseOf rdf:resource="http://postdata.linhd.uned.es/ontology/postdata-core#isMemberOf"/>
        <rdfs:domain rdf:resource="http://postdata.linhd.uned.es/ontology/postdata-core#Organisation"/>
        <rdfs:range rdf:resource="http://postdata.linhd.uned.es/ontology/postdata-core#Person"/>
        <rdfs:comment xml:lang="en">This property points to a Person that belongs to the Organisation</rdfs:comment>
        <rdfs:isDefinedBy>http://postdata.linhd.uned.es/ontology/postdata-core/</rdfs:isDefinedBy>
        <rdfs:label xml:lang="en">has Member</rdfs:label>
    </owl:ObjectProperty>
    


    <!-- http://postdata.linhd.uned.es/ontology/postdata-core#hasOrderedTextUnitList -->

    <owl:ObjectProperty rdf:about="http://postdata.linhd.uned.es/ontology/postdata-core#hasOrderedTextUnitList">
        <rdfs:domain rdf:resource="http://postdata.linhd.uned.es/ontology/postdata-core#Redaction"/>
        <rdfs:range rdf:resource="http://postdata.linhd.uned.es/ontology/postdata-structuralElements#OrderedTextUnitList"/>
        <rdfs:comment xml:lang="en">List of text units that form the Redaction</rdfs:comment>
        <rdfs:isDefinedBy>http://postdata.linhd.uned.es/ontology/postdata-core/</rdfs:isDefinedBy>
        <rdfs:label xml:lang="en">has Ordered Text Unit List</rdfs:label>
    </owl:ObjectProperty>
    


    <!-- http://postdata.linhd.uned.es/ontology/postdata-core#hasPart -->

    <owl:ObjectProperty rdf:about="http://postdata.linhd.uned.es/ontology/postdata-core#hasPart">
        <owl:inverseOf rdf:resource="http://postdata.linhd.uned.es/ontology/postdata-core#isPartOf"/>
        <rdfs:comment xml:lang="en">A property to state entities and their parts. It is the inverse of &apos;is Part Of&apos;.

This property emerges by reusing the part-of Ontology Design Pattern:
- http://www.ontologydesignpatterns.org/cp/owl/partof.owl</rdfs:comment>
        <rdfs:label xml:lang="en">has Part</rdfs:label>
    </owl:ObjectProperty>
    


    <!-- http://postdata.linhd.uned.es/ontology/postdata-core#hasProvenance -->

    <owl:ObjectProperty rdf:about="http://postdata.linhd.uned.es/ontology/postdata-core#hasProvenance">
        <owl:inverseOf rdf:resource="http://postdata.linhd.uned.es/ontology/postdata-core#isProvenanceFor"/>
        <rdfs:domain>
            <owl:Class>
                <owl:unionOf rdf:parseType="Collection">
                    <rdf:Description rdf:about="http://postdata.linhd.uned.es/ontology/postdata-core#Ensemble"/>
                    <rdf:Description rdf:about="http://postdata.linhd.uned.es/ontology/postdata-core#PoeticWork"/>
                </owl:unionOf>
            </owl:Class>
        </rdfs:domain>
        <rdfs:range rdf:resource="http://postdata.linhd.uned.es/ontology/postdata-core#Place"/>
        <rdfs:comment xml:lang="en">This property points to the Place which is the provenance of the current instance of Ensemble or Poetic Work</rdfs:comment>
        <rdfs:isDefinedBy>http://postdata.linhd.uned.es/ontology/postdata-core/</rdfs:isDefinedBy>
        <rdfs:label xml:lang="en">has Provenance</rdfs:label>
    </owl:ObjectProperty>
    


    <!-- http://postdata.linhd.uned.es/ontology/postdata-core#hasSynthesis -->

    <owl:ObjectProperty rdf:about="http://postdata.linhd.uned.es/ontology/postdata-core#hasSynthesis">
        <rdfs:subPropertyOf rdf:resource="http://iflastandards.info/ns/fr/frbr/frbroo/R2i"/>
        <owl:inverseOf rdf:resource="http://postdata.linhd.uned.es/ontology/postdata-core#isSynthesisOf"/>
        <rdfs:domain rdf:resource="http://postdata.linhd.uned.es/ontology/postdata-core#Redaction"/>
        <rdfs:range rdf:resource="http://postdata.linhd.uned.es/ontology/postdata-core#Redaction"/>
        <rdfs:comment xml:lang="en">This property points to one of the texts (an instance of Redaction) which is an analytical version of the text at hand (the current Redaction)</rdfs:comment>
        <rdfs:comment xml:lang="en">has Synthesis</rdfs:comment>
        <rdfs:isDefinedBy>http://postdata.linhd.uned.es/ontology/postdata-core/</rdfs:isDefinedBy>
    </owl:ObjectProperty>
    


    <!-- http://postdata.linhd.uned.es/ontology/postdata-core#hasTranslation -->

    <owl:ObjectProperty rdf:about="http://postdata.linhd.uned.es/ontology/postdata-core#hasTranslation">
        <owl:inverseOf rdf:resource="http://postdata.linhd.uned.es/ontology/postdata-core#isTranslationOf"/>
        <rdfs:domain rdf:resource="http://postdata.linhd.uned.es/ontology/postdata-core#Redaction"/>
        <rdfs:range rdf:resource="http://postdata.linhd.uned.es/ontology/postdata-core#Redaction"/>
        <rdfs:comment xml:lang="en">This property points to another work (an instance of Redaction) which is a translation of this one</rdfs:comment>
        <rdfs:comment xml:lang="en">This property points to the specific location in a bibliographic item (an instance of Location) which contains a translation of the text at hand</rdfs:comment>
        <rdfs:isDefinedBy>http://postdata.linhd.uned.es/ontology/postdata-core/</rdfs:isDefinedBy>
        <rdfs:label xml:lang="en">has Translation</rdfs:label>
    </owl:ObjectProperty>
    


    <!-- http://postdata.linhd.uned.es/ontology/postdata-core#hasWork -->

    <owl:ObjectProperty rdf:about="http://postdata.linhd.uned.es/ontology/postdata-core#hasWork">
        <rdfs:subPropertyOf rdf:resource="http://postdata.linhd.uned.es/ontology/postdata-core#hasPart"/>
        <owl:inverseOf rdf:resource="http://postdata.linhd.uned.es/ontology/postdata-core#workOf"/>
        <rdfs:domain rdf:resource="http://postdata.linhd.uned.es/ontology/postdata-core#Ensemble"/>
        <rdfs:range rdf:resource="http://postdata.linhd.uned.es/ontology/postdata-core#PoeticWork"/>
        <rdfs:comment xml:lang="en">This property points to the Works that are part of an Ensemble.</rdfs:comment>
        <rdfs:isDefinedBy>http://postdata.linhd.uned.es/ontology/postdata-core</rdfs:isDefinedBy>
        <rdfs:label xml:lang="en">has Work</rdfs:label>
    </owl:ObjectProperty>
    


    <!-- http://postdata.linhd.uned.es/ontology/postdata-core#involves -->

    <owl:ObjectProperty rdf:about="http://postdata.linhd.uned.es/ontology/postdata-core#involves">
        <owl:inverseOf rdf:resource="http://postdata.linhd.uned.es/ontology/postdata-core#isInvolvedIn"/>
        <rdfs:domain rdf:resource="http://postdata.linhd.uned.es/ontology/postdata-core#Event"/>
        <rdfs:range>
            <owl:Class>
                <owl:unionOf rdf:parseType="Collection">
                    <rdf:Description rdf:about="http://postdata.linhd.uned.es/ontology/postdata-core#Agent"/>
                    <rdf:Description rdf:about="http://postdata.linhd.uned.es/ontology/postdata-core#Place"/>
                </owl:unionOf>
            </owl:Class>
        </rdfs:range>
        <rdfs:comment xml:lang="en">This property points to an Organisation, Person or Place which are related to the current instance of Event</rdfs:comment>
        <rdfs:isDefinedBy>http://postdata.linhd.uned.es/ontology/postdata-core/</rdfs:isDefinedBy>
        <rdfs:label xml:lang="en">involves</rdfs:label>
    </owl:ObjectProperty>
    


    <!-- http://postdata.linhd.uned.es/ontology/postdata-core#isAgentOf -->

    <owl:ObjectProperty rdf:about="http://postdata.linhd.uned.es/ontology/postdata-core#isAgentOf">
        <rdfs:domain rdf:resource="http://postdata.linhd.uned.es/ontology/postdata-core#Agent"/>
        <rdfs:range rdf:resource="http://postdata.linhd.uned.es/ontology/postdata-core#AgentRole"/>
        <rdfs:comment xml:lang="en">This property relates an Agent with the Agent Role entity that describes a role for that Agent in the context of a Poetic Work, Redaction or Ensemble.

This property emerges by reusing the agent-role Ontology Design Pattern:
- http://www.ontologydesignpatterns.org/cp/owl/agentrole.owl
- http://www.ontologydesignpatterns.org/cp/owl/objectrole.owl</rdfs:comment>
        <rdfs:isDefinedBy>http://postdata.linhd.uned.es/ontology/postdata-core/</rdfs:isDefinedBy>
        <rdfs:label xml:lang="en">is Agent Of</rdfs:label>
    </owl:ObjectProperty>
    


    <!-- http://postdata.linhd.uned.es/ontology/postdata-core#isAgentRoleOf -->

    <owl:ObjectProperty rdf:about="http://postdata.linhd.uned.es/ontology/postdata-core#isAgentRoleOf">
        <rdfs:subPropertyOf rdf:resource="http://www.w3.org/2002/07/owl#topObjectProperty"/>
        <rdfs:domain rdf:resource="http://postdata.linhd.uned.es/ontology/postdata-core#AgentRole"/>
        <rdfs:range>
            <owl:Class>
                <owl:unionOf rdf:parseType="Collection">
                    <rdf:Description rdf:about="http://postdata.linhd.uned.es/ontology/postdata-core#Ensemble"/>
                    <rdf:Description rdf:about="http://postdata.linhd.uned.es/ontology/postdata-core#PoeticWork"/>
                    <rdf:Description rdf:about="http://postdata.linhd.uned.es/ontology/postdata-core#Redaction"/>
                </owl:unionOf>
            </owl:Class>
        </rdfs:range>
        <rdfs:comment xml:lang="en">This property points to the Ensemble, Redaction or Poetic Work on which the given Agent Role entity is applied.

This property emerges by reusing the agent-role Ontology Design Pattern:
- http://www.ontologydesignpatterns.org/cp/owl/agentrole.owl
- http://www.ontologydesignpatterns.org/cp/owl/objectrole.owl</rdfs:comment>
        <rdfs:isDefinedBy>http://postdata.linhd.uned.es/ontology/postdata-core/</rdfs:isDefinedBy>
        <rdfs:label xml:lang="en">Is Agent Role Of</rdfs:label>
    </owl:ObjectProperty>
    


    <!-- http://postdata.linhd.uned.es/ontology/postdata-core#isFrom -->

    <owl:ObjectProperty rdf:about="http://postdata.linhd.uned.es/ontology/postdata-core#isFrom">
        <rdfs:range rdf:resource="http://postdata.linhd.uned.es/ontology/postdata-core#Place"/>
        <rdfs:comment xml:lang="en">This property points to the Place which is the provenance of the item</rdfs:comment>
        <rdfs:isDefinedBy>http://postdata.linhd.uned.es/ontology/postdata-core/</rdfs:isDefinedBy>
        <rdfs:label xml:lang="en">is From</rdfs:label>
    </owl:ObjectProperty>
    


    <!-- http://postdata.linhd.uned.es/ontology/postdata-core#isIndexedIn -->

    <owl:ObjectProperty rdf:about="http://postdata.linhd.uned.es/ontology/postdata-core#isIndexedIn">
        <rdfs:domain rdf:resource="http://postdata.linhd.uned.es/ontology/postdata-core#Redaction"/>
        <rdfs:range rdf:resource="http://postdata.linhd.uned.es/ontology/postdata-transmission#Location"/>
        <rdfs:comment xml:lang="en">This property points to the specific location in the text of the bibliographic item (an instance of Location) in which the current text (Redaction) is indexed.</rdfs:comment>
        <rdfs:isDefinedBy>http://postdata.linhd.uned.es/ontology/postdata-core/</rdfs:isDefinedBy>
        <rdfs:label xml:lang="en">is Indexed In</rdfs:label>
    </owl:ObjectProperty>
    


    <!-- http://postdata.linhd.uned.es/ontology/postdata-core#isInvolvedIn -->

    <owl:ObjectProperty rdf:about="http://postdata.linhd.uned.es/ontology/postdata-core#isInvolvedIn">
        <rdfs:domain>
            <owl:Class>
                <owl:unionOf rdf:parseType="Collection">
                    <rdf:Description rdf:about="http://postdata.linhd.uned.es/ontology/postdata-core#Agent"/>
                    <rdf:Description rdf:about="http://postdata.linhd.uned.es/ontology/postdata-core#Place"/>
                </owl:unionOf>
            </owl:Class>
        </rdfs:domain>
        <rdfs:range rdf:resource="http://postdata.linhd.uned.es/ontology/postdata-core#Event"/>
        <rdfs:comment xml:lang="en">This property points to the Event in which the current instance of Organisation, Person or Place is referenced</rdfs:comment>
        <rdfs:isDefinedBy>http://postdata.linhd.uned.es/ontology/postdata-core/</rdfs:isDefinedBy>
        <rdfs:label xml:lang="en">is Involved In</rdfs:label>
    </owl:ObjectProperty>
    


    <!-- http://postdata.linhd.uned.es/ontology/postdata-core#isMemberOf -->

    <owl:ObjectProperty rdf:about="http://postdata.linhd.uned.es/ontology/postdata-core#isMemberOf">
        <rdfs:domain rdf:resource="http://postdata.linhd.uned.es/ontology/postdata-core#Person"/>
        <rdfs:range rdf:resource="http://postdata.linhd.uned.es/ontology/postdata-core#Organisation"/>
        <rdfs:comment xml:lang="en">This property points to the instance of Organisation to which the Person at hand belongs</rdfs:comment>
        <rdfs:isDefinedBy>http://postdata.linhd.uned.es/ontology/postdata-core/</rdfs:isDefinedBy>
        <rdfs:label xml:lang="en">is Member Of</rdfs:label>
    </owl:ObjectProperty>
    


    <!-- http://postdata.linhd.uned.es/ontology/postdata-core#isMentionedIn -->

    <owl:ObjectProperty rdf:about="http://postdata.linhd.uned.es/ontology/postdata-core#isMentionedIn">
        <owl:inverseOf rdf:resource="http://postdata.linhd.uned.es/ontology/postdata-core#mentions"/>
        <rdfs:range rdf:resource="http://postdata.linhd.uned.es/ontology/postdata-core#Redaction"/>
        <rdfs:comment xml:lang="en">This  property points to the text (an instance of Redaction) that records the current item (Event, Place, Organization or Person) under analysis</rdfs:comment>
        <rdfs:isDefinedBy>http://postdata.linhd.uned.es/ontology/postdata-core/</rdfs:isDefinedBy>
        <rdfs:label xml:lang="en">is Mentioned In</rdfs:label>
    </owl:ObjectProperty>
    


    <!-- http://postdata.linhd.uned.es/ontology/postdata-core#isPartOf -->

    <owl:ObjectProperty rdf:about="http://postdata.linhd.uned.es/ontology/postdata-core#isPartOf">
        <rdfs:comment xml:lang="en">A property to state entities and their parts.

This property arises by reusing the par-of Ontology Design Pattern:
- http://www.ontologydesignpatterns.org/cp/owl/partof.owl</rdfs:comment>
        <rdfs:label xml:lang="en">is Part Of</rdfs:label>
    </owl:ObjectProperty>
    


    <!-- http://postdata.linhd.uned.es/ontology/postdata-core#isProvenanceFor -->

    <owl:ObjectProperty rdf:about="http://postdata.linhd.uned.es/ontology/postdata-core#isProvenanceFor">
        <rdfs:domain rdf:resource="http://postdata.linhd.uned.es/ontology/postdata-core#Place"/>
        <rdfs:range>
            <owl:Class>
                <owl:unionOf rdf:parseType="Collection">
                    <rdf:Description rdf:about="http://postdata.linhd.uned.es/ontology/postdata-core#Ensemble"/>
                    <rdf:Description rdf:about="http://postdata.linhd.uned.es/ontology/postdata-core#PoeticWork"/>
                </owl:unionOf>
            </owl:Class>
        </rdfs:range>
        <rdfs:comment xml:lang="en">This property points to the Entity whose provenance corresponds to the current instance of Place</rdfs:comment>
        <rdfs:isDefinedBy>http://postdata.linhd.uned.es/ontology/postdata-core/</rdfs:isDefinedBy>
        <rdfs:label xml:lang="en">is Provenance For</rdfs:label>
    </owl:ObjectProperty>
    


    <!-- http://postdata.linhd.uned.es/ontology/postdata-core#isRealisedThrough -->

    <owl:ObjectProperty rdf:about="http://postdata.linhd.uned.es/ontology/postdata-core#isRealisedThrough">
        <rdfs:subPropertyOf rdf:resource="http://iflastandards.info/ns/fr/frbr/frbroo/R3"/>
        <owl:inverseOf rdf:resource="http://postdata.linhd.uned.es/ontology/postdata-core#realises"/>
        <rdfs:domain rdf:resource="http://postdata.linhd.uned.es/ontology/postdata-core#PoeticWork"/>
        <rdfs:range rdf:resource="http://postdata.linhd.uned.es/ontology/postdata-core#Redaction"/>
        <rdfs:comment xml:lang="en">This property points to a text (an instance of Redaction) which is one of the materialisations of the work under analysis</rdfs:comment>
        <rdfs:isDefinedBy>http://postdata.linhd.uned.es/ontology/postdata-core/</rdfs:isDefinedBy>
        <rdfs:label xml:lang="en">is Realised Through</rdfs:label>
    </owl:ObjectProperty>
    


    <!-- http://postdata.linhd.uned.es/ontology/postdata-core#isRecordedBy -->

    <owl:ObjectProperty rdf:about="http://postdata.linhd.uned.es/ontology/postdata-core#isRecordedBy">
        <rdfs:domain rdf:resource="http://postdata.linhd.uned.es/ontology/postdata-core#Event"/>
        <rdfs:range rdf:resource="http://postdata.linhd.uned.es/ontology/postdata-transmission#Location"/>
        <rdfs:comment xml:lang="en">This property points to the specific location in the text of the bibliographic item  (an instance of Location) that registers the current event</rdfs:comment>
        <rdfs:isDefinedBy>http://postdata.linhd.uned.es/ontology/postdata-core/</rdfs:isDefinedBy>
        <rdfs:label xml:lang="en">is Recorded By</rdfs:label>
    </owl:ObjectProperty>
    


    <!-- http://postdata.linhd.uned.es/ontology/postdata-core#isReferencedIn -->

    <owl:ObjectProperty rdf:about="http://postdata.linhd.uned.es/ontology/postdata-core#isReferencedIn">
        <rdfs:domain rdf:resource="http://postdata.linhd.uned.es/ontology/postdata-core#Person"/>
        <rdfs:range rdf:resource="http://postdata.linhd.uned.es/ontology/postdata-transmission#Location"/>
        <rdfs:comment xml:lang="en">This property points to the specific location in a bibliographic item (an instance of Location) whose contents are related to the current Person under analysis (usually, its specific bibliography)</rdfs:comment>
        <rdfs:isDefinedBy>http://postdata.linhd.uned.es/ontology/postdata-core/</rdfs:isDefinedBy>
        <rdfs:label xml:lang="en">is Referenced In</rdfs:label>
    </owl:ObjectProperty>
    


    <!-- http://postdata.linhd.uned.es/ontology/postdata-core#isSynthesisOf -->

    <owl:ObjectProperty rdf:about="http://postdata.linhd.uned.es/ontology/postdata-core#isSynthesisOf">
        <rdfs:subPropertyOf rdf:resource="http://iflastandards.info/ns/fr/frbr/frbroo/R2"/>
        <rdfs:domain rdf:resource="http://postdata.linhd.uned.es/ontology/postdata-core#Redaction"/>
        <rdfs:range rdf:resource="http://postdata.linhd.uned.es/ontology/postdata-core#Redaction"/>
        <rdfs:comment xml:lang="en">This property points to another text (an instance of Redaction) of which this version (Redaction) is a synthesis</rdfs:comment>
        <rdfs:isDefinedBy>http://postdata.linhd.uned.es/ontology/postdata-core/</rdfs:isDefinedBy>
        <rdfs:label xml:lang="en">is Synthesis Of</rdfs:label>
    </owl:ObjectProperty>
    


    <!-- http://postdata.linhd.uned.es/ontology/postdata-core#isTranslationOf -->

    <owl:ObjectProperty rdf:about="http://postdata.linhd.uned.es/ontology/postdata-core#isTranslationOf">
        <rdfs:domain rdf:resource="http://postdata.linhd.uned.es/ontology/postdata-core#Redaction"/>
        <rdfs:range rdf:resource="http://postdata.linhd.uned.es/ontology/postdata-core#Redaction"/>
        <rdfs:comment xml:lang="en">This property points to another version (an instance of Redaction) of which this one is a translation</rdfs:comment>
        <rdfs:isDefinedBy>http://postdata.linhd.uned.es/ontology/postdata-core/</rdfs:isDefinedBy>
        <rdfs:label xml:lang="en">is Translation Of</rdfs:label>
    </owl:ObjectProperty>
    


    <!-- http://postdata.linhd.uned.es/ontology/postdata-core#literaryPeriod -->

    <owl:ObjectProperty rdf:about="http://postdata.linhd.uned.es/ontology/postdata-core#literaryPeriod">
        <rdfs:domain rdf:resource="http://postdata.linhd.uned.es/ontology/postdata-core#Person"/>
        <rdfs:range rdf:resource="http://www.w3.org/2004/02/skos/core#Concept"/>
        <rdfs:range>
            <owl:Restriction>
                <owl:onProperty rdf:resource="http://www.w3.org/2004/02/skos/core#inScheme"/>
                <owl:hasValue rdf:resource="http://postdata.linhd.uned.es/kos/literary-period"/>
            </owl:Restriction>
        </rdfs:range>
        <rdfs:comment xml:lang="en">Label of a time frame for grouping certain works.
The values of this property are defined in a controlled vocabulary about literary periods.</rdfs:comment>
        <rdfs:isDefinedBy>http://postdata.linhd.uned.es/ontology/postdata-core/</rdfs:isDefinedBy>
        <rdfs:label xml:lang="en">literary Period</rdfs:label>
    </owl:ObjectProperty>
    


    <!-- http://postdata.linhd.uned.es/ontology/postdata-core#mentions -->

    <owl:ObjectProperty rdf:about="http://postdata.linhd.uned.es/ontology/postdata-core#mentions">
        <rdfs:domain rdf:resource="http://postdata.linhd.uned.es/ontology/postdata-core#Redaction"/>
        <rdfs:comment xml:lang="en">This property points to an instance of Event  or Person or Organisation or Place that is referred in a given Redaction</rdfs:comment>
        <rdfs:isDefinedBy>http://postdata.linhd.uned.es/ontology/postdata-core/</rdfs:isDefinedBy>
        <rdfs:label xml:lang="en">mentions</rdfs:label>
    </owl:ObjectProperty>
    


    <!-- http://postdata.linhd.uned.es/ontology/postdata-core#poeticType -->

    <owl:ObjectProperty rdf:about="http://postdata.linhd.uned.es/ontology/postdata-core#poeticType">
        <rdfs:domain rdf:resource="http://postdata.linhd.uned.es/ontology/postdata-core#PoeticWork"/>
        <rdfs:range rdf:resource="http://www.w3.org/2004/02/skos/core#Concept"/>
        <rdfs:range>
            <owl:Restriction>
                <owl:onProperty rdf:resource="http://www.w3.org/2004/02/skos/core#inScheme"/>
                <owl:hasValue rdf:resource="http://postdata.linhd.uned.es/kos/poetic-type"/>
            </owl:Restriction>
        </rdfs:range>
        <rdfs:comment xml:lang="en">Major literary genre of a Poetic Work, that is, drama or poetry. The values of this property are defined in a controlled vocabulary about poetic types</rdfs:comment>
        <rdfs:isDefinedBy>http://postdata.linhd.uned.es/ontology/postdata-core/</rdfs:isDefinedBy>
        <rdfs:label xml:lang="en">poetic Type</rdfs:label>
    </owl:ObjectProperty>
    


    <!-- http://postdata.linhd.uned.es/ontology/postdata-core#realises -->

    <owl:ObjectProperty rdf:about="http://postdata.linhd.uned.es/ontology/postdata-core#realises">
        <rdfs:subPropertyOf rdf:resource="http://iflastandards.info/ns/fr/frbr/frbroo/R3i"/>
        <rdfs:subPropertyOf rdf:resource="http://www.europeana.eu/schemas/edm/aggregatedCHO"/>
        <rdfs:domain rdf:resource="http://postdata.linhd.uned.es/ontology/postdata-core#Redaction"/>
        <rdfs:range rdf:resource="http://postdata.linhd.uned.es/ontology/postdata-core#PoeticWork"/>
        <rdfs:comment xml:lang="en">This property points to the work (an instance of Poetic Work) of which the text at hand (the current Redaction) is a materialisation.

This property is subproperty of edm:aggregatedCHO to keep alignments with Europeana Data Model.</rdfs:comment>
        <rdfs:isDefinedBy>http://postdata.linhd.uned.es/ontology/postdata-core/</rdfs:isDefinedBy>
        <rdfs:label xml:lang="en">realises</rdfs:label>
    </owl:ObjectProperty>
    


    <!-- http://postdata.linhd.uned.es/ontology/postdata-core#religiousAffiliation -->

    <owl:ObjectProperty rdf:about="http://postdata.linhd.uned.es/ontology/postdata-core#religiousAffiliation">
        <rdfs:domain rdf:resource="http://postdata.linhd.uned.es/ontology/postdata-core#Person"/>
        <rdfs:range rdf:resource="http://www.w3.org/2004/02/skos/core#Concept"/>
        <rdfs:range>
            <owl:Restriction>
                <owl:onProperty rdf:resource="http://www.w3.org/2004/02/skos/core#inScheme"/>
                <owl:hasValue rdf:resource="http://postdata.linhd.uned.es/kos/religious-affiliation"/>
            </owl:Restriction>
        </rdfs:range>
        <rdfs:comment xml:lang="en">Association of a Person with a religion, denomination or sub–denominational religious group. The values of this property are defined in a controlled vocabulary about religious affiliation</rdfs:comment>
        <rdfs:isDefinedBy>http://postdata.linhd.uned.es/ontology/postdata-core/</rdfs:isDefinedBy>
        <rdfs:label xml:lang="en">religious Affiliation</rdfs:label>
    </owl:ObjectProperty>
    


    <!-- http://postdata.linhd.uned.es/ontology/postdata-core#retrievesText -->

    <owl:ObjectProperty rdf:about="http://postdata.linhd.uned.es/ontology/postdata-core#retrievesText">
        <rdfs:domain rdf:resource="http://postdata.linhd.uned.es/ontology/postdata-core#Redaction"/>
        <rdfs:range rdf:resource="http://postdata.linhd.uned.es/ontology/postdata-transmission#Location"/>
        <rdfs:comment xml:lang="en">This property points to the specific location in a bibliographic item (an instance of Location) which contains the edition used as the base of the text (Redaction) at hand</rdfs:comment>
        <rdfs:isDefinedBy>http://postdata.linhd.uned.es/ontology/postdata-core/</rdfs:isDefinedBy>
        <rdfs:label xml:lang="en">retrieves Text</rdfs:label>
    </owl:ObjectProperty>
    


    <!-- http://postdata.linhd.uned.es/ontology/postdata-core#roleFunction -->

    <owl:ObjectProperty rdf:about="http://postdata.linhd.uned.es/ontology/postdata-core#roleFunction">
        <rdfs:domain rdf:resource="http://postdata.linhd.uned.es/ontology/postdata-core#AgentRole"/>
        <rdfs:range rdf:resource="http://www.w3.org/2004/02/skos/core#Concept"/>
        <rdfs:range>
            <owl:Restriction>
                <owl:onProperty rdf:resource="http://www.w3.org/2004/02/skos/core#inScheme"/>
                <owl:hasValue rdf:resource="http://postdata.linhd.uned.es/kos/role-function"/>
            </owl:Restriction>
        </rdfs:range>
        <rdfs:comment xml:lang="en">Specific function performed by some Agent on a Poetic Work (e.g. sponsor, actor, collector, singer, arranger, transcriptor). This is connected to the Agent Role class.</rdfs:comment>
        <rdfs:isDefinedBy>http://postdata.linhd.uned.es/ontology/postdata-core/</rdfs:isDefinedBy>
        <rdfs:label xml:lang="en">role Function</rdfs:label>
    </owl:ObjectProperty>
    


    <!-- http://postdata.linhd.uned.es/ontology/postdata-core#socialStatus -->

    <owl:ObjectProperty rdf:about="http://postdata.linhd.uned.es/ontology/postdata-core#socialStatus">
        <rdfs:domain rdf:resource="http://postdata.linhd.uned.es/ontology/postdata-core#Person"/>
        <rdfs:range rdf:resource="http://www.w3.org/2004/02/skos/core#Concept"/>
        <rdfs:range>
            <owl:Restriction>
                <owl:onProperty rdf:resource="http://www.w3.org/2004/02/skos/core#inScheme"/>
                <owl:hasValue rdf:resource="http://postdata.linhd.uned.es/kos/social-status"/>
            </owl:Restriction>
        </rdfs:range>
        <rdfs:comment xml:lang="en">The social status of the Person, that is the position or rank of a Person within the society. The values are specified in a controlled vocabulary</rdfs:comment>
        <rdfs:isDefinedBy>http://postdata.linhd.uned.es/ontology/postdata-core/</rdfs:isDefinedBy>
        <rdfs:label xml:lang="en">social Status</rdfs:label>
    </owl:ObjectProperty>
    


    <!-- http://postdata.linhd.uned.es/ontology/postdata-core#typeOfCharacter -->

    <owl:ObjectProperty rdf:about="http://postdata.linhd.uned.es/ontology/postdata-core#typeOfCharacter">
        <rdfs:domain rdf:resource="http://postdata.linhd.uned.es/ontology/postdata-core#AgentRole"/>
        <rdfs:range rdf:resource="http://www.w3.org/2004/02/skos/core#Concept"/>
        <rdfs:range>
            <owl:Restriction>
                <owl:onProperty rdf:resource="http://www.w3.org/2004/02/skos/core#inScheme"/>
                <owl:hasValue rdf:resource="http://postdata.linhd.uned.es/kos/character-type"/>
            </owl:Restriction>
        </rdfs:range>
        <rdfs:comment xml:lang="en">Type of character (eg. “main”, “antagonist”, etc.). The values are specified in a controlled vocabulary</rdfs:comment>
        <rdfs:isDefinedBy>http://postdata.linhd.uned.es/ontology/postdata-core/</rdfs:isDefinedBy>
        <rdfs:label xml:lang="en">type Of Character</rdfs:label>
    </owl:ObjectProperty>
    


    <!-- http://postdata.linhd.uned.es/ontology/postdata-core#typeOfDesignation -->

    <owl:ObjectProperty rdf:about="http://postdata.linhd.uned.es/ontology/postdata-core#typeOfDesignation">
        <rdfs:domain rdf:resource="http://postdata.linhd.uned.es/ontology/postdata-core#CreatorRole"/>
        <rdfs:range rdf:resource="http://www.w3.org/2004/02/skos/core#Concept"/>
        <rdfs:range>
            <owl:Restriction>
                <owl:onProperty rdf:resource="http://www.w3.org/2004/02/skos/core#inScheme"/>
                <owl:hasValue rdf:resource="http://postdata.linhd.uned.es/kos/designation-type"/>
            </owl:Restriction>
        </rdfs:range>
        <rdfs:comment xml:lang="en">Type of designation/name. E.g. pseudonym, heteronym, allonym, orthonym variant</rdfs:comment>
        <rdfs:isDefinedBy>http://postdata.linhd.uned.es/ontology/postdata-core/</rdfs:isDefinedBy>
        <rdfs:label xml:lang="en">type Of Designation</rdfs:label>
    </owl:ObjectProperty>
    


    <!-- http://postdata.linhd.uned.es/ontology/postdata-core#typeOfTextualElement -->

    <owl:ObjectProperty rdf:about="http://postdata.linhd.uned.es/ontology/postdata-core#typeOfTextualElement">
        <rdfs:domain rdf:resource="http://postdata.linhd.uned.es/ontology/postdata-core#Redaction"/>
        <rdfs:range rdf:resource="http://www.w3.org/2004/02/skos/core#Concept"/>
        <rdfs:range>
            <owl:Restriction>
                <owl:onProperty rdf:resource="http://www.w3.org/2004/02/skos/core#inScheme"/>
                <owl:hasValue rdf:resource="http://postdata.linhd.uned.es/kos/textual-element-type"/>
            </owl:Restriction>
        </rdfs:range>
        <rdfs:comment xml:lang="en">The type of textual element (e.g. part of a greater ensemble; part of a composed collection of poems; prologue of a work; epilogue of a work; a chapter of a work...)</rdfs:comment>
        <rdfs:isDefinedBy>http://postdata.linhd.uned.es/ontology/postdata-core/</rdfs:isDefinedBy>
        <rdfs:label xml:lang="en">type Of Textual Element</rdfs:label>
    </owl:ObjectProperty>
    


    <!-- http://postdata.linhd.uned.es/ontology/postdata-core#workOf -->

    <owl:ObjectProperty rdf:about="http://postdata.linhd.uned.es/ontology/postdata-core#workOf">
        <rdfs:subPropertyOf rdf:resource="http://postdata.linhd.uned.es/ontology/postdata-core#isPartOf"/>
        <rdfs:domain rdf:resource="http://postdata.linhd.uned.es/ontology/postdata-core#Ensemble"/>
        <rdfs:range rdf:resource="http://postdata.linhd.uned.es/ontology/postdata-core#PoeticWork"/>
        <rdfs:comment xml:lang="en">This property points to the Poetic Work for which a given work is part of.</rdfs:comment>
        <rdfs:isDefinedBy>http://postdata.linhd.uned.es/ontology/postdata-core</rdfs:isDefinedBy>
        <rdfs:label xml:lang="en">work Of</rdfs:label>
    </owl:ObjectProperty>
    


    <!-- http://purl.org/dc/terms/creator -->

    <owl:ObjectProperty rdf:about="http://purl.org/dc/terms/creator">
        <rdfs:comment xml:lang="en">Recommended practice is to identify the creator with a URI. If this is not possible or feasible, a literal value that identifies the creator may be provided.</rdfs:comment>
        <rdfs:label xml:lang="en">creator</rdfs:label>
        <skos:definition xml:lang="en">An entity responsible for making the resource.</skos:definition>
    </owl:ObjectProperty>
    


    <!-- http://www.europeana.eu/schemas/edm/aggregatedCHO -->

    <owl:ObjectProperty rdf:about="http://www.europeana.eu/schemas/edm/aggregatedCHO">
        <rdfs:domain rdf:resource="http://www.openarchives.org/ore/terms/Aggregation"/>
        <rdfs:range rdf:resource="http://www.europeana.eu/schemas/edm/ProvidedCHO"/>
        <rdfs:label xml:lang="en">Aggregated Cultural Heritage Object</rdfs:label>
        <skos:definition xml:lang="en">This property associates an ORE aggregation with the cultural heritage object(s) (CHO for short) it is about.</skos:definition>
    </owl:ObjectProperty>
    


    <!-- http://www.europeana.eu/schemas/edm/isShownBy -->

    <owl:ObjectProperty rdf:about="http://www.europeana.eu/schemas/edm/isShownBy">
        <rdfs:domain rdf:resource="http://www.openarchives.org/ore/terms/Aggregation"/>
        <rdfs:label xml:lang="en">Is Shown By</rdfs:label>
        <skos:definition xml:lang="en">An unambiguous URL reference to the digital object on the provider’s web site in the best available resolution/quality.</skos:definition>
    </owl:ObjectProperty>
    


    <!-- http://www.w3.org/2004/02/skos/core#broadMatch -->

    <owl:ObjectProperty rdf:about="http://www.w3.org/2004/02/skos/core#broadMatch">
        <rdfs:subPropertyOf rdf:resource="http://www.w3.org/2004/02/skos/core#broader"/>
        <rdfs:subPropertyOf rdf:resource="http://www.w3.org/2004/02/skos/core#mappingRelation"/>
        <owl:inverseOf rdf:resource="http://www.w3.org/2004/02/skos/core#narrowMatch"/>
        <rdfs:isDefinedBy rdf:resource="http://www.w3.org/2004/02/skos/core"/>
        <rdfs:label xml:lang="en">has broader match</rdfs:label>
        <skos:definition xml:lang="en">skos:broadMatch is used to state a hierarchical mapping link between two conceptual resources in different concept schemes.</skos:definition>
    </owl:ObjectProperty>
    


    <!-- http://www.w3.org/2004/02/skos/core#broader -->

    <owl:ObjectProperty rdf:about="http://www.w3.org/2004/02/skos/core#broader">
        <rdfs:subPropertyOf rdf:resource="http://www.w3.org/2004/02/skos/core#broaderTransitive"/>
        <owl:inverseOf rdf:resource="http://www.w3.org/2004/02/skos/core#narrower"/>
        <rdfs:comment xml:lang="en">Broader concepts are typically rendered as parents in a concept hierarchy (tree).</rdfs:comment>
        <rdfs:isDefinedBy rdf:resource="http://www.w3.org/2004/02/skos/core"/>
        <rdfs:label xml:lang="en">has broader</rdfs:label>
        <skos:definition xml:lang="en">Relates a concept to a concept that is more general in meaning.</skos:definition>
        <skos:scopeNote xml:lang="en">By convention, skos:broader is only used to assert an immediate (i.e. direct) hierarchical link between two conceptual resources.</skos:scopeNote>
    </owl:ObjectProperty>
    


    <!-- http://www.w3.org/2004/02/skos/core#broaderTransitive -->

    <owl:ObjectProperty rdf:about="http://www.w3.org/2004/02/skos/core#broaderTransitive">
        <rdfs:subPropertyOf rdf:resource="http://www.w3.org/2004/02/skos/core#semanticRelation"/>
        <owl:inverseOf rdf:resource="http://www.w3.org/2004/02/skos/core#narrowerTransitive"/>
        <rdf:type rdf:resource="http://www.w3.org/2002/07/owl#TransitiveProperty"/>
        <rdfs:isDefinedBy rdf:resource="http://www.w3.org/2004/02/skos/core"/>
        <rdfs:label xml:lang="en">has broader transitive</rdfs:label>
        <skos:definition>skos:broaderTransitive is a transitive superproperty of skos:broader.</skos:definition>
        <skos:scopeNote xml:lang="en">By convention, skos:broaderTransitive is not used to make assertions. Rather, the properties can be used to draw inferences about the transitive closure of the hierarchical relation, which is useful e.g. when implementing a simple query expansion algorithm in a search application.</skos:scopeNote>
    </owl:ObjectProperty>
    


    <!-- http://www.w3.org/2004/02/skos/core#closeMatch -->

    <owl:ObjectProperty rdf:about="http://www.w3.org/2004/02/skos/core#closeMatch">
        <rdfs:subPropertyOf rdf:resource="http://www.w3.org/2004/02/skos/core#mappingRelation"/>
        <rdf:type rdf:resource="http://www.w3.org/2002/07/owl#SymmetricProperty"/>
        <rdfs:isDefinedBy rdf:resource="http://www.w3.org/2004/02/skos/core"/>
        <rdfs:label xml:lang="en">has close match</rdfs:label>
        <skos:definition xml:lang="en">skos:closeMatch is used to link two concepts that are sufficiently similar that they can be used interchangeably in some information retrieval applications. In order to avoid the possibility of &quot;compound errors&quot; when combining mappings across more than two concept schemes, skos:closeMatch is not declared to be a transitive property.</skos:definition>
    </owl:ObjectProperty>
    


    <!-- http://www.w3.org/2004/02/skos/core#exactMatch -->

    <owl:ObjectProperty rdf:about="http://www.w3.org/2004/02/skos/core#exactMatch">
        <rdfs:subPropertyOf rdf:resource="http://www.w3.org/2004/02/skos/core#closeMatch"/>
        <rdf:type rdf:resource="http://www.w3.org/2002/07/owl#SymmetricProperty"/>
        <rdf:type rdf:resource="http://www.w3.org/2002/07/owl#TransitiveProperty"/>
        <rdfs:comment xml:lang="en">skos:exactMatch is disjoint with each of the properties skos:broadMatch and skos:relatedMatch.</rdfs:comment>
        <rdfs:isDefinedBy rdf:resource="http://www.w3.org/2004/02/skos/core"/>
        <rdfs:label xml:lang="en">has exact match</rdfs:label>
        <skos:definition xml:lang="en">skos:exactMatch is used to link two concepts, indicating a high degree of confidence that the concepts can be used interchangeably across a wide range of information retrieval applications. skos:exactMatch is a transitive property, and is a sub-property of skos:closeMatch.</skos:definition>
    </owl:ObjectProperty>
    


    <!-- http://www.w3.org/2004/02/skos/core#inScheme -->

    <owl:ObjectProperty rdf:about="http://www.w3.org/2004/02/skos/core#inScheme">
        <rdfs:range rdf:resource="http://www.w3.org/2004/02/skos/core#ConceptScheme"/>
        <rdfs:isDefinedBy rdf:resource="http://www.w3.org/2004/02/skos/core"/>
        <rdfs:label xml:lang="en">is in scheme</rdfs:label>
        <skos:definition xml:lang="en">Relates a resource (for example a concept) to a concept scheme in which it is included.</skos:definition>
        <skos:scopeNote xml:lang="en">A concept may be a member of more than one concept scheme.</skos:scopeNote>
    </owl:ObjectProperty>
    


    <!-- http://www.w3.org/2004/02/skos/core#mappingRelation -->

    <owl:ObjectProperty rdf:about="http://www.w3.org/2004/02/skos/core#mappingRelation">
        <rdfs:subPropertyOf rdf:resource="http://www.w3.org/2004/02/skos/core#semanticRelation"/>
        <rdfs:comment xml:lang="en">These concept mapping relations mirror semantic relations, and the data model defined below is similar (with the exception of skos:exactMatch) to the data model defined for semantic relations. A distinct vocabulary is provided for concept mapping relations, to provide a convenient way to differentiate links within a concept scheme from links between concept schemes. However, this pattern of usage is not a formal requirement of the SKOS data model, and relies on informal definitions of best practice.</rdfs:comment>
        <rdfs:isDefinedBy rdf:resource="http://www.w3.org/2004/02/skos/core"/>
        <rdfs:label xml:lang="en">is in mapping relation with</rdfs:label>
        <skos:definition xml:lang="en">Relates two concepts coming, by convention, from different schemes, and that have comparable meanings</skos:definition>
    </owl:ObjectProperty>
    


    <!-- http://www.w3.org/2004/02/skos/core#narrowMatch -->

    <owl:ObjectProperty rdf:about="http://www.w3.org/2004/02/skos/core#narrowMatch">
        <rdfs:subPropertyOf rdf:resource="http://www.w3.org/2004/02/skos/core#mappingRelation"/>
        <rdfs:subPropertyOf rdf:resource="http://www.w3.org/2004/02/skos/core#narrower"/>
        <rdfs:isDefinedBy rdf:resource="http://www.w3.org/2004/02/skos/core"/>
        <rdfs:label xml:lang="en">has narrower match</rdfs:label>
        <skos:definition xml:lang="en">skos:narrowMatch is used to state a hierarchical mapping link between two conceptual resources in different concept schemes.</skos:definition>
    </owl:ObjectProperty>
    


    <!-- http://www.w3.org/2004/02/skos/core#narrower -->

    <owl:ObjectProperty rdf:about="http://www.w3.org/2004/02/skos/core#narrower">
        <rdfs:subPropertyOf rdf:resource="http://www.w3.org/2004/02/skos/core#narrowerTransitive"/>
        <rdfs:comment xml:lang="en">Narrower concepts are typically rendered as children in a concept hierarchy (tree).</rdfs:comment>
        <rdfs:isDefinedBy rdf:resource="http://www.w3.org/2004/02/skos/core"/>
        <rdfs:label xml:lang="en">has narrower</rdfs:label>
        <skos:definition xml:lang="en">Relates a concept to a concept that is more specific in meaning.</skos:definition>
        <skos:scopeNote xml:lang="en">By convention, skos:broader is only used to assert an immediate (i.e. direct) hierarchical link between two conceptual resources.</skos:scopeNote>
    </owl:ObjectProperty>
    


    <!-- http://www.w3.org/2004/02/skos/core#narrowerTransitive -->

    <owl:ObjectProperty rdf:about="http://www.w3.org/2004/02/skos/core#narrowerTransitive">
        <rdfs:subPropertyOf rdf:resource="http://www.w3.org/2004/02/skos/core#semanticRelation"/>
        <rdf:type rdf:resource="http://www.w3.org/2002/07/owl#TransitiveProperty"/>
        <rdfs:isDefinedBy rdf:resource="http://www.w3.org/2004/02/skos/core"/>
        <rdfs:label xml:lang="en">has narrower transitive</rdfs:label>
        <skos:definition>skos:narrowerTransitive is a transitive superproperty of skos:narrower.</skos:definition>
        <skos:scopeNote xml:lang="en">By convention, skos:narrowerTransitive is not used to make assertions. Rather, the properties can be used to draw inferences about the transitive closure of the hierarchical relation, which is useful e.g. when implementing a simple query expansion algorithm in a search application.</skos:scopeNote>
    </owl:ObjectProperty>
    


    <!-- http://www.w3.org/2004/02/skos/core#related -->

    <owl:ObjectProperty rdf:about="http://www.w3.org/2004/02/skos/core#related">
        <rdfs:subPropertyOf rdf:resource="http://www.w3.org/2004/02/skos/core#semanticRelation"/>
        <rdf:type rdf:resource="http://www.w3.org/2002/07/owl#SymmetricProperty"/>
        <rdfs:comment xml:lang="en">skos:related is disjoint with skos:broaderTransitive</rdfs:comment>
        <rdfs:isDefinedBy rdf:resource="http://www.w3.org/2004/02/skos/core"/>
        <rdfs:label xml:lang="en">has related</rdfs:label>
        <skos:definition xml:lang="en">Relates a concept to a concept with which there is an associative semantic relationship.</skos:definition>
    </owl:ObjectProperty>
    


    <!-- http://www.w3.org/2004/02/skos/core#relatedMatch -->

    <owl:ObjectProperty rdf:about="http://www.w3.org/2004/02/skos/core#relatedMatch">
        <rdfs:subPropertyOf rdf:resource="http://www.w3.org/2004/02/skos/core#mappingRelation"/>
        <rdfs:subPropertyOf rdf:resource="http://www.w3.org/2004/02/skos/core#related"/>
        <rdf:type rdf:resource="http://www.w3.org/2002/07/owl#SymmetricProperty"/>
        <rdfs:isDefinedBy rdf:resource="http://www.w3.org/2004/02/skos/core"/>
        <rdfs:label xml:lang="en">has related match</rdfs:label>
        <skos:definition xml:lang="en">skos:relatedMatch is used to state an associative mapping link between two conceptual resources in different concept schemes.</skos:definition>
    </owl:ObjectProperty>
    


    <!-- http://www.w3.org/2004/02/skos/core#semanticRelation -->

    <owl:ObjectProperty rdf:about="http://www.w3.org/2004/02/skos/core#semanticRelation">
        <rdfs:domain rdf:resource="http://www.w3.org/2004/02/skos/core#Concept"/>
        <rdfs:range rdf:resource="http://www.w3.org/2004/02/skos/core#Concept"/>
        <rdfs:isDefinedBy rdf:resource="http://www.w3.org/2004/02/skos/core"/>
        <rdfs:label xml:lang="en">is in semantic relation with</rdfs:label>
        <skos:definition xml:lang="en">Links a concept to a concept related by meaning.</skos:definition>
        <skos:scopeNote xml:lang="en">This property should not be used directly, but as a super-property for all properties denoting a relationship of meaning between concepts.</skos:scopeNote>
    </owl:ObjectProperty>
    


    <!-- http://www.w3.org/2004/02/skos/core#topConceptOf -->

    <owl:ObjectProperty rdf:about="http://www.w3.org/2004/02/skos/core#topConceptOf">
        <rdfs:subPropertyOf rdf:resource="http://www.w3.org/2004/02/skos/core#inScheme"/>
        <rdfs:domain rdf:resource="http://www.w3.org/2004/02/skos/core#Concept"/>
        <rdfs:range rdf:resource="http://www.w3.org/2004/02/skos/core#ConceptScheme"/>
        <rdfs:isDefinedBy rdf:resource="http://www.w3.org/2004/02/skos/core"/>
        <rdfs:label xml:lang="en">is top concept in scheme</rdfs:label>
        <skos:definition xml:lang="en">Relates a concept to the concept scheme that it is a top level concept of.</skos:definition>
    </owl:ObjectProperty>
    


    <!-- 
    ///////////////////////////////////////////////////////////////////////////////////////
    //
    // Data properties
    //
    ///////////////////////////////////////////////////////////////////////////////////////
     -->

    


    <!-- http://postdata.linhd.uned.es/ontology/postdata-core#additionalName -->

    <owl:DatatypeProperty rdf:about="http://postdata.linhd.uned.es/ontology/postdata-core#additionalName">
        <rdfs:domain rdf:resource="http://postdata.linhd.uned.es/ontology/postdata-core#Person"/>
        <rdfs:range rdf:resource="http://www.w3.org/2001/XMLSchema#string"/>
        <rdfs:comment xml:lang="en">An additional name, such as a nickname, epithet, or alias, or any other descriptive phrase used within a personal name.

Taking as example the writer Charlotte Brontë, an &quot;additionalName&quot; would be her alias: &quot;Currell Bell&quot;.</rdfs:comment>
        <rdfs:isDefinedBy>http://postdata.linhd.uned.es/ontology/postdata-core/</rdfs:isDefinedBy>
        <rdfs:label xml:lang="en">additional Name</rdfs:label>
    </owl:DatatypeProperty>
    


    <!-- http://postdata.linhd.uned.es/ontology/postdata-core#address -->

    <owl:DatatypeProperty rdf:about="http://postdata.linhd.uned.es/ontology/postdata-core#address">
        <rdfs:domain rdf:resource="http://postdata.linhd.uned.es/ontology/postdata-core#Organisation"/>
        <rdfs:range rdf:resource="http://www.w3.org/2001/XMLSchema#string"/>
        <rdfs:comment xml:lang="en">Contains a postal address for an organisation. There can only be one address per Organization.

Taking as example Cervantes&apos; poem &quot;Amadís de Gaula a Don Quijote de la Mancha&quot;, TEI-annotated in the ADSO corpus, the publisher would be &quot;Natural Language Processing Group. Department of Software and Computing Systems. University of Alicante (Spain)&quot;, and its address would be &quot;carretera San Vicente s/n 03690 San Vicente del Raspeig, Alicante (Spain)&quot;.</rdfs:comment>
        <rdfs:isDefinedBy>http://postdata.linhd.uned.es/ontology/postdata-core/</rdfs:isDefinedBy>
        <rdfs:label xml:lang="en">address</rdfs:label>
    </owl:DatatypeProperty>
    


    <!-- http://postdata.linhd.uned.es/ontology/postdata-core#alternativeName -->

    <owl:DatatypeProperty rdf:about="http://postdata.linhd.uned.es/ontology/postdata-core#alternativeName">
        <rdfs:domain rdf:resource="http://postdata.linhd.uned.es/ontology/postdata-core#Person"/>
        <rdfs:range rdf:resource="http://www.w3.org/2001/XMLSchema#string"/>
        <rdfs:comment xml:lang="en">Alternative name that references the current Person. A person may have zero or several alternative names.

Taking as example the character &quot;Aldonza Lorenzo&quot; from the Quixote, an &quot;alternativeName&quot; could be &quot;Dulcinea&quot;.</rdfs:comment>
        <rdfs:isDefinedBy>http://postdata.linhd.uned.es/ontology/postdata-core/</rdfs:isDefinedBy>
        <rdfs:label xml:lang="en">alternative Name</rdfs:label>
    </owl:DatatypeProperty>
    


    <!-- http://postdata.linhd.uned.es/ontology/postdata-core#alternativeTitle -->

    <owl:DatatypeProperty rdf:about="http://postdata.linhd.uned.es/ontology/postdata-core#alternativeTitle">
        <rdfs:domain>
            <owl:Class>
                <owl:unionOf rdf:parseType="Collection">
                    <rdf:Description rdf:about="http://postdata.linhd.uned.es/ontology/postdata-core#PoeticWork"/>
                    <rdf:Description rdf:about="http://postdata.linhd.uned.es/ontology/postdata-core#Redaction"/>
                </owl:unionOf>
            </owl:Class>
        </rdfs:domain>
        <rdfs:range rdf:resource="http://www.w3.org/2001/XMLSchema#string"/>
        <rdfs:comment xml:lang="en">Other known denominations of a Poetic Work or a Redaction.

Taking as example the &quot;Poema de Mio Cid&quot;, an &quot;alternativeTitle&quot; would be &quot;Cantar de Mio Cid&quot;.</rdfs:comment>
        <rdfs:isDefinedBy>http://postdata.linhd.uned.es/ontology/postdata-core/</rdfs:isDefinedBy>
        <rdfs:label xml:lang="en">alternative Title</rdfs:label>
    </owl:DatatypeProperty>
    


    <!-- http://postdata.linhd.uned.es/ontology/postdata-core#audience -->

    <owl:DatatypeProperty rdf:about="http://postdata.linhd.uned.es/ontology/postdata-core#audience">
        <rdfs:domain rdf:resource="http://postdata.linhd.uned.es/ontology/postdata-core#Redaction"/>
        <rdfs:range rdf:resource="http://www.w3.org/2001/XMLSchema#string"/>
        <rdfs:comment xml:lang="en">The meant readership, viewers or listeners of a Redaction. There is at most one possible value for audience.

Taking as example the play &quot;La segunda Celestina&quot;, &quot;audience&quot; would be the Spanish Queen and the people in the court attending the Queen&apos;s birthday celebrations.</rdfs:comment>
        <rdfs:isDefinedBy>http://postdata.linhd.uned.es/ontology/postdata-core/</rdfs:isDefinedBy>
        <rdfs:label xml:lang="en">audience</rdfs:label>
    </owl:DatatypeProperty>
    


    <!-- http://postdata.linhd.uned.es/ontology/postdata-core#biography -->

    <owl:DatatypeProperty rdf:about="http://postdata.linhd.uned.es/ontology/postdata-core#biography">
        <rdfs:domain rdf:resource="http://postdata.linhd.uned.es/ontology/postdata-core#Person"/>
        <rdfs:range rdf:resource="http://www.w3.org/2001/XMLSchema#string"/>
        <rdfs:comment xml:lang="en">An account of a Person&apos;s life written, composed, or produced by another.

Taking as example the poet Antonio Machado, &quot;biography&quot; could be: &quot;Antonio Cipriano José María y Francisco de Santa Ana Machado y Ruiz (26 July 1875 – 22 February 1939), known as Antonio Machado, was a Spanish poet and one of the leading figures of the Spanish literary movement known as the Generation of &apos;98. His work, initially modernist, evolved towards an intimate form of symbolism with romantic traits. He gradually developed a style characterised by both an engagement with humanity on one side and an almost Taoist contemplation of existence on the other, a synthesis that according to Machado echoed the most ancient popular wisdom. In Gerardo Diego&apos;s words, Machado &quot;spoke in verse and lived in poetry.&quot;&quot; (example extracted from Wikipedia).</rdfs:comment>
        <rdfs:isDefinedBy>http://postdata.linhd.uned.es/ontology/postdata-core/</rdfs:isDefinedBy>
        <rdfs:label xml:lang="en">biography</rdfs:label>
    </owl:DatatypeProperty>
    


    <!-- http://postdata.linhd.uned.es/ontology/postdata-core#commentary -->

    <owl:DatatypeProperty rdf:about="http://postdata.linhd.uned.es/ontology/postdata-core#commentary">
        <rdfs:domain>
            <owl:Class>
                <owl:unionOf rdf:parseType="Collection">
                    <rdf:Description rdf:about="http://postdata.linhd.uned.es/ontology/postdata-core#PoeticWork"/>
                    <rdf:Description rdf:about="http://postdata.linhd.uned.es/ontology/postdata-core#Redaction"/>
                </owl:unionOf>
            </owl:Class>
        </rdfs:domain>
        <rdfs:range rdf:resource="http://www.w3.org/2001/XMLSchema#string"/>
        <rdfs:comment xml:lang="en">An explanatory series of notes or comments; an explanatory essay or treatise on a Poetic Work or Redaction.

Taking the Poetic Work example &quot;Versos&quot; by Fernando de Herrera, the comments Francisco de Quevedo wrote on his own edition along the text of the poems would form the &quot;commentary&quot;.</rdfs:comment>
        <rdfs:isDefinedBy>http://postdata.linhd.uned.es/ontology/postdata-core/</rdfs:isDefinedBy>
        <rdfs:label xml:lang="en">commentary</rdfs:label>
    </owl:DatatypeProperty>
    


    <!-- http://postdata.linhd.uned.es/ontology/postdata-core#ethnicity -->

    <owl:DatatypeProperty rdf:about="http://postdata.linhd.uned.es/ontology/postdata-core#ethnicity">
        <rdfs:domain rdf:resource="http://postdata.linhd.uned.es/ontology/postdata-core#Person"/>
        <rdfs:range rdf:resource="http://www.w3.org/2001/XMLSchema#string"/>
        <rdfs:comment xml:lang="en">An ethnic group; a social group that shares a common and distinctive culture, religion, language, or the like.

Taking as Person example the poet &quot;Antonio Enríquez Gómez&quot;, his &quot;ethnicity&quot; would be &quot;crypto-Jewish&quot;.</rdfs:comment>
        <rdfs:isDefinedBy>http://postdata.linhd.uned.es/ontology/postdata-core/</rdfs:isDefinedBy>
        <rdfs:label>ethnicity</rdfs:label>
    </owl:DatatypeProperty>
    


    <!-- http://postdata.linhd.uned.es/ontology/postdata-core#eventNarration -->

    <owl:DatatypeProperty rdf:about="http://postdata.linhd.uned.es/ontology/postdata-core#eventNarration">
        <rdfs:domain rdf:resource="http://postdata.linhd.uned.es/ontology/postdata-core#Event"/>
        <rdfs:range rdf:resource="http://www.w3.org/2001/XMLSchema#string"/>
        <rdfs:comment xml:lang="en">Text that narrates an Event, that is, an excerpt of the Redaction. There is at most one possible description for this property.

Taking the Poetic Work example the &quot;Poema de Mio Cid&quot;, and the Event example the Cid&apos;s arrival to Burgos, we find an &quot;eventNarration&quot; in  lines 1-64, starting with &quot;De los sos ojos tan fuertemientre llorando&quot;.</rdfs:comment>
        <rdfs:isDefinedBy>http://postdata.linhd.uned.es/ontology/postdata-core/</rdfs:isDefinedBy>
        <rdfs:label xml:lang="en">event Narration</rdfs:label>
    </owl:DatatypeProperty>
    


    <!-- http://postdata.linhd.uned.es/ontology/postdata-core#explicit -->

    <owl:DatatypeProperty rdf:about="http://postdata.linhd.uned.es/ontology/postdata-core#explicit">
        <rdfs:domain rdf:resource="http://postdata.linhd.uned.es/ontology/postdata-core#Redaction"/>
        <rdfs:range rdf:resource="http://www.w3.org/2001/XMLSchema#string"/>
        <rdfs:comment xml:lang="en">The closing words of the Redaction (usually, the last verse). There is only one explicit per Redaction.

Taking as example the poem &quot;Canary&quot; by Rita Dove, the last verse, &quot;If you can&apos;t be free, be a mystery&quot;, would be the &quot;explicit&quot;.</rdfs:comment>
        <rdfs:isDefinedBy>http://postdata.linhd.uned.es/ontology/postdata-core/</rdfs:isDefinedBy>
        <rdfs:label xml:lang="en">explicit</rdfs:label>
    </owl:DatatypeProperty>
    


    <!-- http://postdata.linhd.uned.es/ontology/postdata-core#forename -->

    <owl:DatatypeProperty rdf:about="http://postdata.linhd.uned.es/ontology/postdata-core#forename">
        <rdfs:domain rdf:resource="http://postdata.linhd.uned.es/ontology/postdata-core#Person"/>
        <rdfs:range rdf:resource="http://www.w3.org/2001/XMLSchema#string"/>
        <rdfs:comment xml:lang="en">It contains a forename, given or baptismal name.

Taking as example the poet &quot;Antonio Machado&quot;, his &quot;forename&quot; would be &quot;Antonio&quot;.</rdfs:comment>
        <rdfs:isDefinedBy>http://postdata.linhd.uned.es/ontology/postdata-core/</rdfs:isDefinedBy>
        <rdfs:label xml:lang="en">forename</rdfs:label>
    </owl:DatatypeProperty>
    


    <!-- http://postdata.linhd.uned.es/ontology/postdata-core#function -->

    <owl:DatatypeProperty rdf:about="http://postdata.linhd.uned.es/ontology/postdata-core#function">
        <rdfs:subPropertyOf rdf:resource="http://www.w3.org/2002/07/owl#topDataProperty"/>
        <rdfs:domain>
            <owl:Class>
                <owl:unionOf rdf:parseType="Collection">
                    <rdf:Description rdf:about="http://postdata.linhd.uned.es/ontology/postdata-core#PoeticWork"/>
                    <rdf:Description rdf:about="http://postdata.linhd.uned.es/ontology/postdata-core#Redaction"/>
                </owl:unionOf>
            </owl:Class>
        </rdfs:domain>
        <rdfs:range rdf:resource="http://www.w3.org/2001/XMLSchema#string"/>
        <rdfs:comment xml:lang="en">Purpose of the Poetic Work or Redaction (e.g. prayer, spell, curse). A Poetic Work or Redaction may have several functions associated.

Taking as example the poem &quot;Cantico delle creature&quot; by San Francesco d’Assisi, &quot;function&quot; would be &quot;prayer&quot;.</rdfs:comment>
        <rdfs:isDefinedBy>http://postdata.linhd.uned.es/ontology/postdata-core/</rdfs:isDefinedBy>
        <rdfs:label xml:lang="en">function</rdfs:label>
    </owl:DatatypeProperty>
    


    <!-- http://postdata.linhd.uned.es/ontology/postdata-core#genName -->

    <owl:DatatypeProperty rdf:about="http://postdata.linhd.uned.es/ontology/postdata-core#genName">
        <rdfs:domain rdf:resource="http://postdata.linhd.uned.es/ontology/postdata-core#Person"/>
        <rdfs:range rdf:resource="http://www.w3.org/2001/XMLSchema#string"/>
        <rdfs:comment xml:lang="en">It contains a name component used to distinguish otherwise similar names on the basis of the relative age or generation of the Person named.

Taking as example the person &quot;Felipe II&quot;, &quot;genName&quot; is &quot;II&quot;.</rdfs:comment>
        <rdfs:isDefinedBy>http://postdata.linhd.uned.es/ontology/postdata-core/</rdfs:isDefinedBy>
        <rdfs:label xml:lang="en">genName</rdfs:label>
    </owl:DatatypeProperty>
    


    <!-- http://postdata.linhd.uned.es/ontology/postdata-core#incipit -->

    <owl:DatatypeProperty rdf:about="http://postdata.linhd.uned.es/ontology/postdata-core#incipit">
        <rdfs:domain rdf:resource="http://postdata.linhd.uned.es/ontology/postdata-core#Redaction"/>
        <rdfs:range rdf:resource="http://www.w3.org/2001/XMLSchema#string"/>
        <rdfs:comment xml:lang="en">The first line of a Redaction. There is one incipit for each Redaction.

Taking as example the &quot;Soledades&quot; by Góngora, the &quot;incipit&quot; is &quot;Pasos de un peregrino son errante&quot;.</rdfs:comment>
        <rdfs:isDefinedBy>http://postdata.linhd.uned.es/ontology/postdata-core/</rdfs:isDefinedBy>
        <rdfs:label xml:lang="en">incipit</rdfs:label>
    </owl:DatatypeProperty>
    


    <!-- http://postdata.linhd.uned.es/ontology/postdata-core#isAnonymous -->

    <owl:DatatypeProperty rdf:about="http://postdata.linhd.uned.es/ontology/postdata-core#isAnonymous">
        <rdfs:domain rdf:resource="http://postdata.linhd.uned.es/ontology/postdata-core#CreatorRole"/>
        <rdfs:range rdf:resource="http://www.w3.org/2001/XMLSchema#boolean"/>
        <rdfs:comment xml:lang="en">This value indicates if an Agent Role entity does not have an associated Agent playing the role of Creator.

Taking as example the creator of &quot;Libro de Alexandre&quot;, &quot;isAnonymous&quot; is True because the author is unknown to this day.</rdfs:comment>
        <rdfs:isDefinedBy>http://postdata.linhd.uned.es/ontology/postdata-core/</rdfs:isDefinedBy>
        <rdfs:label xml:lang="en">is Anonymous</rdfs:label>
    </owl:DatatypeProperty>
    


    <!-- http://postdata.linhd.uned.es/ontology/postdata-core#isCalligram -->

    <owl:DatatypeProperty rdf:about="http://postdata.linhd.uned.es/ontology/postdata-core#isCalligram">
        <rdfs:domain rdf:resource="http://postdata.linhd.uned.es/ontology/postdata-core#PoeticWork"/>
        <rdfs:range rdf:resource="http://www.w3.org/2001/XMLSchema#boolean"/>
        <rdfs:comment xml:lang="en">Whether a Poetic Work is a calligram or not. That is, a text visually arranged in a way that it forms an image associated with the text contents.

Taking as example the (calligram) poem &quot;La Colombe poignardée et le Jet d’eau&quot; by Apollinaire, &quot;is Calligram&quot; value is True.</rdfs:comment>
        <rdfs:isDefinedBy>http://postdata.linhd.uned.es/ontology/postdata-core/</rdfs:isDefinedBy>
        <rdfs:label xml:lang="en">is Calligram</rdfs:label>
    </owl:DatatypeProperty>
    


    <!-- http://postdata.linhd.uned.es/ontology/postdata-core#isFictional -->

    <owl:DatatypeProperty rdf:about="http://postdata.linhd.uned.es/ontology/postdata-core#isFictional">
        <rdfs:subPropertyOf rdf:resource="http://www.w3.org/2002/07/owl#topDataProperty"/>
        <rdfs:domain rdf:resource="http://postdata.linhd.uned.es/ontology/postdata-core#Person"/>
        <rdfs:range rdf:resource="http://www.w3.org/2001/XMLSchema#boolean"/>
        <rdfs:comment xml:lang="en">Whether a given Person is a fictional character.

Taking as example the character &quot;Don Quijote de la Mancha&quot;, this will have a True value for &quot;is Fictional&quot; property.</rdfs:comment>
        <rdfs:isDefinedBy>http://postdata.linhd.uned.es/ontology/postdata-core/</rdfs:isDefinedBy>
        <rdfs:label xml:lang="en">is Fictional</rdfs:label>
    </owl:DatatypeProperty>
    


    <!-- http://postdata.linhd.uned.es/ontology/postdata-core#isSong -->

    <owl:DatatypeProperty rdf:about="http://postdata.linhd.uned.es/ontology/postdata-core#isSong">
        <rdfs:domain>
            <owl:Class>
                <owl:unionOf rdf:parseType="Collection">
                    <rdf:Description rdf:about="http://postdata.linhd.uned.es/ontology/postdata-core#PoeticWork"/>
                    <rdf:Description rdf:about="http://postdata.linhd.uned.es/ontology/postdata-core#Redaction"/>
                </owl:unionOf>
            </owl:Class>
        </rdfs:domain>
        <rdfs:range rdf:resource="http://www.w3.org/2001/XMLSchema#boolean"/>
        <rdfs:comment xml:lang="en">Whether the Poetic Work or Redaction where composed to be sung.

Taking as example the poetic work &quot;Chanson de Roland&quot;, &quot;is Song&quot; is True because the work is part of a genre which was sang.</rdfs:comment>
        <rdfs:isDefinedBy>http://postdata.linhd.uned.es/ontology/postdata-core/</rdfs:isDefinedBy>
        <rdfs:label xml:lang="en">is Song</rdfs:label>
    </owl:DatatypeProperty>
    


    <!-- http://postdata.linhd.uned.es/ontology/postdata-core#isWrongAttribution -->

    <owl:DatatypeProperty rdf:about="http://postdata.linhd.uned.es/ontology/postdata-core#isWrongAttribution">
        <rdfs:domain rdf:resource="http://postdata.linhd.uned.es/ontology/postdata-core#CreatorRole"/>
        <rdfs:range rdf:resource="http://www.w3.org/2001/XMLSchema#boolean"/>
        <rdfs:comment xml:lang="en">In case the attribution of a Creator Role to a given Agent Role entity of is certainly wrong. This is applied to the Agent Role associated to a Redaction.

Taking as example the poem &quot;Muere lentamente&quot; (by Martha Madeiros) which is erroneously attributed to Pablo Neruda, in the case Neruda is indicated as the author, &quot;is Wrong Attribution&quot; would be True.</rdfs:comment>
        <rdfs:isDefinedBy>http://postdata.linhd.uned.es/ontology/postdata-core/</rdfs:isDefinedBy>
        <rdfs:label xml:lang="en">is Wrong Attribution</rdfs:label>
    </owl:DatatypeProperty>
    


    <!-- http://postdata.linhd.uned.es/ontology/postdata-core#keyword -->

    <owl:DatatypeProperty rdf:about="http://postdata.linhd.uned.es/ontology/postdata-core#keyword">
        <rdfs:domain>
            <owl:Class>
                <owl:unionOf rdf:parseType="Collection">
                    <rdf:Description rdf:about="http://postdata.linhd.uned.es/ontology/postdata-core#PoeticWork"/>
                    <rdf:Description rdf:about="http://postdata.linhd.uned.es/ontology/postdata-core#Redaction"/>
                </owl:unionOf>
            </owl:Class>
        </rdfs:domain>
        <rdfs:range rdf:resource="http://www.w3.org/2001/XMLSchema#string"/>
        <rdfs:comment xml:lang="en">A significant or descriptive word that describes the general ideas or concepts expressed in a Poetic Work or Redaction.

Taking as example the theatre play &quot;Othello&quot; by Shakespeare, one possible &quot;keyword&quot; is &quot;jealousy&quot;.</rdfs:comment>
        <rdfs:isDefinedBy>http://postdata.linhd.uned.es/ontology/postdata-core/</rdfs:isDefinedBy>
        <rdfs:label xml:lang="en">keyword</rdfs:label>
    </owl:DatatypeProperty>
    


    <!-- http://postdata.linhd.uned.es/ontology/postdata-core#language -->

    <owl:DatatypeProperty rdf:about="http://postdata.linhd.uned.es/ontology/postdata-core#language">
        <rdfs:domain>
            <owl:Class>
                <owl:unionOf rdf:parseType="Collection">
                    <rdf:Description rdf:about="http://postdata.linhd.uned.es/ontology/postdata-core#PoeticWork"/>
                    <rdf:Description rdf:about="http://postdata.linhd.uned.es/ontology/postdata-core#Redaction"/>
                </owl:unionOf>
            </owl:Class>
        </rdfs:domain>
        <rdfs:range>
            <rdfs:Datatype>
                <owl:unionOf rdf:parseType="Collection">
                    <rdf:Description rdf:about="http://www.w3.org/2001/XMLSchema#language"/>
                    <rdf:Description rdf:about="http://www.w3.org/2001/XMLSchema#string"/>
                </owl:unionOf>
            </rdfs:Datatype>
        </rdfs:range>
        <rdfs:comment xml:lang="en">Language of the text. There might be several languages used in a Poetic Work or Redaction.

For example the &quot;language&quot; of &quot;Romancero gitano&quot; by Lorca, is &quot;Spanish&quot; (xsd:string). It could also be represented with the associated langauge code &quot;es&quot; (xsd:language)</rdfs:comment>
        <rdfs:isDefinedBy>http://postdata.linhd.uned.es/ontology/postdata-core/</rdfs:isDefinedBy>
        <rdfs:label xml:lang="en">language</rdfs:label>
    </owl:DatatypeProperty>
    


    <!-- http://postdata.linhd.uned.es/ontology/postdata-core#layout -->

    <owl:DatatypeProperty rdf:about="http://postdata.linhd.uned.es/ontology/postdata-core#layout">
        <rdfs:domain rdf:resource="http://postdata.linhd.uned.es/ontology/postdata-core#Redaction"/>
        <rdfs:range rdf:resource="http://www.w3.org/2001/XMLSchema#string"/>
        <rdfs:comment xml:lang="en">The arrangement of textual materials (images included) on a page of a Redaction.

Taking as example &quot;The Waste Land and Other Poems&quot; by T.S. Eliot, edition by Broadview press, printed in 2011, the &quot;layout&quot; can be described in the following way: &quot;the text is left aligned, written in one column. Each stanza is followed by a blank space dividing it from the following stanza. The number of lines is displayed by a number marking every five lines which is aligned to the right edge of the page. Every page contains on average 30-40 lines&quot;.</rdfs:comment>
        <rdfs:isDefinedBy>http://postdata.linhd.uned.es/ontology/postdata-core/</rdfs:isDefinedBy>
        <rdfs:label xml:lang="en">layout</rdfs:label>
    </owl:DatatypeProperty>
    


    <!-- http://postdata.linhd.uned.es/ontology/postdata-core#literaryTradition -->

    <owl:DatatypeProperty rdf:about="http://postdata.linhd.uned.es/ontology/postdata-core#literaryTradition">
        <rdfs:domain rdf:resource="http://postdata.linhd.uned.es/ontology/postdata-core#PoeticWork"/>
        <rdfs:range rdf:resource="http://www.w3.org/2001/XMLSchema#string"/>
        <rdfs:comment xml:lang="en">The literary tradition assigned to a Poetic Work. There might be several values for this property.

Taking as example the theatre play &quot;La vida es sueño&quot; by Calderón de la Barca, &quot;literary Tradition&quot; is &quot;Baroque&quot;.</rdfs:comment>
        <rdfs:isDefinedBy>http://postdata.linhd.uned.es/ontology/postdata-core/</rdfs:isDefinedBy>
        <rdfs:label xml:lang="en">literary Tradition</rdfs:label>
    </owl:DatatypeProperty>
    


    <!-- http://postdata.linhd.uned.es/ontology/postdata-core#name -->

    <owl:DatatypeProperty rdf:about="http://postdata.linhd.uned.es/ontology/postdata-core#name">
        <rdfs:domain rdf:resource="http://postdata.linhd.uned.es/ontology/postdata-core#Person"/>
        <rdfs:range rdf:resource="http://www.w3.org/2001/XMLSchema#string"/>
        <rdfs:comment xml:lang="en">Contains a proper noun or noun phrase that refers the current Person.

Taking as example the full name of Federico García Lorca, &quot;name&quot; would be &quot;Federico del Sagrado Corazón de Jesús García Lorca&quot;.</rdfs:comment>
        <rdfs:isDefinedBy>http://postdata.linhd.uned.es/ontology/postdata-core/</rdfs:isDefinedBy>
        <rdfs:label xml:lang="en">name</rdfs:label>
    </owl:DatatypeProperty>
    


    <!-- http://postdata.linhd.uned.es/ontology/postdata-core#nameLink -->

    <owl:DatatypeProperty rdf:about="http://postdata.linhd.uned.es/ontology/postdata-core#nameLink">
        <rdfs:subPropertyOf rdf:resource="http://www.w3.org/2002/07/owl#topDataProperty"/>
        <rdfs:domain rdf:resource="http://postdata.linhd.uned.es/ontology/postdata-core#Person"/>
        <rdfs:range rdf:resource="http://www.w3.org/2001/XMLSchema#string"/>
        <rdfs:comment xml:lang="en">A connecting phrase or link used within a name of a Person but not regarded as part of it.

Taking as example the writer “Hildegard von Bingen”, her “nameLink” would be “von”.</rdfs:comment>
        <rdfs:isDefinedBy>http://postdata.linhd.uned.es/ontology/postdata-core/</rdfs:isDefinedBy>
        <rdfs:label xml:lang="en">name Link</rdfs:label>
    </owl:DatatypeProperty>
    


    <!-- http://postdata.linhd.uned.es/ontology/postdata-core#narrativeLocation -->

    <owl:DatatypeProperty rdf:about="http://postdata.linhd.uned.es/ontology/postdata-core#narrativeLocation">
        <rdfs:domain>
            <owl:Class>
                <owl:unionOf rdf:parseType="Collection">
                    <rdf:Description rdf:about="http://postdata.linhd.uned.es/ontology/postdata-core#PoeticWork"/>
                    <rdf:Description rdf:about="http://postdata.linhd.uned.es/ontology/postdata-core#Redaction"/>
                </owl:unionOf>
            </owl:Class>
        </rdfs:domain>
        <rdfs:range rdf:resource="http://www.w3.org/2001/XMLSchema#string"/>
        <rdfs:comment xml:lang="en">Location of the narrative. There is at most one possible location for a Redaction or Poetic Work.

Taking as example the poem “Cantar de Mio Cid”, the “narrativeLocation” would be “Spain”.</rdfs:comment>
        <rdfs:isDefinedBy>http://postdata.linhd.uned.es/ontology/postdata-core/</rdfs:isDefinedBy>
        <rdfs:label xml:lang="en">narrative Location</rdfs:label>
    </owl:DatatypeProperty>
    


    <!-- http://postdata.linhd.uned.es/ontology/postdata-core#nationality -->

    <owl:DatatypeProperty rdf:about="http://postdata.linhd.uned.es/ontology/postdata-core#nationality">
        <rdfs:domain rdf:resource="http://postdata.linhd.uned.es/ontology/postdata-core#Person"/>
        <rdfs:range rdf:resource="http://www.w3.org/2001/XMLSchema#string"/>
        <rdfs:comment xml:lang="en">An ethnic group forming a part of one or more political nations that is assigned to a Person.

Taking as example, the poet “Antonio Machado”, his “nationality” would be “Spanish”.</rdfs:comment>
        <rdfs:isDefinedBy>http://postdata.linhd.uned.es/ontology/postdata-core/</rdfs:isDefinedBy>
        <rdfs:label xml:lang="en">nationality</rdfs:label>
    </owl:DatatypeProperty>
    


    <!-- http://postdata.linhd.uned.es/ontology/postdata-core#numberOfLines -->

    <owl:DatatypeProperty rdf:about="http://postdata.linhd.uned.es/ontology/postdata-core#numberOfLines">
        <rdfs:domain rdf:resource="http://postdata.linhd.uned.es/ontology/postdata-core#Ensemble"/>
        <rdfs:range rdf:resource="http://www.w3.org/2001/XMLSchema#integer"/>
        <rdfs:comment xml:lang="en">Number of total lines comprising the Ensemble.

Taking as example La vida es sueño by Calderón de la Barca, number of lines is 3319.</rdfs:comment>
        <rdfs:isDefinedBy>http://postdata.linhd.uned.es/ontology/postdata-core/</rdfs:isDefinedBy>
        <rdfs:label xml:lang="en">number of Lines</rdfs:label>
    </owl:DatatypeProperty>
    


    <!-- http://postdata.linhd.uned.es/ontology/postdata-core#numberOfPlays -->

    <owl:DatatypeProperty rdf:about="http://postdata.linhd.uned.es/ontology/postdata-core#numberOfPlays">
        <rdfs:domain rdf:resource="http://postdata.linhd.uned.es/ontology/postdata-core#Ensemble"/>
        <rdfs:range rdf:resource="http://www.w3.org/2001/XMLSchema#integer"/>
        <rdfs:comment xml:lang="en">Number of plays of an Ensemble</rdfs:comment>
        <rdfs:isDefinedBy>http://postdata.linhd.uned.es/ontology/postdata-core/</rdfs:isDefinedBy>
        <rdfs:label xml:lang="en">number of Plays</rdfs:label>
    </owl:DatatypeProperty>
    


    <!-- http://postdata.linhd.uned.es/ontology/postdata-core#numberOfPoems -->

    <owl:DatatypeProperty rdf:about="http://postdata.linhd.uned.es/ontology/postdata-core#numberOfPoems">
        <rdfs:domain rdf:resource="http://postdata.linhd.uned.es/ontology/postdata-core#Ensemble"/>
        <rdfs:range rdf:resource="http://www.w3.org/2001/XMLSchema#integer"/>
        <rdfs:comment xml:lang="en">Number of poems of an Ensemble</rdfs:comment>
        <rdfs:isDefinedBy>http://postdata.linhd.uned.es/ontology/postdata-core/</rdfs:isDefinedBy>
        <rdfs:label xml:lang="en">number of poems</rdfs:label>
    </owl:DatatypeProperty>
    


    <!-- http://postdata.linhd.uned.es/ontology/postdata-core#numberOfWitnessesUsed -->

    <owl:DatatypeProperty rdf:about="http://postdata.linhd.uned.es/ontology/postdata-core#numberOfWitnessesUsed">
        <rdfs:domain rdf:resource="http://postdata.linhd.uned.es/ontology/postdata-core#Redaction"/>
        <rdfs:range rdf:resource="http://www.w3.org/2001/XMLSchema#integer"/>
        <rdfs:comment xml:lang="en">Number of Primary Sources used in the elaboration of a Redaction.</rdfs:comment>
        <rdfs:isDefinedBy>http://postdata.linhd.uned.es/ontology/postdata-core/</rdfs:isDefinedBy>
        <rdfs:label xml:lang="en">number of Witnesses Used</rdfs:label>
    </owl:DatatypeProperty>
    


    <!-- http://postdata.linhd.uned.es/ontology/postdata-core#originalLanguage -->

    <owl:DatatypeProperty rdf:about="http://postdata.linhd.uned.es/ontology/postdata-core#originalLanguage">
        <rdfs:domain rdf:resource="http://postdata.linhd.uned.es/ontology/postdata-core#Redaction"/>
        <rdfs:range>
            <rdfs:Datatype>
                <owl:unionOf rdf:parseType="Collection">
                    <rdf:Description rdf:about="http://www.w3.org/2001/XMLSchema#language"/>
                    <rdf:Description rdf:about="http://www.w3.org/2001/XMLSchema#string"/>
                </owl:unionOf>
            </rdfs:Datatype>
        </rdfs:range>
        <rdfs:comment xml:lang="en">The language from which the Redaction is a translation</rdfs:comment>
        <rdfs:isDefinedBy>http://postdata.linhd.uned.es/ontology/postdata-core/</rdfs:isDefinedBy>
        <rdfs:label xml:lang="en">original Language</rdfs:label>
    </owl:DatatypeProperty>
    


    <!-- http://postdata.linhd.uned.es/ontology/postdata-core#originalName -->

    <owl:DatatypeProperty rdf:about="http://postdata.linhd.uned.es/ontology/postdata-core#originalName">
        <rdfs:subPropertyOf rdf:resource="http://www.w3.org/2002/07/owl#topDataProperty"/>
        <rdfs:range rdf:resource="http://www.w3.org/2001/XMLSchema#string"/>
        <rdfs:comment xml:lang="en">Name of a Place as it appears in the source text</rdfs:comment>
        <rdfs:isDefinedBy>http://postdata.linhd.uned.es/ontology/postdata-core/</rdfs:isDefinedBy>
        <rdfs:label xml:lang="en">original Name</rdfs:label>
    </owl:DatatypeProperty>
    


    <!-- http://postdata.linhd.uned.es/ontology/postdata-core#originalTitle -->

    <owl:DatatypeProperty rdf:about="http://postdata.linhd.uned.es/ontology/postdata-core#originalTitle">
        <rdfs:domain>
            <owl:Class>
                <owl:unionOf rdf:parseType="Collection">
                    <rdf:Description rdf:about="http://postdata.linhd.uned.es/ontology/postdata-core#PoeticWork"/>
                    <rdf:Description rdf:about="http://postdata.linhd.uned.es/ontology/postdata-core#Redaction"/>
                </owl:unionOf>
            </owl:Class>
        </rdfs:domain>
        <rdfs:range rdf:resource="http://www.w3.org/2001/XMLSchema#string"/>
        <rdfs:comment xml:lang="en">The identifying name of a Redaction or Poetic Work as it appears in its primary source. There is at most one possible original title.</rdfs:comment>
        <rdfs:isDefinedBy>http://postdata.linhd.uned.es/ontology/postdata-core/</rdfs:isDefinedBy>
        <rdfs:label xml:lang="en">original Title</rdfs:label>
    </owl:DatatypeProperty>
    


    <!-- http://postdata.linhd.uned.es/ontology/postdata-core#paraphrasis -->

    <owl:DatatypeProperty rdf:about="http://postdata.linhd.uned.es/ontology/postdata-core#paraphrasis">
        <rdfs:domain rdf:resource="http://postdata.linhd.uned.es/ontology/postdata-core#Redaction"/>
        <rdfs:range rdf:resource="http://www.w3.org/2001/XMLSchema#string"/>
        <rdfs:comment xml:lang="en">The recasting of the contents in words different from that originally used in a Redaction, whether in the same language or in a translation. A Redaction may have zero or one paraphrasis associated.</rdfs:comment>
        <rdfs:isDefinedBy>http://postdata.linhd.uned.es/ontology/postdata-core/</rdfs:isDefinedBy>
        <rdfs:label xml:lang="en">paraphrasis</rdfs:label>
    </owl:DatatypeProperty>
    


    <!-- http://postdata.linhd.uned.es/ontology/postdata-core#penName -->

    <owl:DatatypeProperty rdf:about="http://postdata.linhd.uned.es/ontology/postdata-core#penName">
        <rdfs:domain rdf:resource="http://postdata.linhd.uned.es/ontology/postdata-core#CreatorRole"/>
        <rdfs:range rdf:resource="http://www.w3.org/2001/XMLSchema#string"/>
        <rdfs:comment xml:lang="en">A fictitious name, especially a pen name. A variant name.

This property is used to describe an Agent Role entity as the pen name may vary for the same Agent in different Redactions.</rdfs:comment>
        <rdfs:isDefinedBy>http://postdata.linhd.uned.es/ontology/postdata-core/</rdfs:isDefinedBy>
        <rdfs:label xml:lang="en">pen Name</rdfs:label>
    </owl:DatatypeProperty>
    


    <!-- http://postdata.linhd.uned.es/ontology/postdata-core#portrait -->

    <owl:DatatypeProperty rdf:about="http://postdata.linhd.uned.es/ontology/postdata-core#portrait">
        <rdfs:domain rdf:resource="http://postdata.linhd.uned.es/ontology/postdata-core#Person"/>
        <rdfs:range rdf:resource="http://www.w3.org/2001/XMLSchema#anyURI"/>
        <rdfs:comment xml:lang="en">URL to a digital image file that depicts a given Person.

For Miguel de Cervantes, one of his most famous portraits is available at: https://commons.wikimedia.org/wiki/Category:Miguel_de_Cervantes#/media/File:Cervantes_J%C3%A1uregui.jpg</rdfs:comment>
        <rdfs:isDefinedBy>http://postdata.linhd.uned.es/ontology/postdata-core/</rdfs:isDefinedBy>
        <rdfs:label xml:lang="en">portrait</rdfs:label>
    </owl:DatatypeProperty>
    


    <!-- http://postdata.linhd.uned.es/ontology/postdata-core#positionName -->

    <owl:DatatypeProperty rdf:about="http://postdata.linhd.uned.es/ontology/postdata-core#positionName">
        <rdfs:subPropertyOf rdf:resource="http://www.w3.org/2002/07/owl#topDataProperty"/>
        <rdfs:domain rdf:resource="http://postdata.linhd.uned.es/ontology/postdata-core#Person"/>
        <rdfs:range rdf:resource="http://www.w3.org/2001/XMLSchema#string"/>
        <rdfs:comment xml:lang="en">Contains a name component which indicates that a referent Person has a particular role or position in society, such as an official title or rank.

For example, if we consider the poet &quot;Sir Philip Sidney&quot;, his position name is &quot;sir&quot;.</rdfs:comment>
        <rdfs:isDefinedBy>http://postdata.linhd.uned.es/ontology/postdata-core/</rdfs:isDefinedBy>
        <rdfs:label xml:lang="en">position Name</rdfs:label>
    </owl:DatatypeProperty>
    


    <!-- http://postdata.linhd.uned.es/ontology/postdata-core#sampleText -->

    <owl:DatatypeProperty rdf:about="http://postdata.linhd.uned.es/ontology/postdata-core#sampleText">
        <rdfs:domain rdf:resource="http://postdata.linhd.uned.es/ontology/postdata-core#Redaction"/>
        <rdfs:range rdf:resource="http://www.w3.org/2001/XMLSchema#string"/>
        <rdfs:comment xml:lang="en">Excerpt of a Redaction.</rdfs:comment>
        <rdfs:isDefinedBy>http://postdata.linhd.uned.es/ontology/postdata-core/</rdfs:isDefinedBy>
        <rdfs:label xml:lang="en">sample Text</rdfs:label>
    </owl:DatatypeProperty>
    


    <!-- http://postdata.linhd.uned.es/ontology/postdata-core#subtitle -->

    <owl:DatatypeProperty rdf:about="http://postdata.linhd.uned.es/ontology/postdata-core#subtitle">
        <rdf:type rdf:resource="http://www.w3.org/2002/07/owl#FunctionalProperty"/>
        <rdfs:domain>
            <owl:Class>
                <owl:unionOf rdf:parseType="Collection">
                    <rdf:Description rdf:about="http://postdata.linhd.uned.es/ontology/postdata-core#PoeticWork"/>
                    <rdf:Description rdf:about="http://postdata.linhd.uned.es/ontology/postdata-core#Redaction"/>
                </owl:unionOf>
            </owl:Class>
        </rdfs:domain>
        <rdfs:range rdf:resource="http://www.w3.org/2001/XMLSchema#string"/>
        <rdfs:comment xml:lang="en">A secondary, usually explanatory title</rdfs:comment>
        <rdfs:isDefinedBy>http://postdata.linhd.uned.es/ontology/postdata-core/</rdfs:isDefinedBy>
        <rdfs:label xml:lang="en">subtitle</rdfs:label>
    </owl:DatatypeProperty>
    


    <!-- http://postdata.linhd.uned.es/ontology/postdata-core#surname -->

    <owl:DatatypeProperty rdf:about="http://postdata.linhd.uned.es/ontology/postdata-core#surname">
        <rdfs:domain rdf:resource="http://postdata.linhd.uned.es/ontology/postdata-core#Person"/>
        <rdfs:range rdf:resource="http://www.w3.org/2001/XMLSchema#string"/>
        <rdfs:comment xml:lang="en">Contains a family (inherited) name, as opposed to a given, baptismal, or nick name of a Person.

Taking as example the poet Dante Alighieri, &quot;surname&quot; is &quot;Alighieri&quot;.</rdfs:comment>
        <rdfs:isDefinedBy>http://postdata.linhd.uned.es/ontology/postdata-core/</rdfs:isDefinedBy>
        <rdfs:label xml:lang="en">surname</rdfs:label>
    </owl:DatatypeProperty>
    


    <!-- http://postdata.linhd.uned.es/ontology/postdata-core#text -->

    <owl:DatatypeProperty rdf:about="http://postdata.linhd.uned.es/ontology/postdata-core#text">
        <rdfs:domain rdf:resource="http://postdata.linhd.uned.es/ontology/postdata-core#Redaction"/>
        <rdfs:range rdf:resource="http://www.w3.org/2001/XMLSchema#string"/>
        <rdfs:comment xml:lang="en">Reference to textual contents . The contents of this property do not allow finer analysis by stanza or line. It can be a text of a diplomatic edition, semidiplomatic edition or of a critical edition (among others) or even a translation. The property typeOfRedaction defines the type of Edition or if it is a translation. There is only one possible text value for each Redaction.</rdfs:comment>
        <rdfs:isDefinedBy>http://postdata.linhd.uned.es/ontology/postdata-core/</rdfs:isDefinedBy>
        <rdfs:label xml:lang="en">text</rdfs:label>
    </owl:DatatypeProperty>
    


    <!-- http://postdata.linhd.uned.es/ontology/postdata-core#theme -->

    <owl:DatatypeProperty rdf:about="http://postdata.linhd.uned.es/ontology/postdata-core#theme">
        <rdfs:domain rdf:resource="http://postdata.linhd.uned.es/ontology/postdata-core#PoeticWork"/>
        <rdfs:range rdf:resource="http://www.w3.org/2001/XMLSchema#string"/>
        <rdfs:comment xml:lang="en">Subject or topic a Poetic Work is related to.</rdfs:comment>
        <rdfs:label xml:lang="en">theme</rdfs:label>
    </owl:DatatypeProperty>
    


    <!-- http://postdata.linhd.uned.es/ontology/postdata-core#typeOfEvent -->

    <owl:DatatypeProperty rdf:about="http://postdata.linhd.uned.es/ontology/postdata-core#typeOfEvent">
        <rdfs:domain rdf:resource="http://postdata.linhd.uned.es/ontology/postdata-core#Event"/>
        <rdfs:range rdf:resource="http://www.w3.org/2001/XMLSchema#string"/>
        <rdfs:comment xml:lang="en">The type of event, for instance its modality (real, fictional...).</rdfs:comment>
        <rdfs:isDefinedBy>http://postdata.linhd.uned.es/ontology/postdata-core/</rdfs:isDefinedBy>
        <rdfs:label xml:lang="en">type of Event</rdfs:label>
    </owl:DatatypeProperty>
    


    <!-- http://postdata.linhd.uned.es/ontology/postdata-core#typeOfPlace -->

    <owl:DatatypeProperty rdf:about="http://postdata.linhd.uned.es/ontology/postdata-core#typeOfPlace">
        <rdfs:subPropertyOf rdf:resource="http://www.w3.org/2002/07/owl#topDataProperty"/>
        <rdfs:domain rdf:resource="http://postdata.linhd.uned.es/ontology/postdata-core#Place"/>
        <rdfs:range rdf:resource="http://www.w3.org/2001/XMLSchema#string"/>
        <rdfs:comment xml:lang="en">Type of Place (e.g. fictional)</rdfs:comment>
        <rdfs:isDefinedBy>http://postdata.linhd.uned.es/ontology/postdata-core/</rdfs:isDefinedBy>
        <rdfs:label xml:lang="en">type of Place</rdfs:label>
    </owl:DatatypeProperty>
    


    <!-- http://postdata.linhd.uned.es/ontology/postdata-core#typeOfRedaction -->

    <owl:DatatypeProperty rdf:about="http://postdata.linhd.uned.es/ontology/postdata-core#typeOfRedaction">
        <rdfs:domain rdf:resource="http://postdata.linhd.uned.es/ontology/postdata-core#Redaction"/>
        <rdfs:range rdf:resource="http://www.w3.org/2001/XMLSchema#string"/>
        <rdfs:comment xml:lang="en">The type of the text provided in the Redaction
Eg.: Diplomatic edition, critical edition, translation</rdfs:comment>
        <rdfs:isDefinedBy>http://postdata.linhd.uned.es/ontology/postdata-core/</rdfs:isDefinedBy>
        <rdfs:label xml:lang="en">type of Redaction</rdfs:label>
    </owl:DatatypeProperty>
    


    <!-- http://postdata.linhd.uned.es/ontology/postdata-core#workNumber -->

    <owl:DatatypeProperty rdf:about="http://postdata.linhd.uned.es/ontology/postdata-core#workNumber">
        <rdfs:domain rdf:resource="http://postdata.linhd.uned.es/ontology/postdata-core#Redaction"/>
        <rdfs:range rdf:resource="http://www.w3.org/2001/XMLSchema#string"/>
        <rdfs:comment xml:lang="en">Number that identifies the Redaction inside a collection. There can only be one value associated for each Redaction.</rdfs:comment>
        <rdfs:isDefinedBy>http://postdata.linhd.uned.es/ontology/postdata-core/</rdfs:isDefinedBy>
        <rdfs:label xml:lang="en">work Number</rdfs:label>
    </owl:DatatypeProperty>
    


    <!-- https://schema.org/latitude -->

    <owl:DatatypeProperty rdf:about="https://schema.org/latitude">
        <rdfs:domain rdf:resource="http://postdata.linhd.uned.es/ontology/postdata-core#Place"/>
        <rdfs:range rdf:resource="http://www.w3.org/2001/XMLSchema#string"/>
        <rdfs:comment xml:lang="en">The latitude of a location. For example 37.42242 (WGS 84).</rdfs:comment>
        <rdfs:label xml:lang="en">latitude</rdfs:label>
    </owl:DatatypeProperty>
    


    <!-- https://schema.org/longitude -->

    <owl:DatatypeProperty rdf:about="https://schema.org/longitude">
        <rdfs:domain rdf:resource="http://postdata.linhd.uned.es/ontology/postdata-core#Place"/>
        <rdfs:range rdf:resource="http://www.w3.org/2001/XMLSchema#string"/>
        <rdfs:comment xml:lang="en">The longitude of a location. For example -122.08585 (WGS 84).</rdfs:comment>
        <rdfs:label xml:lang="en">longitude</rdfs:label>
    </owl:DatatypeProperty>
    


    <!-- 
    ///////////////////////////////////////////////////////////////////////////////////////
    //
    // Classes
    //
    ///////////////////////////////////////////////////////////////////////////////////////
     -->

    


    <!-- http://iflastandards.info/ns/fr/frbr/frbroo/F1 -->

    <owl:Class rdf:about="http://iflastandards.info/ns/fr/frbr/frbroo/F1"/>
    


    <!-- http://iflastandards.info/ns/fr/frbr/frbroo/F14 -->

    <owl:Class rdf:about="http://iflastandards.info/ns/fr/frbr/frbroo/F14">
        <rdfs:subClassOf rdf:resource="http://iflastandards.info/ns/fr/frbr/frbroo/F1"/>
    </owl:Class>
    


    <!-- http://iflastandards.info/ns/fr/frbr/frbroo/F17 -->

    <owl:Class rdf:about="http://iflastandards.info/ns/fr/frbr/frbroo/F17">
        <rdfs:subClassOf rdf:resource="http://iflastandards.info/ns/fr/frbr/frbroo/F14"/>
    </owl:Class>
    


    <!-- http://iflastandards.info/ns/fr/frbr/frbroo/F2 -->

    <owl:Class rdf:about="http://iflastandards.info/ns/fr/frbr/frbroo/F2"/>
    


    <!-- http://iflastandards.info/ns/fr/frbr/frbroo/F22 -->

    <owl:Class rdf:about="http://iflastandards.info/ns/fr/frbr/frbroo/F22">
        <rdfs:subClassOf rdf:resource="http://iflastandards.info/ns/fr/frbr/frbroo/F2"/>
    </owl:Class>
    


    <!-- http://postdata.linhd.uned.es/ontology/postdata-core#Agent -->

    <owl:Class rdf:about="http://postdata.linhd.uned.es/ontology/postdata-core#Agent">
        <rdfs:subClassOf>
            <owl:Restriction>
                <owl:onProperty rdf:resource="http://postdata.linhd.uned.es/ontology/postdata-core#isInvolvedIn"/>
                <owl:allValuesFrom rdf:resource="http://postdata.linhd.uned.es/ontology/postdata-core#Event"/>
            </owl:Restriction>
        </rdfs:subClassOf>
        <rdfs:subClassOf>
            <owl:Restriction>
                <owl:onProperty rdf:resource="http://postdata.linhd.uned.es/ontology/postdata-core#isMentionedIn"/>
                <owl:allValuesFrom rdf:resource="http://postdata.linhd.uned.es/ontology/postdata-core#Redaction"/>
            </owl:Restriction>
        </rdfs:subClassOf>
        <rdfs:comment xml:lang="en">Any agentive Object , either physical or social. In the context of the POSTDATA ontology network it will mostly refer to organisations or persons.

This class it is based on CIDOC CRM E39 Actor Class.</rdfs:comment>
        <rdfs:isDefinedBy>http://postdata.linhd.uned.es/ontology/postdata-core/</rdfs:isDefinedBy>
        <rdfs:label xml:lang="en">Agent</rdfs:label>
    </owl:Class>
    


    <!-- http://postdata.linhd.uned.es/ontology/postdata-core#AgentRole -->

    <owl:Class rdf:about="http://postdata.linhd.uned.es/ontology/postdata-core#AgentRole">
        <rdfs:subClassOf>
            <owl:Restriction>
                <owl:onProperty rdf:resource="http://postdata.linhd.uned.es/ontology/postdata-core#date"/>
                <owl:allValuesFrom rdf:resource="http://postdata.linhd.uned.es/ontology/postdata-dates#DateEntity"/>
            </owl:Restriction>
        </rdfs:subClassOf>
        <rdfs:subClassOf>
            <owl:Restriction>
                <owl:onProperty rdf:resource="http://postdata.linhd.uned.es/ontology/postdata-core#roleFunction"/>
                <owl:qualifiedCardinality rdf:datatype="http://www.w3.org/2001/XMLSchema#nonNegativeInteger">1</owl:qualifiedCardinality>
                <owl:onClass>
                    <owl:Class>
                        <owl:intersectionOf rdf:parseType="Collection">
                            <rdf:Description rdf:about="http://www.w3.org/2004/02/skos/core#Concept"/>
                            <owl:Restriction>
                                <owl:onProperty rdf:resource="http://www.w3.org/2004/02/skos/core#inScheme"/>
                                <owl:hasValue rdf:resource="http://postdata.linhd.uned.es/kos/role-function"/>
                            </owl:Restriction>
                        </owl:intersectionOf>
                    </owl:Class>
                </owl:onClass>
            </owl:Restriction>
        </rdfs:subClassOf>
        <rdfs:subClassOf>
            <owl:Restriction>
                <owl:onProperty rdf:resource="http://postdata.linhd.uned.es/ontology/postdata-core#certainty"/>
                <owl:maxQualifiedCardinality rdf:datatype="http://www.w3.org/2001/XMLSchema#nonNegativeInteger">1</owl:maxQualifiedCardinality>
                <owl:onClass>
                    <owl:Class>
                        <owl:intersectionOf rdf:parseType="Collection">
                            <rdf:Description rdf:about="http://www.w3.org/2004/02/skos/core#Concept"/>
                            <owl:Restriction>
                                <owl:onProperty rdf:resource="http://www.w3.org/2004/02/skos/core#inScheme"/>
                                <owl:hasValue rdf:resource="http://postdata.linhd.uned.es/kos/certainty"/>
                            </owl:Restriction>
                        </owl:intersectionOf>
                    </owl:Class>
                </owl:onClass>
            </owl:Restriction>
        </rdfs:subClassOf>
        <rdfs:comment xml:lang="en">This class relates a work (e.g., poetic work, redaction, other transmission elements) and an Agent (Person or Organisation), and allows specifying the role that the agent plays in such work (e.g., creator, sponsor, editor).

This class is based on the agent-role Ontology Design Pattern:
- http://www.ontologydesignpatterns.org/cp/owl/agentrole.owl
- http://www.ontologydesignpatterns.org/cp/owl/objectrole.owl</rdfs:comment>
        <rdfs:isDefinedBy>http://postdata.linhd.uned.es/ontology/postdata-core/</rdfs:isDefinedBy>
        <rdfs:label xml:lang="en">AgentRole</rdfs:label>
    </owl:Class>
    


    <!-- http://postdata.linhd.uned.es/ontology/postdata-core#CreatorRole -->

    <owl:Class rdf:about="http://postdata.linhd.uned.es/ontology/postdata-core#CreatorRole">
        <rdfs:subClassOf>
            <owl:Class>
                <owl:intersectionOf rdf:parseType="Collection">
                    <rdf:Description rdf:about="http://postdata.linhd.uned.es/ontology/postdata-core#AgentRole"/>
                    <owl:Restriction>
                        <owl:onProperty rdf:resource="http://postdata.linhd.uned.es/ontology/postdata-core#roleFunction"/>
                        <owl:hasValue rdf:resource="http://postdata.linhd.uned.es/ontology/postdata-core#Creator"/>
                    </owl:Restriction>
                </owl:intersectionOf>
            </owl:Class>
        </rdfs:subClassOf>
        <rdfs:subClassOf>
            <owl:Restriction>
                <owl:onProperty rdf:resource="http://postdata.linhd.uned.es/ontology/postdata-core#certainty"/>
                <owl:maxQualifiedCardinality rdf:datatype="http://www.w3.org/2001/XMLSchema#nonNegativeInteger">1</owl:maxQualifiedCardinality>
                <owl:onClass>
                    <owl:Class>
                        <owl:intersectionOf rdf:parseType="Collection">
                            <rdf:Description rdf:about="http://www.w3.org/2004/02/skos/core#Concept"/>
                            <owl:Restriction>
                                <owl:onProperty rdf:resource="http://www.w3.org/2004/02/skos/core#inScheme"/>
                                <owl:hasValue rdf:resource="http://postdata.linhd.uned.es/kos/certainty"/>
                            </owl:Restriction>
                        </owl:intersectionOf>
                    </owl:Class>
                </owl:onClass>
            </owl:Restriction>
        </rdfs:subClassOf>
        <rdfs:subClassOf>
            <owl:Restriction>
                <owl:onProperty rdf:resource="http://postdata.linhd.uned.es/ontology/postdata-core#typeOfDesignation"/>
                <owl:maxQualifiedCardinality rdf:datatype="http://www.w3.org/2001/XMLSchema#nonNegativeInteger">1</owl:maxQualifiedCardinality>
                <owl:onClass>
                    <owl:Class>
                        <owl:intersectionOf rdf:parseType="Collection">
                            <rdf:Description rdf:about="http://www.w3.org/2004/02/skos/core#Concept"/>
                            <owl:Restriction>
                                <owl:onProperty rdf:resource="http://www.w3.org/2004/02/skos/core#inScheme"/>
                                <owl:hasValue rdf:resource="http://postdata.linhd.uned.es/kos/designation-type"/>
                            </owl:Restriction>
                        </owl:intersectionOf>
                    </owl:Class>
                </owl:onClass>
            </owl:Restriction>
        </rdfs:subClassOf>
        <rdfs:subClassOf>
            <owl:Restriction>
                <owl:onProperty rdf:resource="http://postdata.linhd.uned.es/ontology/postdata-core#penName"/>
                <owl:maxQualifiedCardinality rdf:datatype="http://www.w3.org/2001/XMLSchema#nonNegativeInteger">1</owl:maxQualifiedCardinality>
                <owl:onDataRange rdf:resource="http://www.w3.org/2001/XMLSchema#string"/>
            </owl:Restriction>
        </rdfs:subClassOf>
        <rdfs:comment xml:lang="en">The CreatorRole class models the role that an agent plays with respect to the creation or authorship of a work. In this sense, it has specific properties that are important for the study of authorship of poetic works.
These properties are:
penName - It is common for authors to use an alias
isAnonymous - In many of the works, especially the older ones, the author is not known and this is an aspect that should be considered.
isWrongAttribution - Sometimes, especially in older works as well, attributions of authorship have been made that are not correct, but this fact is considered an important aspect for scholars of the subject.
typeofDesignation, which is the type of name or designation used, e.g. pseudonyms, heteronyms, etc.</rdfs:comment>
        <rdfs:isDefinedBy>http://postdata.linhd.uned.es/ontology/postdata-core/</rdfs:isDefinedBy>
        <rdfs:label xml:lang="en">Creator Role</rdfs:label>
    </owl:Class>
    


    <!-- http://postdata.linhd.uned.es/ontology/postdata-core#Ensemble -->

    <owl:Class rdf:about="http://postdata.linhd.uned.es/ontology/postdata-core#Ensemble">
        <rdfs:subClassOf rdf:resource="http://iflastandards.info/ns/fr/frbr/frbroo/F17"/>
        <rdfs:subClassOf>
            <owl:Restriction>
                <owl:onProperty rdf:resource="http://postdata.linhd.uned.es/ontology/postdata-core#date"/>
                <owl:allValuesFrom rdf:resource="http://postdata.linhd.uned.es/ontology/postdata-dates#DateEntity"/>
            </owl:Restriction>
        </rdfs:subClassOf>
        <rdfs:subClassOf>
            <owl:Restriction>
                <owl:onProperty rdf:resource="http://postdata.linhd.uned.es/ontology/postdata-core#isFrom"/>
                <owl:allValuesFrom rdf:resource="http://postdata.linhd.uned.es/ontology/postdata-core#Place"/>
            </owl:Restriction>
        </rdfs:subClassOf>
        <rdfs:subClassOf>
            <owl:Restriction>
                <owl:onProperty rdf:resource="http://postdata.linhd.uned.es/ontology/postdata-core#isReferencedIn"/>
                <owl:allValuesFrom rdf:resource="http://postdata.linhd.uned.es/ontology/postdata-transmission#Location"/>
            </owl:Restriction>
        </rdfs:subClassOf>
        <rdfs:subClassOf>
            <owl:Restriction>
                <owl:onProperty rdf:resource="http://postdata.linhd.uned.es/ontology/postdata-core#hasProvenance"/>
                <owl:maxQualifiedCardinality rdf:datatype="http://www.w3.org/2001/XMLSchema#nonNegativeInteger">1</owl:maxQualifiedCardinality>
                <owl:onClass rdf:resource="http://postdata.linhd.uned.es/ontology/postdata-core#Place"/>
            </owl:Restriction>
        </rdfs:subClassOf>
        <rdfs:subClassOf>
            <owl:Restriction>
                <owl:onProperty rdf:resource="http://postdata.linhd.uned.es/ontology/postdata-core#numberOfLines"/>
                <owl:maxQualifiedCardinality rdf:datatype="http://www.w3.org/2001/XMLSchema#nonNegativeInteger">1</owl:maxQualifiedCardinality>
                <owl:onDataRange rdf:resource="http://www.w3.org/2001/XMLSchema#integer"/>
            </owl:Restriction>
        </rdfs:subClassOf>
        <rdfs:subClassOf>
            <owl:Restriction>
                <owl:onProperty rdf:resource="http://postdata.linhd.uned.es/ontology/postdata-core#numberOfPlays"/>
                <owl:maxQualifiedCardinality rdf:datatype="http://www.w3.org/2001/XMLSchema#nonNegativeInteger">1</owl:maxQualifiedCardinality>
                <owl:onDataRange rdf:resource="http://www.w3.org/2001/XMLSchema#integer"/>
            </owl:Restriction>
        </rdfs:subClassOf>
        <rdfs:subClassOf>
            <owl:Restriction>
                <owl:onProperty rdf:resource="http://postdata.linhd.uned.es/ontology/postdata-core#numberOfPoems"/>
                <owl:maxQualifiedCardinality rdf:datatype="http://www.w3.org/2001/XMLSchema#nonNegativeInteger">1</owl:maxQualifiedCardinality>
                <owl:onDataRange rdf:resource="http://www.w3.org/2001/XMLSchema#integer"/>
            </owl:Restriction>
        </rdfs:subClassOf>
        <rdfs:comment xml:lang="en">An abstract work that contains more than one Poetic Work. An Ensemble might be conceived as a collection of works, organized by author, by book song, by book of poems; or as a work mainly written in prose that contains more than one poetic pieces (each one of them being its own Poetic Work). For example, Les fleurs du mal.

This class is based on CIDOC FRBR F17 Aggregation Work Class, ant it is subclass of edm:providedCHO to keep alignement with Europeana Data Model.</rdfs:comment>
        <rdfs:isDefinedBy>http://postdata.linhd.uned.es/ontology/postdata-core/</rdfs:isDefinedBy>
        <rdfs:label xml:lang="en">Ensemble</rdfs:label>
    </owl:Class>
    


    <!-- http://postdata.linhd.uned.es/ontology/postdata-core#Event -->

    <owl:Class rdf:about="http://postdata.linhd.uned.es/ontology/postdata-core#Event">
        <rdfs:subClassOf>
            <owl:Restriction>
                <owl:onProperty rdf:resource="http://postdata.linhd.uned.es/ontology/postdata-core#date"/>
                <owl:allValuesFrom rdf:resource="http://postdata.linhd.uned.es/ontology/postdata-dates#DateEntity"/>
            </owl:Restriction>
        </rdfs:subClassOf>
        <rdfs:subClassOf>
            <owl:Restriction>
                <owl:onProperty rdf:resource="http://postdata.linhd.uned.es/ontology/postdata-core#isMentionedIn"/>
                <owl:allValuesFrom rdf:resource="http://postdata.linhd.uned.es/ontology/postdata-core#Redaction"/>
            </owl:Restriction>
        </rdfs:subClassOf>
        <rdfs:subClassOf>
            <owl:Restriction>
                <owl:onProperty rdf:resource="http://postdata.linhd.uned.es/ontology/postdata-core#eventNarration"/>
                <owl:maxCardinality rdf:datatype="http://www.w3.org/2001/XMLSchema#nonNegativeInteger">1</owl:maxCardinality>
            </owl:Restriction>
        </rdfs:subClassOf>
        <rdfs:comment xml:lang="en">Something that happens or takes place. It is generally mentioned in the text (Redaction) and represented using isMentionedin property.

This class is based on CIDOC CRM E5 Event Class. Nevertheless, in the context of POSTDATA project, we restrict to the description of those events that are mentioned in poems (pdcore:Redaction class) rather than adopting an event-centric approach in which events are used to describe the modifications suffered by the poem itslef.</rdfs:comment>
        <rdfs:isDefinedBy>http://postdata.linhd.uned.es/ontology/postdata-core/</rdfs:isDefinedBy>
        <rdfs:label xml:lang="en">Event</rdfs:label>
    </owl:Class>
    


    <!-- http://postdata.linhd.uned.es/ontology/postdata-core#Organisation -->

    <owl:Class rdf:about="http://postdata.linhd.uned.es/ontology/postdata-core#Organisation">
        <rdfs:subClassOf rdf:resource="http://postdata.linhd.uned.es/ontology/postdata-core#Agent"/>
        <rdfs:subClassOf>
            <owl:Restriction>
                <owl:onProperty rdf:resource="http://postdata.linhd.uned.es/ontology/postdata-core#isFrom"/>
                <owl:allValuesFrom rdf:resource="http://postdata.linhd.uned.es/ontology/postdata-core#Place"/>
            </owl:Restriction>
        </rdfs:subClassOf>
        <rdfs:comment xml:lang="en">Named collection of people regarded as a single unit. Typical examples include institutions such as ‘UNED’ or ‘the BBC’ and businesses such as ‘Google’ but also racial or ethnic groupings or political factions where these are regarded as forming a single agency such as ‘the Carthaginians’ or ‘the Communists’.

This class is defined as a subclass of pdcore:Agent and it is based on CIDOC CRM E74 Group Class.</rdfs:comment>
        <rdfs:isDefinedBy>http://postdata.linhd.uned.es/ontology/postdata-core/</rdfs:isDefinedBy>
        <rdfs:label xml:lang="en">Organisation</rdfs:label>
    </owl:Class>
    


    <!-- http://postdata.linhd.uned.es/ontology/postdata-core#Person -->

    <owl:Class rdf:about="http://postdata.linhd.uned.es/ontology/postdata-core#Person">
        <rdfs:subClassOf rdf:resource="http://postdata.linhd.uned.es/ontology/postdata-core#Agent"/>
        <rdfs:subClassOf>
            <owl:Restriction>
                <owl:onProperty rdf:resource="http://postdata.linhd.uned.es/ontology/postdata-core#birthDate"/>
                <owl:allValuesFrom rdf:resource="http://postdata.linhd.uned.es/ontology/postdata-dates#DateEntity"/>
            </owl:Restriction>
        </rdfs:subClassOf>
        <rdfs:subClassOf>
            <owl:Restriction>
                <owl:onProperty rdf:resource="http://postdata.linhd.uned.es/ontology/postdata-core#birthPlace"/>
                <owl:allValuesFrom rdf:resource="http://postdata.linhd.uned.es/ontology/postdata-core#Place"/>
            </owl:Restriction>
        </rdfs:subClassOf>
        <rdfs:subClassOf>
            <owl:Restriction>
                <owl:onProperty rdf:resource="http://postdata.linhd.uned.es/ontology/postdata-core#birthPlaceCertainty"/>
                <owl:allValuesFrom>
                    <owl:Class>
                        <owl:intersectionOf rdf:parseType="Collection">
                            <rdf:Description rdf:about="http://www.w3.org/2004/02/skos/core#Concept"/>
                            <owl:Restriction>
                                <owl:onProperty rdf:resource="http://www.w3.org/2004/02/skos/core#inScheme"/>
                                <owl:hasValue rdf:resource="http://postdata.linhd.uned.es/kos/certainty"/>
                            </owl:Restriction>
                        </owl:intersectionOf>
                    </owl:Class>
                </owl:allValuesFrom>
            </owl:Restriction>
        </rdfs:subClassOf>
        <rdfs:subClassOf>
            <owl:Restriction>
                <owl:onProperty rdf:resource="http://postdata.linhd.uned.es/ontology/postdata-core#deathDate"/>
                <owl:allValuesFrom rdf:resource="http://postdata.linhd.uned.es/ontology/postdata-dates#DateEntity"/>
            </owl:Restriction>
        </rdfs:subClassOf>
        <rdfs:subClassOf>
            <owl:Restriction>
                <owl:onProperty rdf:resource="http://postdata.linhd.uned.es/ontology/postdata-core#floruit"/>
                <owl:allValuesFrom rdf:resource="http://postdata.linhd.uned.es/ontology/postdata-dates#DateEntity"/>
            </owl:Restriction>
        </rdfs:subClassOf>
        <rdfs:subClassOf>
            <owl:Restriction>
                <owl:onProperty rdf:resource="http://postdata.linhd.uned.es/ontology/postdata-core#isMentionedIn"/>
                <owl:allValuesFrom rdf:resource="http://postdata.linhd.uned.es/ontology/postdata-core#Redaction"/>
            </owl:Restriction>
        </rdfs:subClassOf>
        <rdfs:subClassOf>
            <owl:Restriction>
                <owl:onProperty rdf:resource="http://postdata.linhd.uned.es/ontology/postdata-core#isReferencedIn"/>
                <owl:allValuesFrom rdf:resource="http://postdata.linhd.uned.es/ontology/postdata-transmission#Location"/>
            </owl:Restriction>
        </rdfs:subClassOf>
        <rdfs:subClassOf>
            <owl:Restriction>
                <owl:onProperty rdf:resource="http://postdata.linhd.uned.es/ontology/postdata-core#literaryPeriod"/>
                <owl:allValuesFrom>
                    <owl:Class>
                        <owl:intersectionOf rdf:parseType="Collection">
                            <rdf:Description rdf:about="http://www.w3.org/2004/02/skos/core#Concept"/>
                            <owl:Restriction>
                                <owl:onProperty rdf:resource="http://www.w3.org/2004/02/skos/core#inScheme"/>
                                <owl:hasValue rdf:resource="http://postdata.linhd.uned.es/kos/literary-period"/>
                            </owl:Restriction>
                        </owl:intersectionOf>
                    </owl:Class>
                </owl:allValuesFrom>
            </owl:Restriction>
        </rdfs:subClassOf>
        <rdfs:subClassOf>
            <owl:Restriction>
                <owl:onProperty rdf:resource="http://postdata.linhd.uned.es/ontology/postdata-core#religiousAffiliation"/>
                <owl:allValuesFrom>
                    <owl:Class>
                        <owl:intersectionOf rdf:parseType="Collection">
                            <rdf:Description rdf:about="http://www.w3.org/2004/02/skos/core#Concept"/>
                            <owl:Restriction>
                                <owl:onProperty rdf:resource="http://www.w3.org/2004/02/skos/core#inScheme"/>
                                <owl:hasValue rdf:resource="http://postdata.linhd.uned.es/kos/religious-affiliation"/>
                            </owl:Restriction>
                        </owl:intersectionOf>
                    </owl:Class>
                </owl:allValuesFrom>
            </owl:Restriction>
        </rdfs:subClassOf>
        <rdfs:subClassOf>
            <owl:Restriction>
                <owl:onProperty rdf:resource="http://postdata.linhd.uned.es/ontology/postdata-core#socialStatus"/>
                <owl:allValuesFrom>
                    <owl:Class>
                        <owl:intersectionOf rdf:parseType="Collection">
                            <rdf:Description rdf:about="http://www.w3.org/2004/02/skos/core#Concept"/>
                            <owl:Restriction>
                                <owl:onProperty rdf:resource="http://www.w3.org/2004/02/skos/core#inScheme"/>
                                <owl:hasValue rdf:resource="http://postdata.linhd.uned.es/kos/social-status"/>
                            </owl:Restriction>
                        </owl:intersectionOf>
                    </owl:Class>
                </owl:allValuesFrom>
            </owl:Restriction>
        </rdfs:subClassOf>
        <rdfs:subClassOf>
            <owl:Restriction>
                <owl:onProperty rdf:resource="http://postdata.linhd.uned.es/ontology/postdata-core#gender"/>
                <owl:qualifiedCardinality rdf:datatype="http://www.w3.org/2001/XMLSchema#nonNegativeInteger">1</owl:qualifiedCardinality>
                <owl:onClass>
                    <owl:Class>
                        <owl:intersectionOf rdf:parseType="Collection">
                            <rdf:Description rdf:about="http://www.w3.org/2004/02/skos/core#Concept"/>
                            <owl:Restriction>
                                <owl:onProperty rdf:resource="http://www.w3.org/2004/02/skos/core#inScheme"/>
                                <owl:hasValue rdf:resource="http://postdata.linhd.uned.es/kos/gender"/>
                            </owl:Restriction>
                        </owl:intersectionOf>
                    </owl:Class>
                </owl:onClass>
            </owl:Restriction>
        </rdfs:subClassOf>
        <rdfs:subClassOf>
            <owl:Restriction>
                <owl:onProperty rdf:resource="http://postdata.linhd.uned.es/ontology/postdata-core#birthPlaceCertainty"/>
                <owl:maxQualifiedCardinality rdf:datatype="http://www.w3.org/2001/XMLSchema#nonNegativeInteger">1</owl:maxQualifiedCardinality>
                <owl:onClass>
                    <owl:Class>
                        <owl:intersectionOf rdf:parseType="Collection">
                            <rdf:Description rdf:about="http://www.w3.org/2004/02/skos/core#Concept"/>
                            <owl:Restriction>
                                <owl:onProperty rdf:resource="http://www.w3.org/2004/02/skos/core#inScheme"/>
                                <owl:hasValue rdf:resource="http://postdata.linhd.uned.es/kos/certainty"/>
                            </owl:Restriction>
                        </owl:intersectionOf>
                    </owl:Class>
                </owl:onClass>
            </owl:Restriction>
        </rdfs:subClassOf>
        <rdfs:subClassOf>
            <owl:Restriction>
                <owl:onProperty rdf:resource="http://postdata.linhd.uned.es/ontology/postdata-core#forename"/>
                <owl:maxQualifiedCardinality rdf:datatype="http://www.w3.org/2001/XMLSchema#nonNegativeInteger">1</owl:maxQualifiedCardinality>
                <owl:onDataRange rdf:resource="http://www.w3.org/2001/XMLSchema#string"/>
            </owl:Restriction>
        </rdfs:subClassOf>
        <rdfs:subClassOf>
            <owl:Restriction>
                <owl:onProperty rdf:resource="http://postdata.linhd.uned.es/ontology/postdata-core#nameLink"/>
                <owl:maxQualifiedCardinality rdf:datatype="http://www.w3.org/2001/XMLSchema#nonNegativeInteger">1</owl:maxQualifiedCardinality>
                <owl:onDataRange rdf:resource="http://www.w3.org/2001/XMLSchema#string"/>
            </owl:Restriction>
        </rdfs:subClassOf>
        <rdfs:subClassOf>
            <owl:Restriction>
                <owl:onProperty rdf:resource="http://postdata.linhd.uned.es/ontology/postdata-core#originalName"/>
                <owl:maxQualifiedCardinality rdf:datatype="http://www.w3.org/2001/XMLSchema#nonNegativeInteger">1</owl:maxQualifiedCardinality>
                <owl:onDataRange rdf:resource="http://www.w3.org/2001/XMLSchema#string"/>
            </owl:Restriction>
        </rdfs:subClassOf>
        <rdfs:subClassOf>
            <owl:Restriction>
                <owl:onProperty rdf:resource="http://postdata.linhd.uned.es/ontology/postdata-core#surname"/>
                <owl:maxQualifiedCardinality rdf:datatype="http://www.w3.org/2001/XMLSchema#nonNegativeInteger">1</owl:maxQualifiedCardinality>
                <owl:onDataRange rdf:resource="http://www.w3.org/2001/XMLSchema#string"/>
            </owl:Restriction>
        </rdfs:subClassOf>
        <rdfs:comment xml:lang="en">A human being regarded as an individual. This person may have existed in real life (e.g., Miguel de Cervantes) or may be fictional (e.g., Don Quijote de la Mancha).

This class is defined as subclass of pdcore:Agent, and it is based on CIDOC CRM E21 Person class.</rdfs:comment>
        <rdfs:isDefinedBy>http://postdata.linhd.uned.es/ontology/postdata-core/</rdfs:isDefinedBy>
        <rdfs:label xml:lang="en">Person</rdfs:label>
    </owl:Class>
    


    <!-- http://postdata.linhd.uned.es/ontology/postdata-core#Place -->

    <owl:Class rdf:about="http://postdata.linhd.uned.es/ontology/postdata-core#Place">
        <rdfs:subClassOf>
            <owl:Restriction>
                <owl:onProperty rdf:resource="http://postdata.linhd.uned.es/ontology/postdata-core#date"/>
                <owl:allValuesFrom rdf:resource="http://postdata.linhd.uned.es/ontology/postdata-dates#DateEntity"/>
            </owl:Restriction>
        </rdfs:subClassOf>
        <rdfs:subClassOf>
            <owl:Restriction>
                <owl:onProperty rdf:resource="http://postdata.linhd.uned.es/ontology/postdata-core#isMentionedIn"/>
                <owl:allValuesFrom rdf:resource="http://postdata.linhd.uned.es/ontology/postdata-core#Redaction"/>
            </owl:Restriction>
        </rdfs:subClassOf>
        <rdfs:subClassOf>
            <owl:Restriction>
                <owl:onProperty rdf:resource="http://postdata.linhd.uned.es/ontology/postdata-core#originalName"/>
                <owl:maxQualifiedCardinality rdf:datatype="http://www.w3.org/2001/XMLSchema#nonNegativeInteger">1</owl:maxQualifiedCardinality>
                <owl:onDataRange rdf:resource="http://www.w3.org/2001/XMLSchema#string"/>
            </owl:Restriction>
        </rdfs:subClassOf>
        <rdfs:comment xml:lang="en">A particular position, point, or area in space; a location
This class is defined as a subclass of edm:Place. In the future, it may be also defined as a subclass of schema:Place and geonames:Feature, so as to facilitate linking with existing entities already defined according to schema.org or available in the GeoNames knowledge graph.

This class is based on CIDOC CRM E53 Place Class.</rdfs:comment>
        <rdfs:isDefinedBy>http://postdata.linhd.uned.es/ontology/postdata-core/</rdfs:isDefinedBy>
        <rdfs:label xml:lang="en">Place</rdfs:label>
    </owl:Class>
    


    <!-- http://postdata.linhd.uned.es/ontology/postdata-core#PoeticWork -->

    <owl:Class rdf:about="http://postdata.linhd.uned.es/ontology/postdata-core#PoeticWork">
        <rdfs:subClassOf rdf:resource="http://iflastandards.info/ns/fr/frbr/frbroo/F1"/>
        <rdfs:subClassOf rdf:resource="http://www.europeana.eu/schemas/edm/ProvidedCHO"/>
        <rdfs:subClassOf>
            <owl:Restriction>
                <owl:onProperty rdf:resource="http://postdata.linhd.uned.es/ontology/postdata-core#authorEducationLevel"/>
                <owl:allValuesFrom>
                    <owl:Class>
                        <owl:intersectionOf rdf:parseType="Collection">
                            <rdf:Description rdf:about="http://www.w3.org/2004/02/skos/core#Concept"/>
                            <owl:Restriction>
                                <owl:onProperty rdf:resource="http://www.w3.org/2004/02/skos/core#inScheme"/>
                                <owl:hasValue rdf:resource="http://postdata.linhd.uned.es/kos/education-level"/>
                            </owl:Restriction>
                        </owl:intersectionOf>
                    </owl:Class>
                </owl:allValuesFrom>
            </owl:Restriction>
        </rdfs:subClassOf>
        <rdfs:subClassOf>
            <owl:Restriction>
                <owl:onProperty rdf:resource="http://postdata.linhd.uned.es/ontology/postdata-core#date"/>
                <owl:allValuesFrom rdf:resource="http://postdata.linhd.uned.es/ontology/postdata-dates#DateEntity"/>
            </owl:Restriction>
        </rdfs:subClassOf>
        <rdfs:subClassOf>
            <owl:Restriction>
                <owl:onProperty rdf:resource="http://postdata.linhd.uned.es/ontology/postdata-core#genre"/>
                <owl:allValuesFrom>
                    <owl:Class>
                        <owl:intersectionOf rdf:parseType="Collection">
                            <rdf:Description rdf:about="http://www.w3.org/2004/02/skos/core#Concept"/>
                            <owl:Restriction>
                                <owl:onProperty rdf:resource="http://www.w3.org/2004/02/skos/core#inScheme"/>
                                <owl:hasValue rdf:resource="http://postdata.linhd.uned.es/kos/genre"/>
                            </owl:Restriction>
                        </owl:intersectionOf>
                    </owl:Class>
                </owl:allValuesFrom>
            </owl:Restriction>
        </rdfs:subClassOf>
        <rdfs:subClassOf>
            <owl:Restriction>
                <owl:onProperty rdf:resource="http://postdata.linhd.uned.es/ontology/postdata-core#isReferencedIn"/>
                <owl:allValuesFrom rdf:resource="http://postdata.linhd.uned.es/ontology/postdata-transmission#Location"/>
            </owl:Restriction>
        </rdfs:subClassOf>
        <rdfs:subClassOf>
            <owl:Restriction>
                <owl:onProperty rdf:resource="http://postdata.linhd.uned.es/ontology/postdata-core#poeticType"/>
                <owl:allValuesFrom>
                    <owl:Class>
                        <owl:intersectionOf rdf:parseType="Collection">
                            <rdf:Description rdf:about="http://www.w3.org/2004/02/skos/core#Concept"/>
                            <owl:Restriction>
                                <owl:onProperty rdf:resource="http://www.w3.org/2004/02/skos/core#inScheme"/>
                                <owl:hasValue rdf:resource="http://postdata.linhd.uned.es/kos/poetic-type"/>
                            </owl:Restriction>
                        </owl:intersectionOf>
                    </owl:Class>
                </owl:allValuesFrom>
            </owl:Restriction>
        </rdfs:subClassOf>
        <rdfs:subClassOf>
            <owl:Restriction>
                <owl:onProperty rdf:resource="http://postdata.linhd.uned.es/ontology/postdata-core#date"/>
                <owl:qualifiedCardinality rdf:datatype="http://www.w3.org/2001/XMLSchema#nonNegativeInteger">1</owl:qualifiedCardinality>
                <owl:onClass rdf:resource="http://postdata.linhd.uned.es/ontology/postdata-dates#DateEntity"/>
            </owl:Restriction>
        </rdfs:subClassOf>
        <rdfs:subClassOf>
            <owl:Restriction>
                <owl:onProperty rdf:resource="http://postdata.linhd.uned.es/ontology/postdata-core#hasProvenance"/>
                <owl:maxQualifiedCardinality rdf:datatype="http://www.w3.org/2001/XMLSchema#nonNegativeInteger">1</owl:maxQualifiedCardinality>
                <owl:onClass rdf:resource="http://postdata.linhd.uned.es/ontology/postdata-core#Place"/>
            </owl:Restriction>
        </rdfs:subClassOf>
        <rdfs:subClassOf>
            <owl:Restriction>
                <owl:onProperty rdf:resource="http://postdata.linhd.uned.es/ontology/postdata-core#narrativeLocation"/>
                <owl:maxQualifiedCardinality rdf:datatype="http://www.w3.org/2001/XMLSchema#nonNegativeInteger">1</owl:maxQualifiedCardinality>
                <owl:onDataRange rdf:resource="http://www.w3.org/2001/XMLSchema#string"/>
            </owl:Restriction>
        </rdfs:subClassOf>
        <rdfs:subClassOf>
            <owl:Restriction>
                <owl:onProperty rdf:resource="http://postdata.linhd.uned.es/ontology/postdata-core#originalTitle"/>
                <owl:maxQualifiedCardinality rdf:datatype="http://www.w3.org/2001/XMLSchema#nonNegativeInteger">1</owl:maxQualifiedCardinality>
                <owl:onDataRange rdf:resource="http://www.w3.org/2001/XMLSchema#string"/>
            </owl:Restriction>
        </rdfs:subClassOf>
        <rdfs:comment xml:lang="en">Abstract concept of an artistic creation. In the POSTDATA ontology network these creations must be in verse (e.g., poem, play, song). For example, Os Lusíadas by Luis Vaz de Camões; La Commedia by Dante; the poem Ad te deus by an Anonymous author written in between the 7th and 9th centuries.

This class is based on CIDOC FRBR F1 Work Class and it is aligned with edm:ProvidedCHO Class.</rdfs:comment>
        <rdfs:isDefinedBy>http://postdata.linhd.uned.es/ontology/postdata-core/</rdfs:isDefinedBy>
        <rdfs:label xml:lang="en">Poetic Work</rdfs:label>
    </owl:Class>
    


    <!-- http://postdata.linhd.uned.es/ontology/postdata-core#Redaction -->

    <owl:Class rdf:about="http://postdata.linhd.uned.es/ontology/postdata-core#Redaction">
        <rdfs:subClassOf rdf:resource="http://iflastandards.info/ns/fr/frbr/frbroo/F22"/>
        <rdfs:subClassOf rdf:resource="http://www.openarchives.org/ore/terms/Aggregation"/>
        <rdfs:subClassOf>
            <owl:Restriction>
                <owl:onProperty rdf:resource="http://postdata.linhd.uned.es/ontology/postdata-core#date"/>
                <owl:allValuesFrom rdf:resource="http://postdata.linhd.uned.es/ontology/postdata-dates#DateEntity"/>
            </owl:Restriction>
        </rdfs:subClassOf>
        <rdfs:subClassOf>
            <owl:Restriction>
                <owl:onProperty rdf:resource="http://postdata.linhd.uned.es/ontology/postdata-core#editedIn"/>
                <owl:allValuesFrom rdf:resource="http://postdata.linhd.uned.es/ontology/postdata-transmission#Location"/>
            </owl:Restriction>
        </rdfs:subClassOf>
        <rdfs:subClassOf>
            <owl:Restriction>
                <owl:onProperty rdf:resource="http://postdata.linhd.uned.es/ontology/postdata-core#genre"/>
                <owl:allValuesFrom>
                    <owl:Class>
                        <owl:intersectionOf rdf:parseType="Collection">
                            <rdf:Description rdf:about="http://www.w3.org/2004/02/skos/core#Concept"/>
                            <owl:Restriction>
                                <owl:onProperty rdf:resource="http://www.w3.org/2004/02/skos/core#inScheme"/>
                                <owl:hasValue rdf:resource="http://postdata.linhd.uned.es/kos/genre"/>
                            </owl:Restriction>
                        </owl:intersectionOf>
                    </owl:Class>
                </owl:allValuesFrom>
            </owl:Restriction>
        </rdfs:subClassOf>
        <rdfs:subClassOf>
            <owl:Restriction>
                <owl:onProperty rdf:resource="http://postdata.linhd.uned.es/ontology/postdata-core#hasOrderedTextUnitList"/>
                <owl:allValuesFrom rdf:resource="http://postdata.linhd.uned.es/ontology/postdata-structuralElements#OrderedTextUnitList"/>
            </owl:Restriction>
        </rdfs:subClassOf>
        <rdfs:subClassOf>
            <owl:Restriction>
                <owl:onProperty rdf:resource="http://postdata.linhd.uned.es/ontology/postdata-core#hasSynthesis"/>
                <owl:allValuesFrom rdf:resource="http://postdata.linhd.uned.es/ontology/postdata-core#Redaction"/>
            </owl:Restriction>
        </rdfs:subClassOf>
        <rdfs:subClassOf>
            <owl:Restriction>
                <owl:onProperty rdf:resource="http://postdata.linhd.uned.es/ontology/postdata-core#hasTranslation"/>
                <owl:allValuesFrom>
                    <owl:Class>
                        <owl:unionOf rdf:parseType="Collection">
                            <rdf:Description rdf:about="http://postdata.linhd.uned.es/ontology/postdata-core#Redaction"/>
                            <rdf:Description rdf:about="http://postdata.linhd.uned.es/ontology/postdata-transmission#Location"/>
                        </owl:unionOf>
                    </owl:Class>
                </owl:allValuesFrom>
            </owl:Restriction>
        </rdfs:subClassOf>
        <rdfs:subClassOf>
            <owl:Restriction>
                <owl:onProperty rdf:resource="http://postdata.linhd.uned.es/ontology/postdata-core#isIndexedIn"/>
                <owl:allValuesFrom rdf:resource="http://postdata.linhd.uned.es/ontology/postdata-transmission#Location"/>
            </owl:Restriction>
        </rdfs:subClassOf>
        <rdfs:subClassOf>
            <owl:Restriction>
                <owl:onProperty rdf:resource="http://postdata.linhd.uned.es/ontology/postdata-core#isReferencedIn"/>
                <owl:allValuesFrom rdf:resource="http://postdata.linhd.uned.es/ontology/postdata-transmission#Location"/>
            </owl:Restriction>
        </rdfs:subClassOf>
        <rdfs:subClassOf>
            <owl:Restriction>
                <owl:onProperty rdf:resource="http://postdata.linhd.uned.es/ontology/postdata-core#isSynthesisOf"/>
                <owl:allValuesFrom rdf:resource="http://postdata.linhd.uned.es/ontology/postdata-core#Redaction"/>
            </owl:Restriction>
        </rdfs:subClassOf>
        <rdfs:subClassOf>
            <owl:Restriction>
                <owl:onProperty rdf:resource="http://postdata.linhd.uned.es/ontology/postdata-core#isTranslationOf"/>
                <owl:allValuesFrom rdf:resource="http://postdata.linhd.uned.es/ontology/postdata-core#Redaction"/>
            </owl:Restriction>
        </rdfs:subClassOf>
        <rdfs:subClassOf>
            <owl:Restriction>
                <owl:onProperty rdf:resource="http://postdata.linhd.uned.es/ontology/postdata-core#retrievesText"/>
                <owl:allValuesFrom rdf:resource="http://postdata.linhd.uned.es/ontology/postdata-transmission#Location"/>
            </owl:Restriction>
        </rdfs:subClassOf>
        <rdfs:subClassOf>
            <owl:Restriction>
                <owl:onProperty rdf:resource="http://postdata.linhd.uned.es/ontology/postdata-core#typeOfTextualElement"/>
                <owl:allValuesFrom>
                    <owl:Class>
                        <owl:intersectionOf rdf:parseType="Collection">
                            <rdf:Description rdf:about="http://www.w3.org/2004/02/skos/core#Concept"/>
                            <owl:Restriction>
                                <owl:onProperty rdf:resource="http://www.w3.org/2004/02/skos/core#inScheme"/>
                                <owl:hasValue rdf:resource="http://postdata.linhd.uned.es/kos/textual-element-type"/>
                            </owl:Restriction>
                        </owl:intersectionOf>
                    </owl:Class>
                </owl:allValuesFrom>
            </owl:Restriction>
        </rdfs:subClassOf>
        <rdfs:subClassOf>
            <owl:Restriction>
                <owl:onProperty rdf:resource="http://postdata.linhd.uned.es/ontology/postdata-core#isTranslationOf"/>
                <owl:maxQualifiedCardinality rdf:datatype="http://www.w3.org/2001/XMLSchema#nonNegativeInteger">1</owl:maxQualifiedCardinality>
                <owl:onClass rdf:resource="http://postdata.linhd.uned.es/ontology/postdata-core#Redaction"/>
            </owl:Restriction>
        </rdfs:subClassOf>
        <rdfs:subClassOf>
            <owl:Restriction>
                <owl:onProperty rdf:resource="http://postdata.linhd.uned.es/ontology/postdata-core#realises"/>
                <owl:maxQualifiedCardinality rdf:datatype="http://www.w3.org/2001/XMLSchema#nonNegativeInteger">1</owl:maxQualifiedCardinality>
                <owl:onClass rdf:resource="http://postdata.linhd.uned.es/ontology/postdata-core#PoeticWork"/>
            </owl:Restriction>
        </rdfs:subClassOf>
        <rdfs:subClassOf>
            <owl:Restriction>
                <owl:onProperty rdf:resource="http://postdata.linhd.uned.es/ontology/postdata-core#audience"/>
                <owl:maxCardinality rdf:datatype="http://www.w3.org/2001/XMLSchema#nonNegativeInteger">1</owl:maxCardinality>
            </owl:Restriction>
        </rdfs:subClassOf>
        <rdfs:subClassOf>
            <owl:Restriction>
                <owl:onProperty rdf:resource="http://postdata.linhd.uned.es/ontology/postdata-core#explicit"/>
                <owl:maxQualifiedCardinality rdf:datatype="http://www.w3.org/2001/XMLSchema#nonNegativeInteger">1</owl:maxQualifiedCardinality>
                <owl:onDataRange rdf:resource="http://www.w3.org/2001/XMLSchema#string"/>
            </owl:Restriction>
        </rdfs:subClassOf>
        <rdfs:subClassOf>
            <owl:Restriction>
                <owl:onProperty rdf:resource="http://postdata.linhd.uned.es/ontology/postdata-core#incipit"/>
                <owl:maxCardinality rdf:datatype="http://www.w3.org/2001/XMLSchema#nonNegativeInteger">1</owl:maxCardinality>
            </owl:Restriction>
        </rdfs:subClassOf>
        <rdfs:subClassOf>
            <owl:Restriction>
                <owl:onProperty rdf:resource="http://postdata.linhd.uned.es/ontology/postdata-core#narrativeLocation"/>
                <owl:maxQualifiedCardinality rdf:datatype="http://www.w3.org/2001/XMLSchema#nonNegativeInteger">1</owl:maxQualifiedCardinality>
                <owl:onDataRange rdf:resource="http://www.w3.org/2001/XMLSchema#string"/>
            </owl:Restriction>
        </rdfs:subClassOf>
        <rdfs:subClassOf>
            <owl:Restriction>
                <owl:onProperty rdf:resource="http://postdata.linhd.uned.es/ontology/postdata-core#numberOfWitnessesUsed"/>
                <owl:maxQualifiedCardinality rdf:datatype="http://www.w3.org/2001/XMLSchema#nonNegativeInteger">1</owl:maxQualifiedCardinality>
                <owl:onDataRange rdf:resource="http://www.w3.org/2001/XMLSchema#integer"/>
            </owl:Restriction>
        </rdfs:subClassOf>
        <rdfs:subClassOf>
            <owl:Restriction>
                <owl:onProperty rdf:resource="http://postdata.linhd.uned.es/ontology/postdata-core#originalLanguage"/>
                <owl:maxQualifiedCardinality rdf:datatype="http://www.w3.org/2001/XMLSchema#nonNegativeInteger">1</owl:maxQualifiedCardinality>
                <owl:onDataRange>
                    <rdfs:Datatype>
                        <owl:unionOf rdf:parseType="Collection">
                            <rdf:Description rdf:about="http://www.w3.org/2001/XMLSchema#language"/>
                            <rdf:Description rdf:about="http://www.w3.org/2001/XMLSchema#string"/>
                        </owl:unionOf>
                    </rdfs:Datatype>
                </owl:onDataRange>
            </owl:Restriction>
        </rdfs:subClassOf>
        <rdfs:subClassOf>
            <owl:Restriction>
                <owl:onProperty rdf:resource="http://postdata.linhd.uned.es/ontology/postdata-core#originalTitle"/>
                <owl:maxQualifiedCardinality rdf:datatype="http://www.w3.org/2001/XMLSchema#nonNegativeInteger">1</owl:maxQualifiedCardinality>
                <owl:onDataRange rdf:resource="http://www.w3.org/2001/XMLSchema#string"/>
            </owl:Restriction>
        </rdfs:subClassOf>
        <rdfs:subClassOf>
            <owl:Restriction>
                <owl:onProperty rdf:resource="http://postdata.linhd.uned.es/ontology/postdata-core#paraphrasis"/>
                <owl:maxQualifiedCardinality rdf:datatype="http://www.w3.org/2001/XMLSchema#nonNegativeInteger">1</owl:maxQualifiedCardinality>
                <owl:onDataRange rdf:resource="http://www.w3.org/2001/XMLSchema#string"/>
            </owl:Restriction>
        </rdfs:subClassOf>
        <rdfs:subClassOf>
            <owl:Restriction>
                <owl:onProperty rdf:resource="http://postdata.linhd.uned.es/ontology/postdata-core#text"/>
                <owl:maxQualifiedCardinality rdf:datatype="http://www.w3.org/2001/XMLSchema#nonNegativeInteger">1</owl:maxQualifiedCardinality>
                <owl:onDataRange rdf:resource="http://www.w3.org/2001/XMLSchema#string"/>
            </owl:Restriction>
        </rdfs:subClassOf>
        <rdfs:subClassOf>
            <owl:Restriction>
                <owl:onProperty rdf:resource="http://postdata.linhd.uned.es/ontology/postdata-core#workNumber"/>
                <owl:maxQualifiedCardinality rdf:datatype="http://www.w3.org/2001/XMLSchema#nonNegativeInteger">1</owl:maxQualifiedCardinality>
                <owl:onDataRange rdf:resource="http://www.w3.org/2001/XMLSchema#string"/>
            </owl:Restriction>
        </rdfs:subClassOf>
        <rdfs:comment xml:lang="en">Representatives of a work, that is, of a Poetic Work. Each version and edition of a work is its own redaction.
Eg.: The palaeographic edition of A solis ortu usque ad occidua preserved in Lat. 1154 (BNF) and its critical edition are two Redaction of the same Poetic Work.

This class is based on FRBR F22 Self Contained Expression and it is aligned with ore:Aggregation to keep alignment with Europeana Data Model.</rdfs:comment>
        <rdfs:isDefinedBy>http://postdata.linhd.uned.es/ontology/postdata-core/</rdfs:isDefinedBy>
        <rdfs:label xml:lang="en">Redaction</rdfs:label>
    </owl:Class>
    


    <!-- http://postdata.linhd.uned.es/ontology/postdata-dates#DateEntity -->

    <owl:Class rdf:about="http://postdata.linhd.uned.es/ontology/postdata-dates#DateEntity">
        <rdfs:comment xml:lang="en">The temporal entity asociated to an opus, manifestation, event..</rdfs:comment>
        <rdfs:isDefinedBy>http://postdata.linhd.uned.es/ontology/postdata-dates</rdfs:isDefinedBy>
        <rdfs:label xml:lang="en">DateEntity</rdfs:label>
    </owl:Class>
    


    <!-- http://postdata.linhd.uned.es/ontology/postdata-structuralElements#OrderedTextUnitList -->

    <owl:Class rdf:about="http://postdata.linhd.uned.es/ontology/postdata-structuralElements#OrderedTextUnitList">
        <rdfs:comment xml:lang="en">An ordered list of text units with a given length and indexed elements. Examples of these lists are the list of stanzas and the list of lines, associated to a Redaction.

This class emerges by reusing the Ordered List Ontology Design Pattern:
- http://purl.org/ontology/olo/core</rdfs:comment>
        <rdfs:isDefinedBy>http://postdata.linhd.uned.es/ontology/postdata-core/</rdfs:isDefinedBy>
        <rdfs:label xml:lang="en">Ordered Text Unit List</rdfs:label>
    </owl:Class>
    


    <!-- http://postdata.linhd.uned.es/ontology/postdata-transmission#Location -->

    <owl:Class rdf:about="http://postdata.linhd.uned.es/ontology/postdata-transmission#Location">
        <rdfs:comment xml:lang="en">The particular position of a piece of information in a text</rdfs:comment>
        <rdfs:isDefinedBy xml:lang="en">http://postdata.linhd.uned.es/ontology/postdata-transmission</rdfs:isDefinedBy>
        <rdfs:label xml:lang="en">Location</rdfs:label>
    </owl:Class>
    


    <!-- http://www.europeana.eu/schemas/edm/ProvidedCHO -->

    <owl:Class rdf:about="http://www.europeana.eu/schemas/edm/ProvidedCHO">
        <rdfs:subClassOf>
            <owl:Restriction>
                <owl:onProperty>
                    <rdf:Description>
                        <owl:inverseOf rdf:resource="http://www.europeana.eu/schemas/edm/aggregatedCHO"/>
                    </rdf:Description>
                </owl:onProperty>
                <owl:cardinality rdf:datatype="http://www.w3.org/2001/XMLSchema#nonNegativeInteger">1</owl:cardinality>
            </owl:Restriction>
        </rdfs:subClassOf>
        <rdfs:label xml:lang="en">Provided CHO</rdfs:label>
        <skos:definition xml:lang="en">This class comprises the Cultural Heritage objects that Europeana collects descriptions about.</skos:definition>
        <skos:example xml:lang="en">Mona Lisa, Winged Victory of Samothrace</skos:example>
        <skos:note xml:lang="en">This class has been mostly motivated by the need to assign a type to the “central node” in the EDM pattern, during the ingestion process, related to the XML expression of EDM at that stage. It was especially intended to fit the cases where edm:PhysicalThing  cannot be used as the type of the resource standing for the real-world object (independently of any specific data contributor perspective).</skos:note>
        <skos:scopeNote xml:lang="en">Rationale: This class is the range of edm:aggregatedCHO. A resource of type ProvidedCHO can be the subject of statements using edm:isRelatedTo or any more specific property.</skos:scopeNote>
    </owl:Class>
    


    <!-- http://www.openarchives.org/ore/terms/Aggregation -->

    <owl:Class rdf:about="http://www.openarchives.org/ore/terms/Aggregation">
        <rdfs:comment xml:lang="en">A set of related resources (Aggregated Resources), grouped together such that the set can be treated as a single resource. This is the entity described within the ORE interoperability framework by a Resource Map.</rdfs:comment>
        <rdfs:isDefinedBy>http://www.openarchives.org/ore/terms/</rdfs:isDefinedBy>
        <rdfs:label xml:lang="en">Aggregation</rdfs:label>
    </owl:Class>
    


    <!-- http://www.w3.org/2002/07/owl#Thing -->

    <rdf:Description rdf:about="http://www.w3.org/2002/07/owl#Thing">
        <rdfs:label>Thing</rdfs:label>
    </rdf:Description>
    


    <!-- http://www.w3.org/2004/02/skos/core#Concept -->

    <owl:Class rdf:about="http://www.w3.org/2004/02/skos/core#Concept">
        <owl:disjointWith rdf:resource="http://www.w3.org/2004/02/skos/core#ConceptScheme"/>
        <rdfs:isDefinedBy rdf:resource="http://www.w3.org/2004/02/skos/core"/>
        <rdfs:label>Concept</rdfs:label>
        <rdfs:label xml:lang="en">Concept</rdfs:label>
        <skos:definition xml:lang="en">An idea or notion; a unit of thought.</skos:definition>
    </owl:Class>
    


    <!-- http://www.w3.org/2004/02/skos/core#ConceptScheme -->

    <owl:Class rdf:about="http://www.w3.org/2004/02/skos/core#ConceptScheme">
        <rdfs:isDefinedBy rdf:resource="http://www.w3.org/2004/02/skos/core"/>
        <rdfs:label xml:lang="en">Concept Scheme</rdfs:label>
        <skos:definition xml:lang="en">A set of concepts, optionally including statements about semantic relationships between those concepts.</skos:definition>
        <skos:example xml:lang="en">Thesauri, classification schemes, subject heading lists, taxonomies, &apos;folksonomies&apos;, and other types of controlled vocabulary are all examples of concept schemes. Concept schemes are also embedded in glossaries and terminologies.</skos:example>
        <skos:scopeNote xml:lang="en">A concept scheme may be defined to include concepts from different sources.</skos:scopeNote>
    </owl:Class>
    


    <!-- 
    ///////////////////////////////////////////////////////////////////////////////////////
    //
    // Individuals
    //
    ///////////////////////////////////////////////////////////////////////////////////////
     -->

    


    <!-- http://iflastandards.info/ns/fr/frbr/frbroo/F1 -->

    <owl:NamedIndividual rdf:about="http://iflastandards.info/ns/fr/frbr/frbroo/F1"/>
    


    <!-- http://iflastandards.info/ns/fr/frbr/frbroo/F14 -->

    <owl:NamedIndividual rdf:about="http://iflastandards.info/ns/fr/frbr/frbroo/F14"/>
    


    <!-- http://iflastandards.info/ns/fr/frbr/frbroo/F17 -->

    <owl:NamedIndividual rdf:about="http://iflastandards.info/ns/fr/frbr/frbroo/F17"/>
    


    <!-- http://iflastandards.info/ns/fr/frbr/frbroo/F2 -->

    <owl:NamedIndividual rdf:about="http://iflastandards.info/ns/fr/frbr/frbroo/F2"/>
    


    <!-- http://iflastandards.info/ns/fr/frbr/frbroo/F22 -->

    <owl:NamedIndividual rdf:about="http://iflastandards.info/ns/fr/frbr/frbroo/F22"/>
    


    <!-- http://postdata.linhd.uned.es/kos/certainty -->

    <owl:NamedIndividual rdf:about="http://postdata.linhd.uned.es/kos/certainty">
        <rdf:type rdf:resource="http://www.w3.org/2004/02/skos/core#ConceptScheme"/>
        <dc:creator xml:lang="en">POSTDATA Project “This project has received funding from the European Research Council (ERC) under the European Union’s Horizon 2020 research and innovation programme (grant agreement Nº [679528])”</dc:creator>
        <terms:date rdf:datatype="http://www.w3.org/2001/XMLSchema#date">2019-05-22</terms:date>
        <terms:title xml:lang="en">Controlled vocabulary about certainty degree</terms:title>
        <terms:title xml:lang="es">Vocabulario controlado sobre grados de certeza</terms:title>
        <skos:definition xml:lang="en">Controlled vocabulary about certainty degree</skos:definition>
        <skos:hasTopConcept rdf:resource="http://postdata.linhd.uned.es/kos/certainty/definitely"/>
        <skos:hasTopConcept rdf:resource="http://postdata.linhd.uned.es/kos/certainty/definitely-not"/>
        <skos:hasTopConcept rdf:resource="http://postdata.linhd.uned.es/kos/certainty/possibily"/>
        <skos:hasTopConcept rdf:resource="http://postdata.linhd.uned.es/kos/certainty/probably"/>
        <skos:hasTopConcept rdf:resource="http://postdata.linhd.uned.es/kos/certainty/probably-not"/>
        <skos:prefLabel xml:lang="en">Certainty Scheme</skos:prefLabel>
        <prov:wasAttributedTo rdf:resource="https://www.linkedin.com/in/m-luisa-diez-platas-05710614"/>
    </owl:NamedIndividual>
    


    <!-- http://postdata.linhd.uned.es/kos/character-type -->

    <owl:NamedIndividual rdf:about="http://postdata.linhd.uned.es/kos/character-type">
        <rdf:type rdf:resource="http://www.w3.org/2004/02/skos/core#ConceptScheme"/>
        <dc:creator xml:lang="en">POSTDATA Project “This project has received funding from the European Research Council (ERC) under the European Union’s Horizon 2020 research and innovation programme (grant agreement Nº [679528])”</dc:creator>
        <terms:date rdf:datatype="http://www.w3.org/2001/XMLSchema#date">2019-10-27</terms:date>
        <terms:title xml:lang="es">Tesauro sobre tipos de rol</terms:title>
        <terms:title xml:lang="en">Thesaurus about character types</terms:title>
        <skos:definition xml:lang="en">Thesaurus about character types</skos:definition>
        <skos:prefLabel xml:lang="en">Character type scheme</skos:prefLabel>
    </owl:NamedIndividual>
    


    <!-- http://postdata.linhd.uned.es/kos/designation-type -->

    <owl:NamedIndividual rdf:about="http://postdata.linhd.uned.es/kos/designation-type">
        <rdf:type rdf:resource="http://www.w3.org/2004/02/skos/core#ConceptScheme"/>
        <dc:creator xml:lang="en">POSTDATA Project “This project has received funding from the European Research Council (ERC) under the European Union’s Horizon 2020 research and innovation programme (grant agreement Nº [679528])”</dc:creator>
        <terms:date rdf:datatype="http://www.w3.org/2001/XMLSchema#date">2019-10-27</terms:date>
        <terms:title xml:lang="es">Tesauro sobre tipos de nombre</terms:title>
        <terms:title xml:lang="en">Thesaurus about type of name</terms:title>
        <skos:definition xml:lang="en">Thesaurus about type of name</skos:definition>
        <skos:hasTopConcept rdf:resource="http://postdata.linhd.uned.es/kos/certainty/designation-type/allonym"/>
        <skos:hasTopConcept rdf:resource="http://postdata.linhd.uned.es/kos/designation-type/heteronym"/>
        <skos:hasTopConcept rdf:resource="http://postdata.linhd.uned.es/kos/designation-type/orthonym"/>
        <skos:hasTopConcept rdf:resource="http://postdata.linhd.uned.es/kos/designation-type/pseudonym"/>
        <skos:prefLabel xml:lang="en">Designation Type Scheme</skos:prefLabel>
        <prov:wasAttributedTo rdf:resource="https://www.linkedin.com/in/m-luisa-diez-platas-05710614"/>
    </owl:NamedIndividual>
    


    <!-- http://postdata.linhd.uned.es/kos/education-level -->

    <owl:NamedIndividual rdf:about="http://postdata.linhd.uned.es/kos/education-level">
        <rdf:type rdf:resource="http://www.w3.org/2004/02/skos/core#ConceptScheme"/>
        <dc:creator xml:lang="en">POSTDATA Project “This project has received funding from the European Research Council (ERC) under the European Union’s Horizon 2020 research and innovation programme (grant agreement Nº [679528])”</dc:creator>
        <terms:date rdf:datatype="http://www.w3.org/2001/XMLSchema#date">2019-10-27</terms:date>
        <terms:title xml:lang="es">Tesauro sobre nivel educativo</terms:title>
        <terms:title xml:lang="en">Thesaurus about education level</terms:title>
        <skos:definition xml:lang="en">Thesaurus about education levels. It includes all the concepts that are narrower to UNESCOTHES Educational Levels Concept (http://skos.um.es/unescothes/C01252)</skos:definition>
        <skos:prefLabel xml:lang="en">Education Level Scheme</skos:prefLabel>
        <prov:wasAttributedTo rdf:resource="https://www.linkedin.com/in/m-luisa-diez-platas-05710614"/>
    </owl:NamedIndividual>
    


    <!-- http://postdata.linhd.uned.es/kos/gender -->

    <owl:NamedIndividual rdf:about="http://postdata.linhd.uned.es/kos/gender">
        <rdf:type rdf:resource="http://www.w3.org/2004/02/skos/core#ConceptScheme"/>
        <dc:creator xml:lang="en">POSTDATA Project “This project has received funding from the European Research Council (ERC) under the European Union’s Horizon 2020 research and innovation programme (grant agreement Nº [679528])”</dc:creator>
        <terms:date rdf:datatype="http://www.w3.org/2001/XMLSchema#date">2019-10-27</terms:date>
        <terms:title xml:lang="es">Tesauro sobre géneros</terms:title>
        <terms:title xml:lang="en">Thesaurus about genders</terms:title>
        <skos:definition xml:lang="en">Thesaurus about genders</skos:definition>
        <skos:hasTopConcept rdf:resource="http://postdata.linhd.uned.es/kos/gender/female"/>
        <skos:hasTopConcept rdf:resource="http://postdata.linhd.uned.es/kos/gender/male"/>
        <skos:hasTopConcept rdf:resource="http://postdata.linhd.uned.es/kos/gender/other"/>
        <skos:hasTopConcept rdf:resource="http://postdata.linhd.uned.es/kos/gender/transgender"/>
        <skos:hasTopConcept rdf:resource="http://postdata.linhd.uned.es/kos/gender/unknown"/>
        <skos:prefLabel xml:lang="en">Gender Scheme</skos:prefLabel>
        <prov:wasAttributedTo rdf:resource="https://www.linkedin.com/in/m-luisa-diez-platas-05710614"/>
    </owl:NamedIndividual>
    


    <!-- http://postdata.linhd.uned.es/kos/genre -->

    <owl:NamedIndividual rdf:about="http://postdata.linhd.uned.es/kos/genre">
        <rdf:type rdf:resource="http://www.w3.org/2004/02/skos/core#ConceptScheme"/>
        <dc:creator xml:lang="en">POSTDATA Project “This project has received funding from the European Research Council (ERC) under the European Union’s Horizon 2020 research and innovation programme (grant agreement Nº [679528])”</dc:creator>
        <terms:date rdf:datatype="http://www.w3.org/2001/XMLSchema#date">2019-10-27</terms:date>
        <terms:title xml:lang="es">Tesauro sobre géneros literario</terms:title>
        <terms:title xml:lang="en">Thesaurus about literary genres</terms:title>
        <skos:definition xml:lang="en">Thesaurus about literary genres</skos:definition>
        <skos:prefLabel xml:lang="en">Genre Scheme</skos:prefLabel>
        <prov:wasAttributedTo rdf:resource="https://www.linkedin.com/in/m-luisa-diez-platas-05710614"/>
    </owl:NamedIndividual>
    


    <!-- http://postdata.linhd.uned.es/kos/literary-period -->

    <owl:NamedIndividual rdf:about="http://postdata.linhd.uned.es/kos/literary-period">
        <rdf:type rdf:resource="http://www.w3.org/2004/02/skos/core#ConceptScheme"/>
        <dc:creator xml:lang="en">POSTDATA Project “This project has received funding from the European Research Council (ERC) under the European Union’s Horizon 2020 research and innovation programme (grant agreement Nº [679528])”</dc:creator>
        <terms:date rdf:datatype="http://www.w3.org/2001/XMLSchema#date">2019-10-27</terms:date>
        <terms:title xml:lang="es">Tesauro sobre etiquuets de periodos temporales para agrupar ciertas obras</terms:title>
        <terms:title xml:lang="en">Thesaurus about labels of a time frame for grouping certain works</terms:title>
        <skos:definition xml:lang="en">Thesaurus about labels of a time frame for grouping certain works</skos:definition>
        <skos:prefLabel xml:lang="en">Literary Period Scheme</skos:prefLabel>
    </owl:NamedIndividual>
    


    <!-- http://postdata.linhd.uned.es/kos/literary-period-renaissance -->

    <owl:NamedIndividual rdf:about="http://postdata.linhd.uned.es/kos/literary-period-renaissance">
        <rdf:type rdf:resource="http://www.w3.org/2004/02/skos/core#Concept"/>
        <skos:inScheme rdf:resource="http://postdata.linhd.uned.es/kos/literary-period"/>
        <skos:topConceptOf rdf:resource="http://postdata.linhd.uned.es/kos/literary-period"/>
        <skos:prefLabel xml:lang="es">Renacimiento</skos:prefLabel>
        <skos:prefLabel xml:lang="en">Renaissance</skos:prefLabel>
    </owl:NamedIndividual>
    


    <!-- http://postdata.linhd.uned.es/kos/poetic-type -->

    <owl:NamedIndividual rdf:about="http://postdata.linhd.uned.es/kos/poetic-type">
        <rdf:type rdf:resource="http://www.w3.org/2004/02/skos/core#ConceptScheme"/>
        <dc:creator xml:lang="en">POSTDATA Project “This project has received funding from the European Research Council (ERC) under the European Union’s Horizon 2020 research and innovation programme (grant agreement Nº [679528])”</dc:creator>
        <terms:date rdf:datatype="http://www.w3.org/2001/XMLSchema#date">2019-10-27</terms:date>
        <terms:title xml:lang="es">Tesauro sobre el género literario principal de la obra</terms:title>
        <terms:title xml:lang="en">Thesaurus about major literary genre of the compositions. </terms:title>
        <skos:definition xml:lang="en">Thesaurus about major literary genre of the compositions</skos:definition>
        <skos:prefLabel xml:lang="en">Poetic Type Scheme</skos:prefLabel>
        <prov:wasAttributedTo rdf:resource="https://www.linkedin.com/in/m-luisa-diez-platas-05710614"/>
    </owl:NamedIndividual>
    


    <!-- http://postdata.linhd.uned.es/kos/religious-affiliation -->

    <owl:NamedIndividual rdf:about="http://postdata.linhd.uned.es/kos/religious-affiliation">
        <rdf:type rdf:resource="http://www.w3.org/2004/02/skos/core#ConceptScheme"/>
        <dc:creator xml:lang="en">POSTDATA Project “This project has received funding from the European Research Council (ERC) under the European Union’s Horizon 2020 research and innovation programme (grant agreement Nº [679528])”</dc:creator>
        <terms:date rdf:datatype="http://www.w3.org/2001/XMLSchema#date">2019-04-29</terms:date>
        <terms:title xml:lang="es">Tesauro sobre afiliaciones religiosas</terms:title>
        <terms:title xml:lang="es">Thesaurus about religious affiliations</terms:title>
        <skos:definition xml:lang="en">Thesaurus about religious affiliations</skos:definition>
        <skos:hasTopConcept rdf:resource="http://postdata.linhd.uned.es/kos/religious-affiliation/christian"/>
        <skos:hasTopConcept rdf:resource="http://postdata.linhd.uned.es/kos/religious-affiliation/unaffiliated"/>
        <skos:prefLabel xml:lang="en">Religious Affiliation Scheme</skos:prefLabel>
        <prov:wasAttributedTo rdf:resource="http://www.linkedin.com/in/ocorcho"/>
    </owl:NamedIndividual>
    


    <!-- http://postdata.linhd.uned.es/kos/role-function -->

    <owl:NamedIndividual rdf:about="http://postdata.linhd.uned.es/kos/role-function">
        <rdf:type rdf:resource="http://www.w3.org/2004/02/skos/core#ConceptScheme"/>
        <dc:creator xml:lang="en">POSTDATA Project “This project has received funding from the European Research Council (ERC) under the European Union’s Horizon 2020 research and innovation programme (grant agreement Nº [679528])”</dc:creator>
        <terms:date rdf:datatype="http://www.w3.org/2001/XMLSchema#date">2019-10-27</terms:date>
        <terms:title xml:lang="es">Tesauro sobre el papel específico representado por un agente en una obra</terms:title>
        <terms:title xml:lang="en">Thesaurus about specific function performed by some agent on a work</terms:title>
        <skos:definition xml:lang="en">Thesaurus about specific function performed by some agent on a work</skos:definition>
        <skos:hasTopConcept rdf:resource="http://postdata.linhd.uned.es/kos/role-function/actor"/>
        <skos:hasTopConcept rdf:resource="http://postdata.linhd.uned.es/kos/role-function/arranger"/>
        <skos:hasTopConcept rdf:resource="http://postdata.linhd.uned.es/kos/role-function/collector"/>
        <skos:hasTopConcept rdf:resource="http://postdata.linhd.uned.es/kos/role-function/singer"/>
        <skos:hasTopConcept rdf:resource="http://postdata.linhd.uned.es/kos/role-function/sponsor"/>
        <skos:hasTopConcept rdf:resource="http://postdata.linhd.uned.es/kos/role-function/transcriptor"/>
        <skos:prefLabel xml:lang="en">Role Function Scheme</skos:prefLabel>
        <prov:wasAttributedTo rdf:resource="https://www.linkedin.com/in/m-luisa-diez-platas-05710614"/>
    </owl:NamedIndividual>
    


    <!-- http://postdata.linhd.uned.es/kos/social-status -->

    <owl:NamedIndividual rdf:about="http://postdata.linhd.uned.es/kos/social-status">
        <rdf:type rdf:resource="http://www.w3.org/2004/02/skos/core#ConceptScheme"/>
        <dc:creator xml:lang="en">POSTDATA Project “This project has received funding from the European Research Council (ERC) under the European Union’s Horizon 2020 research and innovation programme (grant agreement Nº [679528])”</dc:creator>
        <terms:date rdf:datatype="http://www.w3.org/2001/XMLSchema#date">2019-10-27</terms:date>
        <terms:title xml:lang="es">Tesauro sobre el statuus social de una persona</terms:title>
        <terms:title xml:lang="en">Thesaurus about the socialstatus of a person</terms:title>
        <skos:definition xml:lang="en">Thesaurus about the socialstatus of a person</skos:definition>
        <skos:prefLabel xml:lang="en">Social Status Scheme</skos:prefLabel>
    </owl:NamedIndividual>
    


    <!-- http://postdata.linhd.uned.es/kos/textual-element-type -->

    <owl:NamedIndividual rdf:about="http://postdata.linhd.uned.es/kos/textual-element-type">
        <rdf:type rdf:resource="http://www.w3.org/2004/02/skos/core#ConceptScheme"/>
        <dc:creator xml:lang="en">POSTDATA Project “This project has received funding from the European Research Council (ERC) under the European Union’s Horizon 2020 research and innovation programme (grant agreement Nº [679528])”</dc:creator>
        <terms:date rdf:datatype="http://www.w3.org/2001/XMLSchema#date">2019-10-27</terms:date>
        <terms:title xml:lang="es">Tesauro sobre tipos de elementos textuales</terms:title>
        <terms:title xml:lang="en">Thesaurus about type of textual element</terms:title>
        <skos:definition xml:lang="en">Thesaurus about type of textual element</skos:definition>
        <skos:hasTopConcept rdf:resource="http://postdata.linhd.uned.es/kos/textual-element-type/chapter"/>
        <skos:hasTopConcept rdf:resource="http://postdata.linhd.uned.es/kos/textual-element-type/epilogue"/>
        <skos:hasTopConcept rdf:resource="http://postdata.linhd.uned.es/kos/textual-element-type/prologue"/>
        <skos:prefLabel xml:lang="en">Textual Element Type Scheme</skos:prefLabel>
        <prov:wasAttributedTo rdf:resource="https://www.linkedin.com/in/m-luisa-diez-platas-05710614"/>
    </owl:NamedIndividual>
    


    <!-- http://postdata.linhd.uned.es/kos/certainty/definitely -->

    <owl:NamedIndividual rdf:about="http://postdata.linhd.uned.es/kos/certainty/definitely">
        <rdf:type rdf:resource="http://www.w3.org/2004/02/skos/core#Concept"/>
        <skos:inScheme rdf:resource="http://postdata.linhd.uned.es/kos/certainty"/>
        <skos:notation>definitely</skos:notation>
        <skos:prefLabel xml:lang="en">Definitely</skos:prefLabel>
        <skos:prefLabel xml:lang="es">Definitivamente</skos:prefLabel>
    </owl:NamedIndividual>
    


    <!-- http://postdata.linhd.uned.es/kos/certainty/definitely-not -->

    <owl:NamedIndividual rdf:about="http://postdata.linhd.uned.es/kos/certainty/definitely-not">
        <rdf:type rdf:resource="http://www.w3.org/2004/02/skos/core#Concept"/>
        <skos:inScheme rdf:resource="http://postdata.linhd.uned.es/kos/certainty"/>
        <skos:notation>definitely-not</skos:notation>
        <skos:prefLabel xml:lang="en">Definitely not</skos:prefLabel>
        <skos:prefLabel xml:lang="es">Definitivamente no</skos:prefLabel>
    </owl:NamedIndividual>
    


    <!-- http://postdata.linhd.uned.es/kos/certainty/possibily -->

    <owl:NamedIndividual rdf:about="http://postdata.linhd.uned.es/kos/certainty/possibily">
        <rdf:type rdf:resource="http://www.w3.org/2004/02/skos/core#Concept"/>
        <skos:inScheme rdf:resource="http://postdata.linhd.uned.es/kos/certainty"/>
        <skos:notation>possibily</skos:notation>
        <skos:prefLabel xml:lang="es">Posiblemente</skos:prefLabel>
        <skos:prefLabel xml:lang="en">Possibily</skos:prefLabel>
    </owl:NamedIndividual>
    


    <!-- http://postdata.linhd.uned.es/kos/certainty/probably -->

    <owl:NamedIndividual rdf:about="http://postdata.linhd.uned.es/kos/certainty/probably">
        <rdf:type rdf:resource="http://www.w3.org/2004/02/skos/core#Concept"/>
        <skos:inScheme rdf:resource="http://postdata.linhd.uned.es/kos/certainty"/>
        <skos:notation>probably</skos:notation>
        <skos:prefLabel xml:lang="es">Probablemente</skos:prefLabel>
        <skos:prefLabel xml:lang="en">Probably</skos:prefLabel>
    </owl:NamedIndividual>
    


    <!-- http://postdata.linhd.uned.es/kos/certainty/probably-not -->

    <owl:NamedIndividual rdf:about="http://postdata.linhd.uned.es/kos/certainty/probably-not">
        <rdf:type rdf:resource="http://www.w3.org/2004/02/skos/core#Concept"/>
        <skos:inScheme rdf:resource="http://postdata.linhd.uned.es/kos/certainty"/>
        <skos:notation>probably-not</skos:notation>
        <skos:prefLabel xml:lang="es">Probablemente no</skos:prefLabel>
        <skos:prefLabel xml:lang="en">Probably not</skos:prefLabel>
    </owl:NamedIndividual>
    


    <!-- http://postdata.linhd.uned.es/kos/certainty/designation-type/allonym -->

    <owl:NamedIndividual rdf:about="http://postdata.linhd.uned.es/kos/certainty/designation-type/allonym">
        <rdf:type rdf:resource="http://www.w3.org/2004/02/skos/core#Concept"/>
        <skos:inScheme rdf:resource="http://postdata.linhd.uned.es/kos/designation-type"/>
        <skos:topConceptOf rdf:resource="http://postdata.linhd.uned.es/kos/designation-type"/>
        <skos:prefLabel xml:lang="en">Allonym</skos:prefLabel>
    </owl:NamedIndividual>
    


    <!-- http://postdata.linhd.uned.es/kos/character-type/donor -->

    <owl:NamedIndividual rdf:about="http://postdata.linhd.uned.es/kos/character-type/donor">
        <rdf:type rdf:resource="http://www.w3.org/2004/02/skos/core#Concept"/>
        <skos:inScheme rdf:resource="http://postdata.linhd.uned.es/kos/character-type"/>
        <skos:topConceptOf rdf:resource="http://postdata.linhd.uned.es/kos/character-type"/>
        <skos:prefLabel xml:lang="es">Donante del objeto mágico</skos:prefLabel>
        <skos:prefLabel xml:lang="en">Donor</skos:prefLabel>
    </owl:NamedIndividual>
    


    <!-- http://postdata.linhd.uned.es/kos/character-type/falsehero -->

    <owl:NamedIndividual rdf:about="http://postdata.linhd.uned.es/kos/character-type/falsehero">
        <rdf:type rdf:resource="http://www.w3.org/2004/02/skos/core#Concept"/>
        <skos:inScheme rdf:resource="http://postdata.linhd.uned.es/kos/character-type"/>
        <skos:topConceptOf rdf:resource="http://postdata.linhd.uned.es/kos/character-type"/>
        <skos:prefLabel xml:lang="en">False Hero</skos:prefLabel>
        <skos:prefLabel xml:lang="es">Falso héroe</skos:prefLabel>
    </owl:NamedIndividual>
    


    <!-- http://postdata.linhd.uned.es/kos/character-type/helper -->

    <owl:NamedIndividual rdf:about="http://postdata.linhd.uned.es/kos/character-type/helper">
        <rdf:type rdf:resource="http://www.w3.org/2004/02/skos/core#Concept"/>
        <skos:inScheme rdf:resource="http://postdata.linhd.uned.es/kos/character-type"/>
        <skos:topConceptOf rdf:resource="http://postdata.linhd.uned.es/kos/character-type"/>
        <skos:prefLabel xml:lang="es">Auxiliar</skos:prefLabel>
        <skos:prefLabel xml:lang="en">Helper</skos:prefLabel>
    </owl:NamedIndividual>
    


    <!-- http://postdata.linhd.uned.es/kos/character-type/hero -->

    <owl:NamedIndividual rdf:about="http://postdata.linhd.uned.es/kos/character-type/hero">
        <rdf:type rdf:resource="http://www.w3.org/2004/02/skos/core#Concept"/>
        <skos:inScheme rdf:resource="http://postdata.linhd.uned.es/kos/character-type"/>
        <skos:topConceptOf rdf:resource="http://postdata.linhd.uned.es/kos/character-type"/>
        <skos:prefLabel xml:lang="en">Hero</skos:prefLabel>
        <skos:prefLabel xml:lang="es">Héroe</skos:prefLabel>
    </owl:NamedIndividual>
    


    <!-- http://postdata.linhd.uned.es/kos/character-type/princess -->

    <owl:NamedIndividual rdf:about="http://postdata.linhd.uned.es/kos/character-type/princess">
        <rdf:type rdf:resource="http://www.w3.org/2004/02/skos/core#Concept"/>
        <skos:inScheme rdf:resource="http://postdata.linhd.uned.es/kos/character-type"/>
        <skos:topConceptOf rdf:resource="http://postdata.linhd.uned.es/kos/character-type"/>
        <skos:prefLabel xml:lang="es">Princesa</skos:prefLabel>
        <skos:prefLabel xml:lang="en">Princess</skos:prefLabel>
    </owl:NamedIndividual>
    


    <!-- http://postdata.linhd.uned.es/kos/character-type/princessfather -->

    <owl:NamedIndividual rdf:about="http://postdata.linhd.uned.es/kos/character-type/princessfather">
        <rdf:type rdf:resource="http://www.w3.org/2004/02/skos/core#Concept"/>
        <skos:inScheme rdf:resource="http://postdata.linhd.uned.es/kos/character-type"/>
        <skos:topConceptOf rdf:resource="http://postdata.linhd.uned.es/kos/character-type"/>
        <skos:prefLabel xml:lang="en">Princess&apos; Father</skos:prefLabel>
        <skos:prefLabel xml:lang="es">Rey o mandatario</skos:prefLabel>
    </owl:NamedIndividual>
    


    <!-- http://postdata.linhd.uned.es/kos/character-type/villain -->

    <owl:NamedIndividual rdf:about="http://postdata.linhd.uned.es/kos/character-type/villain">
        <rdf:type rdf:resource="http://www.w3.org/2004/02/skos/core#Concept"/>
        <skos:inScheme rdf:resource="http://postdata.linhd.uned.es/kos/character-type"/>
        <skos:topConceptOf rdf:resource="http://postdata.linhd.uned.es/kos/character-type"/>
        <skos:prefLabel xml:lang="es">Agresor</skos:prefLabel>
        <skos:prefLabel xml:lang="en">Villain</skos:prefLabel>
    </owl:NamedIndividual>
    


    <!-- http://postdata.linhd.uned.es/kos/designation-type/heteronym -->

    <owl:NamedIndividual rdf:about="http://postdata.linhd.uned.es/kos/designation-type/heteronym">
        <rdf:type rdf:resource="http://www.w3.org/2004/02/skos/core#Concept"/>
        <skos:inScheme rdf:resource="http://postdata.linhd.uned.es/kos/designation-type"/>
        <skos:notation>heteronym</skos:notation>
        <skos:prefLabel xml:lang="en">heteronym</skos:prefLabel>
        <skos:prefLabel xml:lang="es">heterónimo</skos:prefLabel>
    </owl:NamedIndividual>
    


    <!-- http://postdata.linhd.uned.es/kos/designation-type/orthonym -->

    <owl:NamedIndividual rdf:about="http://postdata.linhd.uned.es/kos/designation-type/orthonym">
        <rdf:type rdf:resource="http://www.w3.org/2004/02/skos/core#Concept"/>
        <skos:inScheme rdf:resource="http://postdata.linhd.uned.es/kos/designation-type"/>
        <skos:topConceptOf rdf:resource="http://postdata.linhd.uned.es/kos/designation-type"/>
        <skos:prefLabel xml:lang="en">Orthonym</skos:prefLabel>
        <skos:prefLabel xml:lang="es">Ortónimo</skos:prefLabel>
    </owl:NamedIndividual>
    


    <!-- http://postdata.linhd.uned.es/kos/designation-type/pseudonym -->

    <owl:NamedIndividual rdf:about="http://postdata.linhd.uned.es/kos/designation-type/pseudonym">
        <rdf:type rdf:resource="http://www.w3.org/2004/02/skos/core#Concept"/>
        <skos:inScheme rdf:resource="http://postdata.linhd.uned.es/kos/designation-type"/>
        <skos:notation>pseudonym</skos:notation>
        <skos:prefLabel xml:lang="en">pseudonym</skos:prefLabel>
        <skos:prefLabel xml:lang="es">pseudónimo</skos:prefLabel>
    </owl:NamedIndividual>
    


    <!-- http://postdata.linhd.uned.es/kos/gender/female -->

    <owl:NamedIndividual rdf:about="http://postdata.linhd.uned.es/kos/gender/female">
        <rdf:type rdf:resource="http://www.w3.org/2004/02/skos/core#Concept"/>
        <skos:inScheme rdf:resource="http://postdata.linhd.uned.es/kos/gender"/>
        <skos:topConceptOf rdf:resource="http://postdata.linhd.uned.es/kos/gender"/>
        <skos:prefLabel xml:lang="en">Female</skos:prefLabel>
        <skos:prefLabel xml:lang="es">Mujer</skos:prefLabel>
    </owl:NamedIndividual>
    


    <!-- http://postdata.linhd.uned.es/kos/gender/male -->

    <owl:NamedIndividual rdf:about="http://postdata.linhd.uned.es/kos/gender/male">
        <rdf:type rdf:resource="http://www.w3.org/2004/02/skos/core#Concept"/>
        <skos:inScheme rdf:resource="http://postdata.linhd.uned.es/kos/gender"/>
        <skos:topConceptOf rdf:resource="http://postdata.linhd.uned.es/kos/gender"/>
        <skos:prefLabel xml:lang="es">Hombre</skos:prefLabel>
        <skos:prefLabel xml:lang="en">Male</skos:prefLabel>
    </owl:NamedIndividual>
    


    <!-- http://postdata.linhd.uned.es/kos/gender/other -->

    <owl:NamedIndividual rdf:about="http://postdata.linhd.uned.es/kos/gender/other">
        <rdf:type rdf:resource="http://www.w3.org/2004/02/skos/core#Concept"/>
        <skos:inScheme rdf:resource="http://postdata.linhd.uned.es/kos/gender"/>
        <skos:topConceptOf rdf:resource="http://postdata.linhd.uned.es/kos/gender"/>
        <skos:prefLabel xml:lang="en">Other</skos:prefLabel>
        <skos:prefLabel xml:lang="es">Otro</skos:prefLabel>
    </owl:NamedIndividual>
    


    <!-- http://postdata.linhd.uned.es/kos/gender/transgender -->

    <owl:NamedIndividual rdf:about="http://postdata.linhd.uned.es/kos/gender/transgender">
        <rdf:type rdf:resource="http://www.w3.org/2004/02/skos/core#Concept"/>
        <skos:inScheme rdf:resource="http://postdata.linhd.uned.es/kos/gender"/>
        <skos:topConceptOf rdf:resource="http://postdata.linhd.uned.es/kos/gender"/>
        <skos:prefLabel xml:lang="en">Transgender</skos:prefLabel>
        <skos:prefLabel xml:lang="es">Transgénero</skos:prefLabel>
    </owl:NamedIndividual>
    


    <!-- http://postdata.linhd.uned.es/kos/gender/unknown -->

    <owl:NamedIndividual rdf:about="http://postdata.linhd.uned.es/kos/gender/unknown">
        <rdf:type rdf:resource="http://www.w3.org/2004/02/skos/core#Concept"/>
        <skos:inScheme rdf:resource="http://postdata.linhd.uned.es/kos/gender"/>
        <skos:topConceptOf rdf:resource="http://postdata.linhd.uned.es/kos/gender"/>
        <skos:prefLabel xml:lang="es">Desconocido</skos:prefLabel>
        <skos:prefLabel xml:lang="en">Unknown</skos:prefLabel>
    </owl:NamedIndividual>
    


    <!-- http://postdata.linhd.uned.es/kos/literary-period/baroque -->

    <owl:NamedIndividual rdf:about="http://postdata.linhd.uned.es/kos/literary-period/baroque">
        <rdf:type rdf:resource="http://www.w3.org/2004/02/skos/core#Concept"/>
        <skos:inScheme rdf:resource="http://postdata.linhd.uned.es/kos/literary-period"/>
        <skos:topConceptOf rdf:resource="http://postdata.linhd.uned.es/kos/literary-period"/>
        <skos:prefLabel xml:lang="en">Baroque</skos:prefLabel>
        <skos:prefLabel xml:lang="es">Barroco</skos:prefLabel>
    </owl:NamedIndividual>
    


    <!-- http://postdata.linhd.uned.es/kos/literary-period/classical-antiquity -->

    <owl:NamedIndividual rdf:about="http://postdata.linhd.uned.es/kos/literary-period/classical-antiquity">
        <rdf:type rdf:resource="http://www.w3.org/2004/02/skos/core#Concept"/>
        <skos:inScheme rdf:resource="http://postdata.linhd.uned.es/kos/literary-period"/>
        <skos:topConceptOf rdf:resource="http://postdata.linhd.uned.es/kos/literary-period"/>
        <skos:prefLabel xml:lang="es">Antigüedad Clásica</skos:prefLabel>
        <skos:prefLabel xml:lang="en">Classical Antiquity</skos:prefLabel>
    </owl:NamedIndividual>
    


    <!-- http://postdata.linhd.uned.es/kos/literary-period/enlightenment -->

    <owl:NamedIndividual rdf:about="http://postdata.linhd.uned.es/kos/literary-period/enlightenment">
        <rdf:type rdf:resource="http://www.w3.org/2004/02/skos/core#Concept"/>
        <skos:inScheme rdf:resource="http://postdata.linhd.uned.es/kos/literary-period"/>
        <skos:topConceptOf rdf:resource="http://postdata.linhd.uned.es/kos/literary-period"/>
        <skos:prefLabel xml:lang="en">Enlightenment</skos:prefLabel>
        <skos:prefLabel xml:lang="es">Ilustración</skos:prefLabel>
    </owl:NamedIndividual>
    


    <!-- http://postdata.linhd.uned.es/kos/literary-period/middle-ages -->

    <owl:NamedIndividual rdf:about="http://postdata.linhd.uned.es/kos/literary-period/middle-ages">
        <rdf:type rdf:resource="http://www.w3.org/2004/02/skos/core#Concept"/>
        <skos:inScheme rdf:resource="http://postdata.linhd.uned.es/kos/literary-period"/>
        <skos:topConceptOf rdf:resource="http://postdata.linhd.uned.es/kos/literary-period"/>
        <skos:prefLabel xml:lang="es">Edad Media</skos:prefLabel>
        <skos:prefLabel xml:lang="en">Middle Ages</skos:prefLabel>
    </owl:NamedIndividual>
    


    <!-- http://postdata.linhd.uned.es/kos/literary-period/modernism -->

    <owl:NamedIndividual rdf:about="http://postdata.linhd.uned.es/kos/literary-period/modernism">
        <rdf:type rdf:resource="http://www.w3.org/2004/02/skos/core#Concept"/>
        <skos:inScheme rdf:resource="http://postdata.linhd.uned.es/kos/literary-period"/>
        <skos:topConceptOf rdf:resource="http://postdata.linhd.uned.es/kos/literary-period"/>
        <skos:prefLabel xml:lang="en">Modernism</skos:prefLabel>
        <skos:prefLabel xml:lang="es">Modernismo</skos:prefLabel>
    </owl:NamedIndividual>
    


    <!-- http://postdata.linhd.uned.es/kos/literary-period/realism -->

    <owl:NamedIndividual rdf:about="http://postdata.linhd.uned.es/kos/literary-period/realism">
        <rdf:type rdf:resource="http://www.w3.org/2004/02/skos/core#Concept"/>
        <skos:inScheme rdf:resource="http://postdata.linhd.uned.es/kos/literary-period"/>
        <skos:topConceptOf rdf:resource="http://postdata.linhd.uned.es/kos/literary-period"/>
        <skos:prefLabel xml:lang="en">Realism</skos:prefLabel>
        <skos:prefLabel xml:lang="es">Realismo</skos:prefLabel>
    </owl:NamedIndividual>
    


    <!-- http://postdata.linhd.uned.es/kos/literary-period/romanticism -->

    <owl:NamedIndividual rdf:about="http://postdata.linhd.uned.es/kos/literary-period/romanticism">
        <rdf:type rdf:resource="http://www.w3.org/2004/02/skos/core#Concept"/>
        <skos:inScheme rdf:resource="http://postdata.linhd.uned.es/kos/literary-period"/>
        <skos:topConceptOf rdf:resource="http://postdata.linhd.uned.es/kos/literary-period"/>
        <skos:prefLabel xml:lang="en">Romanticism</skos:prefLabel>
        <skos:prefLabel xml:lang="es">Romanticismo</skos:prefLabel>
    </owl:NamedIndividual>
    


    <!-- http://postdata.linhd.uned.es/kos/literary-period/vanguardism -->

    <owl:NamedIndividual rdf:about="http://postdata.linhd.uned.es/kos/literary-period/vanguardism">
        <rdf:type rdf:resource="http://www.w3.org/2004/02/skos/core#Concept"/>
        <skos:inScheme rdf:resource="http://postdata.linhd.uned.es/kos/literary-period"/>
        <skos:topConceptOf rdf:resource="http://postdata.linhd.uned.es/kos/literary-period"/>
        <skos:prefLabel xml:lang="es">Vanguardias</skos:prefLabel>
        <skos:prefLabel xml:lang="en">Vanguardism</skos:prefLabel>
    </owl:NamedIndividual>
    


    <!-- http://postdata.linhd.uned.es/kos/religious-affiliation/catholic -->

    <owl:NamedIndividual rdf:about="http://postdata.linhd.uned.es/kos/religious-affiliation/catholic">
        <rdf:type rdf:resource="http://www.w3.org/2004/02/skos/core#Concept"/>
        <skos:broader rdf:resource="http://postdata.linhd.uned.es/kos/religious-affiliation/christian"/>
        <skos:inScheme rdf:resource="http://postdata.linhd.uned.es/kos/religious-affiliation"/>
        <skos:notation>catholic</skos:notation>
        <skos:prefLabel xml:lang="en">Catholic</skos:prefLabel>
        <skos:prefLabel xml:lang="es">Católico</skos:prefLabel>
    </owl:NamedIndividual>
    


    <!-- http://postdata.linhd.uned.es/kos/religious-affiliation/christian -->

    <owl:NamedIndividual rdf:about="http://postdata.linhd.uned.es/kos/religious-affiliation/christian">
        <rdf:type rdf:resource="http://www.w3.org/2004/02/skos/core#Concept"/>
        <skos:exactMatch rdf:resource="http://vocabularies.unesco.org/thesaurus/concept5153"/>
        <skos:inScheme rdf:resource="http://postdata.linhd.uned.es/kos/religious-affiliation"/>
        <skos:narrower rdf:resource="http://postdata.linhd.uned.es/kos/religious-affiliation/catholic"/>
        <skos:narrower rdf:resource="http://postdata.linhd.uned.es/kos/religious-affiliation/jehovah-witness"/>
        <skos:narrower rdf:resource="http://postdata.linhd.uned.es/kos/religious-affiliation/mormon"/>
        <skos:narrower rdf:resource="http://postdata.linhd.uned.es/kos/religious-affiliation/orthodox"/>
        <skos:narrower rdf:resource="http://postdata.linhd.uned.es/kos/religious-affiliation/other-christian"/>
        <skos:narrower rdf:resource="http://postdata.linhd.uned.es/kos/religious-affiliation/protestant"/>
        <skos:notation>christian</skos:notation>
        <skos:prefLabel xml:lang="en">Christian</skos:prefLabel>
        <skos:prefLabel xml:lang="es">Cristiano</skos:prefLabel>
    </owl:NamedIndividual>
    


    <!-- http://postdata.linhd.uned.es/kos/religious-affiliation/jehovah-witness -->

    <owl:NamedIndividual rdf:about="http://postdata.linhd.uned.es/kos/religious-affiliation/jehovah-witness">
        <rdf:type rdf:resource="http://www.w3.org/2004/02/skos/core#Concept"/>
        <skos:broader rdf:resource="http://postdata.linhd.uned.es/kos/religious-affiliation/christian"/>
        <skos:inScheme rdf:resource="http://postdata.linhd.uned.es/kos/religious-affiliation"/>
        <skos:notation>jehovah-witness</skos:notation>
        <skos:prefLabel xml:lang="en">Jehova&apos;s Witness</skos:prefLabel>
        <skos:prefLabel xml:lang="es">Testigo de Jehová</skos:prefLabel>
    </owl:NamedIndividual>
    


    <!-- http://postdata.linhd.uned.es/kos/religious-affiliation/mormon -->

    <owl:NamedIndividual rdf:about="http://postdata.linhd.uned.es/kos/religious-affiliation/mormon">
        <rdf:type rdf:resource="http://www.w3.org/2004/02/skos/core#Concept"/>
        <skos:broader rdf:resource="http://postdata.linhd.uned.es/kos/religious-affiliation/christian"/>
        <skos:inScheme rdf:resource="http://postdata.linhd.uned.es/kos/religious-affiliation"/>
        <skos:notation>mormon</skos:notation>
        <skos:prefLabel xml:lang="en">Mormon</skos:prefLabel>
        <skos:prefLabel xml:lang="es">Mormón</skos:prefLabel>
    </owl:NamedIndividual>
    


    <!-- http://postdata.linhd.uned.es/kos/religious-affiliation/orthodox -->

    <owl:NamedIndividual rdf:about="http://postdata.linhd.uned.es/kos/religious-affiliation/orthodox">
        <rdf:type rdf:resource="http://www.w3.org/2004/02/skos/core#Concept"/>
        <skos:broader rdf:resource="http://postdata.linhd.uned.es/kos/religious-affiliation/christian"/>
        <skos:inScheme rdf:resource="http://postdata.linhd.uned.es/kos/religious-affiliation"/>
        <skos:notation>orthodox</skos:notation>
        <skos:prefLabel xml:lang="en">Orthodox</skos:prefLabel>
        <skos:prefLabel xml:lang="es">Ortodoxo</skos:prefLabel>
    </owl:NamedIndividual>
    


    <!-- http://postdata.linhd.uned.es/kos/religious-affiliation/other-christian -->

    <owl:NamedIndividual rdf:about="http://postdata.linhd.uned.es/kos/religious-affiliation/other-christian">
        <rdf:type rdf:resource="http://www.w3.org/2004/02/skos/core#Concept"/>
        <skos:broader rdf:resource="http://postdata.linhd.uned.es/kos/religious-affiliation/christian"/>
        <skos:inScheme rdf:resource="http://postdata.linhd.uned.es/kos/religious-affiliation"/>
        <skos:notation>other-christian</skos:notation>
        <skos:prefLabel xml:lang="en">Other Christian</skos:prefLabel>
        <skos:prefLabel xml:lang="es">Otros Cristianos</skos:prefLabel>
    </owl:NamedIndividual>
    


    <!-- http://postdata.linhd.uned.es/kos/religious-affiliation/protestant -->

    <owl:NamedIndividual rdf:about="http://postdata.linhd.uned.es/kos/religious-affiliation/protestant">
        <rdf:type rdf:resource="http://www.w3.org/2004/02/skos/core#Concept"/>
        <skos:broader rdf:resource="http://postdata.linhd.uned.es/kos/religious-affiliation/christian"/>
        <skos:inScheme rdf:resource="http://postdata.linhd.uned.es/kos/religious-affiliation"/>
        <skos:notation>protestant</skos:notation>
        <skos:prefLabel xml:lang="en">Protestant</skos:prefLabel>
        <skos:prefLabel xml:lang="es">Protestante</skos:prefLabel>
    </owl:NamedIndividual>
    


    <!-- http://postdata.linhd.uned.es/kos/religious-affiliation/unaffiliated -->

    <owl:NamedIndividual rdf:about="http://postdata.linhd.uned.es/kos/religious-affiliation/unaffiliated">
        <rdf:type rdf:resource="http://www.w3.org/2004/02/skos/core#Concept"/>
        <skos:inScheme rdf:resource="http://postdata.linhd.uned.es/kos/religious-affiliation"/>
        <skos:notation>unaffiliated</skos:notation>
        <skos:prefLabel xml:lang="es">Sin afiliación</skos:prefLabel>
        <skos:prefLabel xml:lang="en">Unaffiliated</skos:prefLabel>
    </owl:NamedIndividual>
    


    <!-- http://postdata.linhd.uned.es/kos/role-function/actor -->

    <owl:NamedIndividual rdf:about="http://postdata.linhd.uned.es/kos/role-function/actor">
        <rdf:type rdf:resource="http://www.w3.org/2004/02/skos/core#Concept"/>
        <skos:inScheme rdf:resource="http://postdata.linhd.uned.es/kos/role-function"/>
        <skos:notation>actor</skos:notation>
        <skos:prefLabel xml:lang="en">Actor</skos:prefLabel>
        <skos:prefLabel xml:lang="es">Agente</skos:prefLabel>
    </owl:NamedIndividual>
    


    <!-- http://postdata.linhd.uned.es/kos/role-function/arranger -->

    <owl:NamedIndividual rdf:about="http://postdata.linhd.uned.es/kos/role-function/arranger">
        <rdf:type rdf:resource="http://www.w3.org/2004/02/skos/core#Concept"/>
        <skos:inScheme rdf:resource="http://postdata.linhd.uned.es/kos/role-function"/>
        <skos:notation>arranger</skos:notation>
        <skos:prefLabel xml:lang="en">Arranger</skos:prefLabel>
        <skos:prefLabel xml:lang="es">Organizador</skos:prefLabel>
    </owl:NamedIndividual>
    


    <!-- http://postdata.linhd.uned.es/kos/role-function/collector -->

    <owl:NamedIndividual rdf:about="http://postdata.linhd.uned.es/kos/role-function/collector">
        <rdf:type rdf:resource="http://www.w3.org/2004/02/skos/core#Concept"/>
        <skos:inScheme rdf:resource="http://postdata.linhd.uned.es/kos/role-function"/>
        <skos:notation>collector</skos:notation>
        <skos:prefLabel xml:lang="es">Coleccionista</skos:prefLabel>
        <skos:prefLabel xml:lang="en">Collector</skos:prefLabel>
    </owl:NamedIndividual>
    


    <!-- http://postdata.linhd.uned.es/kos/role-function/singer -->

    <owl:NamedIndividual rdf:about="http://postdata.linhd.uned.es/kos/role-function/singer">
        <rdf:type rdf:resource="http://www.w3.org/2004/02/skos/core#Concept"/>
        <skos:inScheme rdf:resource="http://postdata.linhd.uned.es/kos/role-function"/>
        <skos:notation>singer</skos:notation>
        <skos:prefLabel xml:lang="es">Cantante</skos:prefLabel>
        <skos:prefLabel xml:lang="en">Singer</skos:prefLabel>
    </owl:NamedIndividual>
    


    <!-- http://postdata.linhd.uned.es/kos/role-function/sponsor -->

    <owl:NamedIndividual rdf:about="http://postdata.linhd.uned.es/kos/role-function/sponsor">
        <rdf:type rdf:resource="http://www.w3.org/2004/02/skos/core#Concept"/>
        <skos:inScheme rdf:resource="http://postdata.linhd.uned.es/kos/role-function"/>
        <skos:notation>sponsor</skos:notation>
        <skos:prefLabel xml:lang="es">Patrocinador</skos:prefLabel>
        <skos:prefLabel xml:lang="en">Sponsor</skos:prefLabel>
    </owl:NamedIndividual>
    


    <!-- http://postdata.linhd.uned.es/kos/role-function/transcriptor -->

    <owl:NamedIndividual rdf:about="http://postdata.linhd.uned.es/kos/role-function/transcriptor">
        <rdf:type rdf:resource="http://www.w3.org/2004/02/skos/core#Concept"/>
        <skos:inScheme rdf:resource="http://postdata.linhd.uned.es/kos/role-function"/>
        <skos:notation>Ttranscriptor</skos:notation>
        <skos:prefLabel xml:lang="en">Transcriptor</skos:prefLabel>
        <skos:prefLabel xml:lang="es">Transcriptor</skos:prefLabel>
    </owl:NamedIndividual>
    


    <!-- http://postdata.linhd.uned.es/kos/social-status/beggar -->

    <owl:NamedIndividual rdf:about="http://postdata.linhd.uned.es/kos/social-status/beggar">
        <rdf:type rdf:resource="http://www.w3.org/2004/02/skos/core#Concept"/>
        <skos:inScheme rdf:resource="http://postdata.linhd.uned.es/kos/social-status"/>
        <skos:topConceptOf rdf:resource="http://postdata.linhd.uned.es/kos/social-status"/>
        <skos:prefLabel xml:lang="en">Beggar</skos:prefLabel>
        <skos:prefLabel xml:lang="es">Pobre</skos:prefLabel>
    </owl:NamedIndividual>
    


    <!-- http://postdata.linhd.uned.es/kos/social-status/hidalgo -->

    <owl:NamedIndividual rdf:about="http://postdata.linhd.uned.es/kos/social-status/hidalgo">
        <rdf:type rdf:resource="http://www.w3.org/2004/02/skos/core#Concept"/>
        <skos:inScheme rdf:resource="http://postdata.linhd.uned.es/kos/social-status"/>
        <skos:topConceptOf rdf:resource="http://postdata.linhd.uned.es/kos/social-status"/>
        <skos:prefLabel xml:lang="es">Hildago</skos:prefLabel>
    </owl:NamedIndividual>
    


    <!-- http://postdata.linhd.uned.es/kos/social-status/knight -->

    <owl:NamedIndividual rdf:about="http://postdata.linhd.uned.es/kos/social-status/knight">
        <rdf:type rdf:resource="http://www.w3.org/2004/02/skos/core#Concept"/>
        <skos:inScheme rdf:resource="http://postdata.linhd.uned.es/kos/social-status"/>
        <skos:topConceptOf rdf:resource="http://postdata.linhd.uned.es/kos/social-status"/>
        <skos:prefLabel xml:lang="es">Caballero</skos:prefLabel>
        <skos:prefLabel xml:lang="en">Knight</skos:prefLabel>
    </owl:NamedIndividual>
    


    <!-- http://postdata.linhd.uned.es/kos/social-status/mechanical-arts -->

    <owl:NamedIndividual rdf:about="http://postdata.linhd.uned.es/kos/social-status/mechanical-arts">
        <rdf:type rdf:resource="http://www.w3.org/2004/02/skos/core#Concept"/>
        <skos:inScheme rdf:resource="http://postdata.linhd.uned.es/kos/social-status"/>
        <skos:topConceptOf rdf:resource="http://postdata.linhd.uned.es/kos/social-status"/>
        <skos:prefLabel xml:lang="en">Mechanical arts</skos:prefLabel>
        <skos:prefLabel xml:lang="es">Oficial</skos:prefLabel>
    </owl:NamedIndividual>
    


    <!-- http://postdata.linhd.uned.es/kos/social-status/nobleman -->

    <owl:NamedIndividual rdf:about="http://postdata.linhd.uned.es/kos/social-status/nobleman">
        <rdf:type rdf:resource="http://www.w3.org/2004/02/skos/core#Concept"/>
        <skos:inScheme rdf:resource="http://postdata.linhd.uned.es/kos/social-status"/>
        <skos:topConceptOf rdf:resource="http://postdata.linhd.uned.es/kos/social-status"/>
        <skos:prefLabel xml:lang="es">Noble</skos:prefLabel>
        <skos:prefLabel xml:lang="en">Nobleman</skos:prefLabel>
    </owl:NamedIndividual>
    


    <!-- http://postdata.linhd.uned.es/kos/social-status/priest -->

    <owl:NamedIndividual rdf:about="http://postdata.linhd.uned.es/kos/social-status/priest">
        <rdf:type rdf:resource="http://www.w3.org/2004/02/skos/core#Concept"/>
        <skos:inScheme rdf:resource="http://postdata.linhd.uned.es/kos/social-status"/>
        <skos:topConceptOf rdf:resource="http://postdata.linhd.uned.es/kos/social-status"/>
        <skos:prefLabel xml:lang="es">Clérigo</skos:prefLabel>
        <skos:prefLabel xml:lang="en">Priest</skos:prefLabel>
    </owl:NamedIndividual>
    


    <!-- http://postdata.linhd.uned.es/kos/social-status/public-position -->

    <owl:NamedIndividual rdf:about="http://postdata.linhd.uned.es/kos/social-status/public-position">
        <rdf:type rdf:resource="http://www.w3.org/2004/02/skos/core#Concept"/>
        <skos:inScheme rdf:resource="http://postdata.linhd.uned.es/kos/social-status"/>
        <skos:topConceptOf rdf:resource="http://postdata.linhd.uned.es/kos/social-status"/>
        <skos:prefLabel xml:lang="es">Cargo público</skos:prefLabel>
        <skos:prefLabel xml:lang="en">Public position</skos:prefLabel>
    </owl:NamedIndividual>
    


    <!-- http://postdata.linhd.uned.es/kos/social-status/scholar -->

    <owl:NamedIndividual rdf:about="http://postdata.linhd.uned.es/kos/social-status/scholar">
        <rdf:type rdf:resource="http://www.w3.org/2004/02/skos/core#Concept"/>
        <skos:inScheme rdf:resource="http://postdata.linhd.uned.es/kos/social-status"/>
        <skos:topConceptOf rdf:resource="http://postdata.linhd.uned.es/kos/social-status"/>
        <skos:prefLabel xml:lang="es">Letrado</skos:prefLabel>
        <skos:prefLabel xml:lang="en">Scholar</skos:prefLabel>
    </owl:NamedIndividual>
    


    <!-- http://postdata.linhd.uned.es/kos/social-status/servant -->

    <owl:NamedIndividual rdf:about="http://postdata.linhd.uned.es/kos/social-status/servant">
        <rdf:type rdf:resource="http://www.w3.org/2004/02/skos/core#Concept"/>
        <skos:inScheme rdf:resource="http://postdata.linhd.uned.es/kos/social-status"/>
        <skos:topConceptOf rdf:resource="http://postdata.linhd.uned.es/kos/social-status"/>
        <skos:prefLabel xml:lang="es">Criado</skos:prefLabel>
        <skos:prefLabel xml:lang="en">Servant</skos:prefLabel>
    </owl:NamedIndividual>
    


    <!-- http://postdata.linhd.uned.es/kos/social-status/soldier -->

    <owl:NamedIndividual rdf:about="http://postdata.linhd.uned.es/kos/social-status/soldier">
        <rdf:type rdf:resource="http://www.w3.org/2004/02/skos/core#Concept"/>
        <skos:inScheme rdf:resource="http://postdata.linhd.uned.es/kos/social-status"/>
        <skos:topConceptOf rdf:resource="http://postdata.linhd.uned.es/kos/social-status"/>
        <skos:prefLabel xml:lang="es">Soldado</skos:prefLabel>
        <skos:prefLabel xml:lang="en">Soldier</skos:prefLabel>
    </owl:NamedIndividual>
    


    <!-- http://postdata.linhd.uned.es/kos/social-status/writer -->

    <owl:NamedIndividual rdf:about="http://postdata.linhd.uned.es/kos/social-status/writer">
        <rdf:type rdf:resource="http://www.w3.org/2004/02/skos/core#Concept"/>
        <skos:inScheme rdf:resource="http://postdata.linhd.uned.es/kos/social-status"/>
        <skos:topConceptOf rdf:resource="http://postdata.linhd.uned.es/kos/social-status"/>
        <skos:prefLabel xml:lang="es">Escritor</skos:prefLabel>
        <skos:prefLabel xml:lang="en">Writer</skos:prefLabel>
    </owl:NamedIndividual>
    


    <!-- http://postdata.linhd.uned.es/kos/textual-element-type/chapter -->

    <owl:NamedIndividual rdf:about="http://postdata.linhd.uned.es/kos/textual-element-type/chapter">
        <rdf:type rdf:resource="http://www.w3.org/2004/02/skos/core#Concept"/>
        <skos:inScheme rdf:resource="http://postdata.linhd.uned.es/kos/textual-element-type"/>
        <skos:notation>chapter</skos:notation>
        <skos:prefLabel xml:lang="es">Capítulo</skos:prefLabel>
        <skos:prefLabel xml:lang="en">Chapter</skos:prefLabel>
    </owl:NamedIndividual>
    


    <!-- http://postdata.linhd.uned.es/kos/textual-element-type/epilogue -->

    <owl:NamedIndividual rdf:about="http://postdata.linhd.uned.es/kos/textual-element-type/epilogue">
        <rdf:type rdf:resource="http://www.w3.org/2004/02/skos/core#Concept"/>
        <skos:inScheme rdf:resource="http://postdata.linhd.uned.es/kos/textual-element-type"/>
        <skos:notation>epilogue</skos:notation>
        <skos:prefLabel xml:lang="en">Epilogue</skos:prefLabel>
        <skos:prefLabel xml:lang="es">Epílogo</skos:prefLabel>
    </owl:NamedIndividual>
    


    <!-- http://postdata.linhd.uned.es/kos/textual-element-type/poem -->

    <owl:NamedIndividual rdf:about="http://postdata.linhd.uned.es/kos/textual-element-type/poem">
        <rdf:type rdf:resource="http://www.w3.org/2004/02/skos/core#Concept"/>
        <skos:inScheme rdf:resource="http://postdata.linhd.uned.es/kos/textual-element-type"/>
        <skos:topConceptOf rdf:resource="http://postdata.linhd.uned.es/kos/textual-element-type"/>
        <skos:prefLabel xml:lang="en">Poem</skos:prefLabel>
        <skos:prefLabel xml:lang="es">Poema</skos:prefLabel>
    </owl:NamedIndividual>
    


    <!-- http://postdata.linhd.uned.es/kos/textual-element-type/prologue -->

    <owl:NamedIndividual rdf:about="http://postdata.linhd.uned.es/kos/textual-element-type/prologue">
        <rdf:type rdf:resource="http://www.w3.org/2004/02/skos/core#Concept"/>
        <skos:inScheme rdf:resource="http://postdata.linhd.uned.es/kos/textual-element-type"/>
        <skos:notation>prologue</skos:notation>
        <skos:prefLabel xml:lang="en">Prologue</skos:prefLabel>
        <skos:prefLabel xml:lang="es">Prólogo</skos:prefLabel>
    </owl:NamedIndividual>
    


    <!-- http://postdata.linhd.uned.es/kos/textual-element-type/stanza -->

    <owl:NamedIndividual rdf:about="http://postdata.linhd.uned.es/kos/textual-element-type/stanza">
        <rdf:type rdf:resource="http://www.w3.org/2004/02/skos/core#Concept"/>
        <skos:inScheme rdf:resource="http://postdata.linhd.uned.es/kos/textual-element-type"/>
        <skos:topConceptOf rdf:resource="http://postdata.linhd.uned.es/kos/textual-element-type"/>
        <skos:prefLabel xml:lang="es">Estrofa</skos:prefLabel>
        <skos:prefLabel xml:lang="en">Stanza</skos:prefLabel>
    </owl:NamedIndividual>
    


    <!-- http://postdata.linhd.uned.es/ontology/postdata-core#Creator -->

    <owl:NamedIndividual rdf:about="http://postdata.linhd.uned.es/ontology/postdata-core#Creator">
        <rdf:type rdf:resource="http://www.w3.org/2004/02/skos/core#Concept"/>
        <skos:inScheme rdf:resource="http://postdata.linhd.uned.es/kos/role-function"/>
        <skos:prefLabel xml:lang="es">Creador</skos:prefLabel>
        <skos:prefLabel xml:lang="en">Creator</skos:prefLabel>
    </owl:NamedIndividual>
    


    <!-- http://postdata.linhd.uned.es/ontology/postdata-core#Editor -->

    <owl:NamedIndividual rdf:about="http://postdata.linhd.uned.es/ontology/postdata-core#Editor">
        <rdf:type rdf:resource="http://www.w3.org/2004/02/skos/core#Concept"/>
        <skos:inScheme rdf:resource="http://postdata.linhd.uned.es/kos/role-function"/>
        <skos:prefLabel xml:lang="en">Editor</skos:prefLabel>
    </owl:NamedIndividual>
    


    <!-- http://vocabularies.unesco.org/thesaurus/concept12949 -->

    <owl:NamedIndividual rdf:about="http://vocabularies.unesco.org/thesaurus/concept12949">
        <rdf:type rdf:resource="http://www.w3.org/2004/02/skos/core#Concept"/>
        <skos:broader rdf:resource="http://vocabularies.unesco.org/thesaurus/concept293"/>
        <skos:inScheme rdf:resource="http://postdata.linhd.uned.es/kos/religious-affiliation"/>
        <skos:topConceptOf rdf:resource="http://postdata.linhd.uned.es/kos/religious-affiliation"/>
        <skos:prefLabel xml:lang="en">Moslems</skos:prefLabel>
        <skos:prefLabel xml:lang="fr">Musulman</skos:prefLabel>
        <skos:prefLabel xml:lang="es">Musulmán</skos:prefLabel>
        <skos:prefLabel xml:lang="ru">Мусульмане</skos:prefLabel>
        <skos:prefLabel xml:lang="ar">مسلمون</skos:prefLabel>
    </owl:NamedIndividual>
    


    <!-- http://vocabularies.unesco.org/thesaurus/concept1485 -->

    <owl:NamedIndividual rdf:about="http://vocabularies.unesco.org/thesaurus/concept1485">
        <rdf:type rdf:resource="http://www.w3.org/2004/02/skos/core#Concept"/>
        <skos:broader rdf:resource="http://vocabularies.unesco.org/thesaurus/concept36"/>
        <skos:inScheme rdf:resource="http://postdata.linhd.uned.es/kos/education-level"/>
        <skos:topConceptOf rdf:resource="http://postdata.linhd.uned.es/kos/education-level"/>
        <skos:prefLabel xml:lang="fr">Enseignement supérieur</skos:prefLabel>
        <skos:prefLabel xml:lang="es">Enseñanza superior</skos:prefLabel>
        <skos:prefLabel xml:lang="en">Higher education</skos:prefLabel>
        <skos:prefLabel xml:lang="ru">Высшее образование</skos:prefLabel>
        <skos:prefLabel xml:lang="ar">تعليم عالي</skos:prefLabel>
    </owl:NamedIndividual>
    


    <!-- http://vocabularies.unesco.org/thesaurus/concept2493 -->

    <owl:NamedIndividual rdf:about="http://vocabularies.unesco.org/thesaurus/concept2493">
        <rdf:type rdf:resource="http://www.w3.org/2004/02/skos/core#Concept"/>
        <skos:broader rdf:resource="http://vocabularies.unesco.org/thesaurus/concept327"/>
        <skos:inScheme rdf:resource="http://postdata.linhd.uned.es/kos/poetic-type"/>
        <skos:topConceptOf rdf:resource="http://postdata.linhd.uned.es/kos/poetic-type"/>
        <skos:prefLabel xml:lang="es">Poesía</skos:prefLabel>
        <skos:prefLabel xml:lang="en">Poetry</skos:prefLabel>
        <skos:prefLabel xml:lang="fr">Poésie</skos:prefLabel>
        <skos:prefLabel xml:lang="ru">Поэзия</skos:prefLabel>
        <skos:prefLabel xml:lang="ar">شعر</skos:prefLabel>
    </owl:NamedIndividual>
    


    <!-- http://vocabularies.unesco.org/thesaurus/concept2533 -->

    <owl:NamedIndividual rdf:about="http://vocabularies.unesco.org/thesaurus/concept2533">
        <rdf:type rdf:resource="http://www.w3.org/2004/02/skos/core#Concept"/>
        <skos:broader rdf:resource="http://vocabularies.unesco.org/thesaurus/concept293"/>
        <skos:inScheme rdf:resource="http://postdata.linhd.uned.es/kos/religious-affiliation"/>
        <skos:topConceptOf rdf:resource="http://postdata.linhd.uned.es/kos/religious-affiliation"/>
        <skos:prefLabel xml:lang="en">Jews</skos:prefLabel>
        <skos:prefLabel xml:lang="es">Judío</skos:prefLabel>
        <skos:prefLabel xml:lang="fr">Juif</skos:prefLabel>
        <skos:prefLabel xml:lang="ru">Евреи</skos:prefLabel>
        <skos:prefLabel xml:lang="ar">يهود</skos:prefLabel>
    </owl:NamedIndividual>
    


    <!-- http://vocabularies.unesco.org/thesaurus/concept293 -->

    <owl:NamedIndividual rdf:about="http://vocabularies.unesco.org/thesaurus/concept293"/>
    


    <!-- http://vocabularies.unesco.org/thesaurus/concept327 -->

    <owl:NamedIndividual rdf:about="http://vocabularies.unesco.org/thesaurus/concept327"/>
    


    <!-- http://vocabularies.unesco.org/thesaurus/concept36 -->

    <owl:NamedIndividual rdf:about="http://vocabularies.unesco.org/thesaurus/concept36"/>
    


    <!-- http://vocabularies.unesco.org/thesaurus/concept4777 -->

    <owl:NamedIndividual rdf:about="http://vocabularies.unesco.org/thesaurus/concept4777">
        <rdf:type rdf:resource="http://www.w3.org/2004/02/skos/core#Concept"/>
        <skos:broader rdf:resource="http://vocabularies.unesco.org/thesaurus/concept293"/>
        <skos:inScheme rdf:resource="http://postdata.linhd.uned.es/kos/religious-affiliation"/>
        <skos:topConceptOf rdf:resource="http://postdata.linhd.uned.es/kos/religious-affiliation"/>
        <skos:prefLabel xml:lang="fr">Saint</skos:prefLabel>
        <skos:prefLabel xml:lang="en">Saints</skos:prefLabel>
        <skos:prefLabel xml:lang="es">Santo</skos:prefLabel>
        <skos:prefLabel xml:lang="ru">Святые</skos:prefLabel>
        <skos:prefLabel xml:lang="ar">قديسون</skos:prefLabel>
    </owl:NamedIndividual>
    


    <!-- http://vocabularies.unesco.org/thesaurus/concept4979 -->

    <owl:NamedIndividual rdf:about="http://vocabularies.unesco.org/thesaurus/concept4979">
        <rdf:type rdf:resource="http://www.w3.org/2004/02/skos/core#Concept"/>
        <skos:broader rdf:resource="http://vocabularies.unesco.org/thesaurus/concept293"/>
        <skos:inScheme rdf:resource="http://postdata.linhd.uned.es/kos/religious-affiliation"/>
        <skos:topConceptOf rdf:resource="http://postdata.linhd.uned.es/kos/religious-affiliation"/>
        <skos:prefLabel xml:lang="fr">Chef religieux</skos:prefLabel>
        <skos:prefLabel xml:lang="es">Jefe religioso</skos:prefLabel>
        <skos:prefLabel xml:lang="en">Religious leaders</skos:prefLabel>
        <skos:prefLabel xml:lang="ru">Религиозные лидеры</skos:prefLabel>
        <skos:prefLabel xml:lang="ar">زعماء دينيون</skos:prefLabel>
    </owl:NamedIndividual>
    


    <!-- http://vocabularies.unesco.org/thesaurus/concept5081 -->

    <owl:NamedIndividual rdf:about="http://vocabularies.unesco.org/thesaurus/concept5081">
        <rdf:type rdf:resource="http://www.w3.org/2004/02/skos/core#Concept"/>
        <skos:broader rdf:resource="http://vocabularies.unesco.org/thesaurus/concept36"/>
        <skos:inScheme rdf:resource="http://postdata.linhd.uned.es/kos/education-level"/>
        <skos:topConceptOf rdf:resource="http://postdata.linhd.uned.es/kos/education-level"/>
        <skos:prefLabel xml:lang="en">Early childhood education</skos:prefLabel>
        <skos:prefLabel xml:lang="es">Educación de la primera infancia</skos:prefLabel>
        <skos:prefLabel xml:lang="fr">Éducation de la prime enfance</skos:prefLabel>
        <skos:prefLabel xml:lang="ru">Раннее детское образование</skos:prefLabel>
        <skos:prefLabel xml:lang="ar">تعليم في مرحلة الطفولة المبكرة</skos:prefLabel>
    </owl:NamedIndividual>
    


    <!-- http://vocabularies.unesco.org/thesaurus/concept5153 -->

    <owl:NamedIndividual rdf:about="http://vocabularies.unesco.org/thesaurus/concept5153"/>
    


    <!-- http://vocabularies.unesco.org/thesaurus/concept5426 -->

    <owl:NamedIndividual rdf:about="http://vocabularies.unesco.org/thesaurus/concept5426">
        <rdf:type rdf:resource="http://www.w3.org/2004/02/skos/core#Concept"/>
        <skos:broader rdf:resource="http://vocabularies.unesco.org/thesaurus/concept293"/>
        <skos:inScheme rdf:resource="http://postdata.linhd.uned.es/kos/religious-affiliation"/>
        <skos:topConceptOf rdf:resource="http://postdata.linhd.uned.es/kos/religious-affiliation"/>
        <skos:prefLabel xml:lang="en">Clergy</skos:prefLabel>
        <skos:prefLabel xml:lang="fr">Clergé</skos:prefLabel>
        <skos:prefLabel xml:lang="es">Clero</skos:prefLabel>
        <skos:prefLabel xml:lang="ru">Духовенство</skos:prefLabel>
        <skos:prefLabel xml:lang="ar">رجال الدين</skos:prefLabel>
    </owl:NamedIndividual>
    


    <!-- http://vocabularies.unesco.org/thesaurus/concept8399 -->

    <owl:NamedIndividual rdf:about="http://vocabularies.unesco.org/thesaurus/concept8399">
        <rdf:type rdf:resource="http://www.w3.org/2004/02/skos/core#Concept"/>
        <skos:broader rdf:resource="http://vocabularies.unesco.org/thesaurus/concept327"/>
        <skos:inScheme rdf:resource="http://postdata.linhd.uned.es/kos/poetic-type"/>
        <skos:topConceptOf rdf:resource="http://postdata.linhd.uned.es/kos/poetic-type"/>
        <skos:prefLabel xml:lang="en">Drama</skos:prefLabel>
        <skos:prefLabel xml:lang="es">Drama</skos:prefLabel>
        <skos:prefLabel xml:lang="fr">Drame</skos:prefLabel>
        <skos:prefLabel xml:lang="ru">Драма</skos:prefLabel>
        <skos:prefLabel xml:lang="ar">دراما</skos:prefLabel>
    </owl:NamedIndividual>
    


    <!-- http://vocabularies.unesco.org/thesaurus/concept9290 -->

    <owl:NamedIndividual rdf:about="http://vocabularies.unesco.org/thesaurus/concept9290">
        <rdf:type rdf:resource="http://www.w3.org/2004/02/skos/core#Concept"/>
        <skos:broader rdf:resource="http://vocabularies.unesco.org/thesaurus/concept36"/>
        <skos:inScheme rdf:resource="http://postdata.linhd.uned.es/kos/education-level"/>
        <skos:topConceptOf rdf:resource="http://postdata.linhd.uned.es/kos/education-level"/>
        <skos:prefLabel xml:lang="fr">Enseignement primaire</skos:prefLabel>
        <skos:prefLabel xml:lang="es">Enseñanza primaria</skos:prefLabel>
        <skos:prefLabel xml:lang="en">Primary education</skos:prefLabel>
        <skos:prefLabel xml:lang="ru">Начальное образование</skos:prefLabel>
        <skos:prefLabel xml:lang="ar">تعليم ابتدائي</skos:prefLabel>
    </owl:NamedIndividual>
    


    <!-- http://vocabularies.unesco.org/thesaurus/concept9291 -->

    <owl:NamedIndividual rdf:about="http://vocabularies.unesco.org/thesaurus/concept9291">
        <rdf:type rdf:resource="http://www.w3.org/2004/02/skos/core#Concept"/>
        <skos:broader rdf:resource="http://vocabularies.unesco.org/thesaurus/concept36"/>
        <skos:inScheme rdf:resource="http://postdata.linhd.uned.es/kos/education-level"/>
        <skos:topConceptOf rdf:resource="http://postdata.linhd.uned.es/kos/education-level"/>
        <skos:prefLabel xml:lang="fr">Enseignement secondaire</skos:prefLabel>
        <skos:prefLabel xml:lang="es">Enseñanza secundaria</skos:prefLabel>
        <skos:prefLabel xml:lang="en">Secondary education</skos:prefLabel>
        <skos:prefLabel xml:lang="ru">Среднее образование</skos:prefLabel>
        <skos:prefLabel xml:lang="ar">تعليم ثانوي</skos:prefLabel>
    </owl:NamedIndividual>
    <rdf:Description>
        <owl:maxQualifiedCardinality rdf:datatype="http://www.w3.org/2001/XMLSchema#nonNegativeInteger">1</owl:maxQualifiedCardinality>
    </rdf:Description>
    <rdf:Description>
        <owl:maxQualifiedCardinality rdf:datatype="http://www.w3.org/2001/XMLSchema#nonNegativeInteger">1</owl:maxQualifiedCardinality>
    </rdf:Description>
    <rdf:Description>
        <owl:maxQualifiedCardinality rdf:datatype="http://www.w3.org/2001/XMLSchema#nonNegativeInteger">1</owl:maxQualifiedCardinality>
    </rdf:Description>
    


    <!-- 
    ///////////////////////////////////////////////////////////////////////////////////////
    //
    // Annotations
    //
    ///////////////////////////////////////////////////////////////////////////////////////
     -->

    <rdf:Description rdf:about="http://iflastandards.info/ns/fr/frbr/frbroo/">
        <skos:note xml:lang="en">Element set of the Functional Requirements for Bibliographic Records object-oriented extension to the the CIDOC Conceptual Reference Model (CRM)</skos:note>
        <dc:title xml:lang="en">FRBRoo model</dc:title>
    </rdf:Description>
    <rdf:Description rdf:about="http://iflastandards.info/ns/fr/frbr/frbroo/F1">
        <skos:scopeNote xml:lang="en">The substance of Work is concepts. A Work may be elaborated by one or more Actors simultaneously or over time. A Work may have members that constitute components of the overall concept or that are alternatives to other members of the work. Members of a work may or may not represent the concept of the Work as a whole; for instance a translation reinterprets the whole, a volume of a trilogy represents a part of the concept. A Work can be either individual or complex. If it is individual its concept is completely realised in a single F22 Self-Contained Expression. If it is complex its concept is embedded in an F15 Complex Work. An F15 Complex Work consists of members that are either F15 Complex Works themselves or F14 Individual Works. The member relationship of Work is based on the members respecting the same concept, and should not be confused with the structural parts of an expression, that might be taken from other work(s). A Work is the product of an intellectual process of one or more persons, yet only indirect evidence about it is at our hands. This can be contextual information such as the existence of an order for a work, reflections of the creators themselves that are documented somewhere, and finally the expressions of the work created. As ideas normally take shape during discussion, elaboration and implementation, it is not reasonable to assume that a work starts with a complete concept. Moreover, it can be very difficult or impossible to define the whole of the concept of a work at some given time. The only objective evidence for such a notion can be based on a stage of expressions at a given time. In this sense, self-contained expressions serve as a kind of &quot;snap-shots&quot; of a work. A Work may aggregate expressions of other works into a new expression. For instance, an anthology of poems is regarded as a work in its own right that makes use of expressions of the individual poems that have been selected and ordered as part of an intellectual process. This does not make the contents of the aggregated expressions part of this work, but only parts of the resulting expression.</skos:scopeNote>
        <regap:name xml:lang="en">Work</regap:name>
        <skos:definition xml:lang="en">This class comprises the sums of concepts which appear in the course of the coherent evolution of an original idea into one or more expressions that are dominated by the original idea.</skos:definition>
        <rdfs:label xml:lang="en">Work</rdfs:label>
        <rdfs:isDefinedBy rdf:resource="http://iflastandards.info/ns/fr/frbr/frbroo/"/>
        <rdfs:comment xml:lang="en">This class comprises the sums of concepts which appear in the course of the coherent evolution of an original idea into one or more expressions that are dominated by the original idea. The substance of Work is concepts. A Work may be elaborated by one or more Actors simultaneously or over time. A Work may have members that constitute components of the overall concept or that are alternatives to other members of the work. Members of a work may or may not represent the concept of the Work as a whole; for instance a translation reinterprets the whole, a volume of a trilogy represents a part of the concept. A Work can be either individual or complex. If it is individual its concept is completely realised in a single F22 Self-Contained Expression. If it is complex its concept is embedded in an F15 Complex Work. An F15 Complex Work consists of members that are either F15 Complex Works themselves or F14 Individual Works. The member relationship of Work is based on the members respecting the same concept, and should not be confused with the structural parts of an expression, that might be taken from other work(s). A Work is the product of an intellectual process of one or more persons, yet only indirect evidence about it is at our hands. This can be contextual information such as the existence of an order for a work, reflections of the creators themselves that are documented somewhere, and finally the expressions of the work created. As ideas normally take shape during discussion, elaboration and implementation, it is not reasonable to assume that a work starts with a complete concept. Moreover, it can be very difficult or impossible to define the whole of the concept of a work at some given time. The only objective evidence for such a notion can be based on a stage of expressions at a given time. In this sense, self-contained expressions serve as a kind of &quot;snap-shots&quot; of a work. A Work may aggregate expressions of other works into a new expression. For instance, an anthology of poems is regarded as a work in its own right that makes use of expressions of the individual poems that have been selected and ordered as part of an intellectual process. This does not make the contents of the aggregated expressions part of this work, but only parts of the resulting expression.</rdfs:comment>
    </rdf:Description>
    <rdf:Description rdf:about="http://iflastandards.info/ns/fr/frbr/frbroo/F14">
        <rdfs:isDefinedBy rdf:resource="http://iflastandards.info/ns/fr/frbr/frbroo/"/>
        <rdfs:comment xml:lang="en">This class comprises works that are realised by one and only one self-contained expression, i.e., works representing the concept as expressed by precisely this expression, and that do not have other works as parts. Inherent to the notion of work is the completion of recognisable outcomes of the work. These outcomes, i.e. the Self-Contained Expressions, are regarded as the symbolic equivalents of Individual Works, which form the atoms of a complex work. Normally creators would characterise an outcome of a work as finished. In other cases, one could recognise an outcome of a work as complete from the elaboration or logical coherence of its content, or if there is any historical knowledge about the creator deliberately or accidentally never finishing (completing) that particular expression. In all those cases, one would regard the corresponding expression as equivalent to one Individual Work.</rdfs:comment>
        <rdfs:label xml:lang="en">Individual Work</rdfs:label>
        <regap:name xml:lang="en">IndividualWork</regap:name>
        <skos:scopeNote xml:lang="en">Inherent to the notion of work is the completion of recognisable outcomes of the work. These outcomes, i.e. the Self-Contained Expressions, are regarded as the symbolic equivalents of Individual Works, which form the atoms of a complex work. Normally creators would characterise an outcome of a work as finished. In other cases, one could recognise an outcome of a work as complete from the elaboration or logical coherence of its content, or if there is any historical knowledge about the creator deliberately or accidentally never finishing (completing) that particular expression. In all those cases, one would regard the corresponding expression as equivalent to one Individual Work.</skos:scopeNote>
        <skos:definition xml:lang="en">This class comprises works that are realised by one and only one self-contained expression, i.e., works representing the concept as expressed by precisely this expression, and that do not have other works as parts.</skos:definition>
    </rdf:Description>
    <rdf:Description rdf:about="http://iflastandards.info/ns/fr/frbr/frbroo/F17">
        <rdfs:label xml:lang="en">Aggregation Work</rdfs:label>
        <regap:name xml:lang="en">http://iflastandards.info/ns/fr/frbr/frbroo/F16</regap:name>
        <regap:name xml:lang="en">AggregationWork</regap:name>
        <rdfs:comment xml:lang="en">This class comprises works whose essence is the selection and/or arrangement of expressions of one or more other works. This does not make the contents of the aggregated expressions part of this work, but only part of the resulting expression. F17 Aggregation Work may include additional original parts. An expression of a work may include expressions of other works within it. For instance, an anthology of poems is regarded as a work in its own right that makes use of expressions of the individual poems that have been selected and ordered as part of an intellectual process. A new version of an aggregate work does not make the resulting complex work an aggregate work as well. The inclusion of expressions from a complex work in an aggregation work does not make the aggregation work itself complex.</rdfs:comment>
        <rdfs:isDefinedBy rdf:resource="http://iflastandards.info/ns/fr/frbr/frbroo/"/>
    </rdf:Description>
    <rdf:Description rdf:about="http://iflastandards.info/ns/fr/frbr/frbroo/F2">
        <regap:name xml:lang="en">Expression</regap:name>
        <rdfs:label xml:lang="en">Expression</rdfs:label>
        <skos:definition xml:lang="en">This class comprises the intellectual or artistic realisations of works in the form of identifiable immaterial objects, such as texts, poems, jokes, musical or choreographic notations, movement pattern, sound pattern, images, multimedia objects, or any combination of such forms that have objectively recognisable structures.</skos:definition>
        <rdfs:comment xml:lang="en">This class comprises the intellectual or artistic realisations of works in the form of identifiable immaterial objects, such as texts, poems, jokes, musical or choreographic notations, movement pattern, sound pattern, images, multimedia objects, or any combination of such forms that have objectively recognisable structures. The substance of F2 Expression is signs. Expressions cannot exist without a physical carrier, but do not depend on a specific physical carrier and can exist on one or more carriers simultaneously. Carriers may include human memory. Inasmuch as the form of F2 Expression is an inherent characteristic of the F2 Expression, any change in form (e.g., from alpha-numeric notation to spoken word, a poem created in capitals and rendered in lower case) is a new F2 Expression. Similarly, changes in the intellectual conventions or instruments that are employed to express a work (e.g., translation from one language to another) result in the creation of a new F2 Expression. Thus, if a text is revised or modified, the resulting F2 Expression is considered to be a new F2 Expression. Minor changes, such as corrections of spelling and punctuation, etc., are normally considered variations within the same F2 Expression. On a practical level, the degree to which distinctions are made between variant expressions of a work will depend to some extent on the nature of the F1 Work itself, and on the anticipated needs of users. The genre of the work may provide an indication of which features are essential to the expression. In some cases, aspects of physical form, such as typeface and page layout, are not integral to the intellectual or artistic realisation of the work as such, and therefore are not distinctive criteria for the respective expressions. For another work features such as layout may be essential. For instance, the author or a graphic designer may wrap a poem around an image. An expression of a work may include expressions of other works within it. For instance, an anthology of poems is regarded as a work in its own right that makes use of expressions of the individual poems that have been selected and ordered as part of an intellectual process. This does not make the contents of the aggregated expressions part of this work, but only parts of the resulting expression. If an instance of F2 Expression is of a specific form, such as text, image, etc., it may be simultaneously instantiated in the specific classes representing these forms in CIDOC CRM. Thereby one can make use of the more specific properties of these classes, such as language (which is applicable to linguistic objects only).</rdfs:comment>
        <skos:scopeNote xml:lang="en">The substance of F2 Expression is signs. Expressions cannot exist without a physical carrier, but do not depend on a specific physical carrier and can exist on one or more carriers simultaneously. Carriers may include human memory. Inasmuch as the form of F2 Expression is an inherent characteristic of the F2 Expression, any change in form (e.g., from alpha-numeric notation to spoken word, a poem created in capitals and rendered in lower case) is a new F2 Expression. Similarly, changes in the intellectual conventions or instruments that are employed to express a work (e.g., translation from one language to another) result in the creation of a new F2 Expression. Thus, if a text is revised or modified, the resulting F2 Expression is considered to be a new F2 Expression. Minor changes, such as corrections of spelling and punctuation, etc., are normally considered variations within the same F2 Expression. On a practical level, the degree to which distinctions are made between variant expressions of a work will depend to some extent on the nature of the F1 Work itself, and on the anticipated needs of users. The genre of the work may provide an indication of which features are essential to the expression. In some cases, aspects of physical form, such as typeface and page layout, are not integral to the intellectual or artistic realisation of the work as such, and therefore are not distinctive criteria for the respective expressions. For another work features such as layout may be essential. For instance, the author or a graphic designer may wrap a poem around an image. An expression of a work may include expressions of other works within it. For instance, an anthology of poems is regarded as a work in its own right that makes use of expressions of the individual poems that have been selected and ordered as part of an intellectual process. This does not make the contents of the aggregated expressions part of this work, but only parts of the resulting expression. If an instance of F2 Expression is of a specific form, such as text, image, etc., it may be simultaneously instantiated in the specific classes representing these forms in CIDOC CRM. Thereby one can make use of the more specific properties of these classes, such as language (which is applicable to linguistic objects only).</skos:scopeNote>
        <rdfs:isDefinedBy rdf:resource="http://iflastandards.info/ns/fr/frbr/frbroo/"/>
    </rdf:Description>
    <rdf:Description rdf:about="http://iflastandards.info/ns/fr/frbr/frbroo/F22">
        <regap:name xml:lang="en">SelfContainedExpression</regap:name>
        <rdfs:label xml:lang="en">Self Contained Expression</rdfs:label>
        <rdfs:comment xml:lang="en">This class comprises the immaterial realisations of individual works at a particular time that are regarded as a complete whole. The quality of wholeness reflects the intention of its creator that this expression should convey the concept of the work. Such a whole can in turn be part of a larger whole. Inherent to the notion of work is the completion of recognisable outcomes of the work. These outcomes, i.e. the Self-Contained Expressions, are regarded as the symbolic equivalents of Individual Works, which form the atoms of a complex work. A Self-Contained Expression may contain expressions or parts of expressions from other work, such as citations or items collected in anthologies. Even though they are incorporated in the Self-Contained Expression, they are not regarded as becoming members of the expressed container work by their inclusion in the expression, but are rather regarded as foreign or referred elements. F22 Self-Contained Expression can be distinguished from F23 Expression Fragment in that an F23 Expression Fragment was not intended by its creator to make sense by itself. Normally creators would characterise an outcome of a work as finished. In other cases, one could recognise an outcome of a work as complete from the elaboration or logical coherence of its content, or if there is any historical knowledge about the creator deliberately or accidentally never finishing (completing) that particular expression. In all those cases, one would regard an expression as self-contained.</rdfs:comment>
        <skos:definition xml:lang="en">This class comprises the immaterial realisations of individual works at a particular time that are regarded as a complete whole.</skos:definition>
        <rdfs:isDefinedBy rdf:resource="http://iflastandards.info/ns/fr/frbr/frbroo/"/>
        <skos:scopeNote xml:lang="en">The quality of wholeness reflects the intention of its creator that this expression should convey the concept of the work. Such a whole can in turn be part of a larger whole. Inherent to the notion of work is the completion of recognisable outcomes of the work. These outcomes, i.e. the Self-Contained Expressions, are regarded as the symbolic equivalents of Individual Works, which form the atoms of a complex work. A Self-Contained Expression may contain expressions or parts of expressions from other work, such as citations or items collected in anthologies. Even though they are incorporated in the Self-Contained Expression, they are not regarded as becoming members of the expressed container work by their inclusion in the expression, but are rather regarded as foreign or referred elements. F22 Self-Contained Expression can be distinguished from F23 Expression Fragment in that an F23 Expression Fragment was not intended by its creator to make sense by itself. Normally creators would characterise an outcome of a work as finished. In other cases, one could recognise an outcome of a work as complete from the elaboration or logical coherence of its content, or if there is any historical knowledge about the creator deliberately or accidentally never finishing (completing) that particular expression. In all those cases, one would regard an expression as self-contained.</skos:scopeNote>
    </rdf:Description>
    <rdf:Description rdf:about="http://schema.org/endDate">
        <rdfs:isDefinedBy>https://schema.org/endDate</rdfs:isDefinedBy>
        <rdfs:label xml:lang="en">endDate</rdfs:label>
        <rdfs:comment xml:lang="en">The end date and time of the item (in &lt;a href=&quot;http://en.wikipedia.org/wiki/ISO_8601&quot;&gt;ISO 8601 date format&lt;/a&gt;).</rdfs:comment>
    </rdf:Description>
    <rdf:Description rdf:about="http://schema.org/startDate">
        <rdfs:label xml:lang="en">startDate</rdfs:label>
    </rdf:Description>
    <rdf:Description rdf:about="http://www.europeana.eu/schemas/edm/language">
        <rdfs:label xml:lang="en">Europeana Language</rdfs:label>
        <skos:definition xml:lang="en">The value for this element is added by the Data Ingestion Team as part of the ingestion process, based on the language of the data provider.</skos:definition>
    </rdf:Description>
    <rdf:Description rdf:about="http://www.europeana.eu/schemas/edm/unstored">
        <skos:definition xml:lang="en">This is a container element which includes all relevant information that
otherwise cannot be mapped to another element in the ESE.</skos:definition>
        <rdfs:label xml:lang="en">Unstored</rdfs:label>
    </rdf:Description>
    <rdf:Description rdf:about="http://www.w3.org/2003/06/sw-vocab-status/ns#moreinfo">
        <rdfs:isDefinedBy rdf:resource="http://www.w3.org/2003/06/sw-vocab-status/ns#"/>
        <ns2:term_status>unstable</ns2:term_status>
        <rdfs:label>more info</rdfs:label>
        <rdfs:comment>more information about the status etc of a term, typically human oriented</rdfs:comment>
    </rdf:Description>
    <rdf:Description rdf:about="http://www.w3.org/2003/06/sw-vocab-status/ns#userdocs">
        <rdfs:isDefinedBy rdf:resource="http://www.w3.org/2003/06/sw-vocab-status/ns#"/>
        <ns2:term_status>unstable</ns2:term_status>
        <rdfs:comment>human-oriented documentation, examples etc for use of this term</rdfs:comment>
        <rdfs:label>user docs</rdfs:label>
    </rdf:Description>
</rdf:RDF>



<!-- Generated by the OWL API (version 4.5.9.2019-02-01T07:24:44Z) https://github.com/owlcs/owlapi -->

